{
    "@graph": [
        {
            "@id": "oslc_cm:Enhancement",
            "rdfs:comment": "A request for new functionality.",
            "rdfs:label": "Enhancement",
            "rdfs:isDefinedBy": {
                "@id": "http://open-services.net/ns/cm#"
            },
            "rdfs:subClassOf": {
                "@id": "oslc_cm:ChangeRequest"
            },
            "@type": "rdfs:Class"
        },
        {
            "@id": "http://open-services.net/ns/cm#",
            "dcterms:issued": {
                "@value": "2023-07-06",
                "@type": "http://www.w3.org/2001/XMLSchema#date"
            },
            "dcterms:license": {
                "@id": "http://www.apache.org/licenses/LICENSE-2.0"
            },
            "dcterms:hasVersion": "OS",
            "dcterms:description": {
                "@value": "All vocabulary URIs defined in the OSLC Change Management (CM) namespace.",
                "@type": "rdf:XMLLiteral"
            },
            "dcterms:publisher": {
                "@id": "https://open-services.net/about/"
            },
            "dcterms:title": "The OSLC Change Management(CM) Vocabulary",
            "@type": "owl:Ontology",
            "rdfs:label": "The OSLC Change Management(CM) Vocabulary",
            "dcterms:isPartOf": {
                "@id": "https://docs.oasis-open-projects.org/oslc-op/cm/v3.0/errata01/os/change-mgt-spec.html"
            },
            "dcterms:source": {
                "@id": "https://docs.oasis-open-projects.org/oslc-op/cm/v3.0/errata01/os/change-mgt-vocab.ttl"
            },
            "vann:preferredNamespacePrefix": "oslc_cm"
        },
        {
            "@id": "oslc_cm:ChangeRequest",
            "rdfs:comment": "The CM Change Request resource.",
            "rdfs:label": "ChangeRequest",
            "rdfs:isDefinedBy": {
                "@id": "http://open-services.net/ns/cm#"
            },
            "@type": "rdfs:Class"
        },
        {
            "@id": "oslc_cm:tracksRequirement",
            "rdfs:comment": "Tracks the associated Requirement or Requirement\nChangeSet resources. It is likely that the target resource will be an\noslc_rm:Requirement.",
            "rdfs:label": "tracksRequirement",
            "rdfs:isDefinedBy": {
                "@id": "http://open-services.net/ns/cm#"
            },
            "@type": "rdf:Property"
        },
        {
            "@id": "oslc_cm:authorizer",
            "rdfs:comment": "The URI of a resource describing an agent who is responsible authorizing for and/or has authorized effort to be expended to address a set of change requests.",
            "rdfs:label": "authorizer",
            "rdfs:isDefinedBy": {
                "@id": "http://open-services.net/ns/cm#"
            },
            "@type": "rdf:Property"
        },
        {
            "@id": "oslc_cm:testedByTestCase",
            "rdfs:comment": "Test case by which this change request is tested. It is\nlikely that the target resource will be an oslc_qm:TestCase.",
            "rdfs:label": "testedByTestCase",
            "rdfs:isDefinedBy": {
                "@id": "http://open-services.net/ns/cm#"
            },
            "@type": "rdf:Property"
        },
        {
            "@id": "oslc_cm:relatedChangeRequest",
            "rdfs:comment": "This relationship is loosely coupled, has no specific\nmeaning, and can be used to link related change requests. It is likely\nthat the target resource will be an oslc_cm:ChangeRequest.",
            "rdfs:label": "relatedChangeRequest",
            "rdfs:isDefinedBy": {
                "@id": "http://open-services.net/ns/cm#"
            },
            "@type": "rdf:Property"
        },
        {
            "@id": "oslc_cm:reviewed",
            "rdfs:comment": "Whether or not the Change Request has been reviewed.",
            "rdfs:label": "reviewed",
            "rdfs:isDefinedBy": {
                "@id": "http://open-services.net/ns/cm#"
            },
            "@type": "rdf:Property"
        },
        {
            "@id": "oslc_cm:affectsPlanItem",
            "rdfs:comment": "Change request affects a plan item. It is likely that\nthe target resource will be an oslc_cm:ChangeRequest.",
            "rdfs:label": "affectsPlanItem",
            "rdfs:isDefinedBy": {
                "@id": "http://open-services.net/ns/cm#"
            },
            "@type": "rdf:Property"
        },
        {
            "@id": "oslc_cm:Reviewed",
            "rdfs:comment": "Whether or not the Change Request has been reviewed.",
            "rdfs:label": "reviewed",
            "rdfs:isDefinedBy": {
                "@id": "http://open-services.net/ns/cm#"
            },
            "@type": "oslc_cm:State"
        },
        {
            "@id": "oslc_cm:State",
            "rdfs:comment": "Defines the possible oslc_cm:state property values.",
            "rdfs:label": "State",
            "rdfs:isDefinedBy": {
                "@id": "http://open-services.net/ns/cm#"
            },
            "@type": "rdfs:Class"
        },
        {
            "@id": "oslc_cm:severity",
            "rdfs:comment": "Used to indicate the severity or potential impact of a defect.\nIt is likely that the target resource will be an oslc_cm:Severity.",
            "rdfs:label": "severity",
            "rdfs:isDefinedBy": {
                "@id": "http://open-services.net/ns/cm#"
            },
            "@type": "rdf:Property"
        },
        {
            "@id": "oslc_cm:requirementsChangeRequest",
            "rdfs:comment": "Used for associating a change request for usage in tracking changes to a Requirements resource.",
            "rdfs:label": "requirementsChangeRequest",
            "rdfs:isDefinedBy": {
                "@id": "http://open-services.net/ns/cm#"
            },
            "@type": "rdfs:Resource"
        },
        {
            "@id": "oslc_cm:Severity",
            "rdfs:comment": "Defines the possible oslc_cm:severity property values.",
            "rdfs:label": "Severity",
            "rdfs:isDefinedBy": {
                "@id": "http://open-services.net/ns/cm#"
            },
            "@type": "rdfs:Class"
        },
        {
            "@id": "oslc_cm:status",
            "rdfs:comment": "Used to indicate the status of the change request based\non values defined by the service provider. Most often a read-only\nproperty. It is likely that the target resource will be a string corresponding to an\noslc_cm:State value.",
            "rdfs:label": "status",
            "vs:term_status": "archaic",
            "rdfs:isDefinedBy": {
                "@id": "http://open-services.net/ns/cm#"
            },
            "@type": "rdf:Property"
        },
        {
            "@id": "oslc_cm:priority",
            "rdfs:comment": "Used to indicate the relative importance of ChangeRequests.\nIt is likely that the target resource will be an\noslc_cm:Priority.",
            "rdfs:label": "priority",
            "rdfs:isDefinedBy": {
                "@id": "http://open-services.net/ns/cm#"
            },
            "@type": "rdf:Property"
        },
        {
            "@id": "oslc_cm:Fixed",
            "rdfs:comment": "Whether or not the Change Request has been fixed.",
            "rdfs:label": "fixed",
            "rdfs:isDefinedBy": {
                "@id": "http://open-services.net/ns/cm#"
            },
            "@type": "oslc_cm:State"
        },
        {
            "@id": "oslc_cm:verified",
            "rdfs:comment": "Whether or not the resolution or fix of the Change Request has been verified.",
            "rdfs:label": "verified",
            "rdfs:isDefinedBy": {
                "@id": "http://open-services.net/ns/cm#"
            },
            "@type": "rdf:Property"
        },
        {
            "@id": "oslc_cm:Priority",
            "rdfs:comment": "Defines the possible oslc_cm:priority property values.",
            "rdfs:label": "Priority",
            "rdfs:isDefinedBy": {
                "@id": "http://open-services.net/ns/cm#"
            },
            "@type": "rdfs:Class"
        },
        {
            "@id": "oslc_cm:Normal",
            "rdfs:comment": "Affects non-critical functionality. There is a workaround.",
            "rdfs:label": "Normal",
            "rdfs:isDefinedBy": {
                "@id": "http://open-services.net/ns/cm#"
            },
            "@type": "oslc_cm:Severity"
        },
        {
            "@id": "oslc_cm:state",
            "rdfs:comment": "Used to indicate the status of the change request.",
            "rdfs:label": "state",
            "rdfs:isDefinedBy": {
                "@id": "http://open-services.net/ns/cm#"
            },
            "@type": "rdf:Property"
        },
        {
            "@id": "oslc_cm:affectsTestResult",
            "rdfs:comment": "Associated resource that is affected by this Change\nRequest. It is likely that the target resource will be an\noslc_qm:TestResult.",
            "rdfs:label": "affectsTestResult",
            "rdfs:isDefinedBy": {
                "@id": "http://open-services.net/ns/cm#"
            },
            "@type": "rdf:Property"
        },
        {
            "@id": "oslc_cm:Blocker",
            "rdfs:comment": "Severe problem. No workaround. Blocks development, test, or usage.",
            "rdfs:label": "Blocker",
            "rdfs:isDefinedBy": {
                "@id": "http://open-services.net/ns/cm#"
            },
            "@type": "oslc_cm:Severity"
        },
        {
            "@id": "oslc_cm:SeverityUnassigned",
            "rdfs:comment": "The severity of the change request is intentionally not set.",
            "rdfs:label": "SeverityUnassigned",
            "rdfs:isDefinedBy": {
                "@id": "http://open-services.net/ns/cm#"
            },
            "@type": "oslc_cm:Severity"
        },
        {
            "@id": "oslc_cm:Critical",
            "rdfs:comment": "Severe problem. No workaround.",
            "rdfs:label": "Critical",
            "rdfs:isDefinedBy": {
                "@id": "http://open-services.net/ns/cm#"
            },
            "@type": "oslc_cm:Severity"
        },
        {
            "@id": "oslc_cm:closeDate",
            "rdfs:comment": "The date at which no further activity or work is intended to be conducted.",
            "rdfs:label": "closeDate",
            "rdfs:isDefinedBy": {
                "@id": "http://open-services.net/ns/cm#"
            },
            "@type": "rdf:Property"
        },
        {
            "@id": "oslc_cm:affectedByDefect",
            "rdfs:comment": "Change request is affected by a reported defect. It is\nlikely that the target resource will be an oslc_cm:Defect.",
            "rdfs:label": "affectedByDefect",
            "rdfs:isDefinedBy": {
                "@id": "http://open-services.net/ns/cm#"
            },
            "@type": "rdf:Property"
        },
        {
            "@id": "oslc_cm:Low",
            "rdfs:comment": "Action on the change request can be safely deferred.",
            "rdfs:label": "Low",
            "rdfs:isDefinedBy": {
                "@id": "http://open-services.net/ns/cm#"
            },
            "@type": "oslc_cm:Priority"
        },
        {
            "@id": "oslc_cm:planItem",
            "rdfs:comment": "Used for associating change requests into plans (project, release, sprint, etc).",
            "rdfs:label": "planItem",
            "rdfs:isDefinedBy": {
                "@id": "http://open-services.net/ns/cm#"
            },
            "@type": "rdfs:Resource"
        },
        {
            "@id": "oslc_cm:ReviewTask",
            "rdfs:comment": "A request to make a change and review the change.",
            "rdfs:label": "ReviewTask",
            "rdfs:isDefinedBy": {
                "@id": "http://open-services.net/ns/cm#"
            },
            "rdfs:subClassOf": {
                "@id": "oslc_cm:Task"
            },
            "@type": "rdfs:Class"
        },
        {
            "@id": "oslc_cm:Task",
            "rdfs:comment": "An executable and trackable activity.",
            "rdfs:label": "Task",
            "rdfs:isDefinedBy": {
                "@id": "http://open-services.net/ns/cm#"
            },
            "rdfs:subClassOf": {
                "@id": "oslc_cm:ChangeRequest"
            },
            "@type": "rdfs:Class"
        },
        {
            "@id": "oslc_cm:affectsRequirement",
            "rdfs:comment": "The ChangeRequest affects a Requirement. It is likely\nthat the target resource will be an oslc_rm:Requirement.",
            "rdfs:label": "affectsRequirement",
            "rdfs:isDefinedBy": {
                "@id": "http://open-services.net/ns/cm#"
            },
            "@type": "rdf:Property"
        },
        {
            "@id": "oslc_cm:defect",
            "rdfs:comment": "Used to report defects in testing.",
            "rdfs:label": "defect",
            "rdfs:isDefinedBy": {
                "@id": "http://open-services.net/ns/cm#"
            },
            "@type": "rdfs:Resource"
        },
        {
            "@id": "oslc_cm:Closed",
            "rdfs:comment": "Whether or not the Change Request is completely done, no further fixes or fix verification is needed.",
            "rdfs:label": "closed",
            "rdfs:isDefinedBy": {
                "@id": "http://open-services.net/ns/cm#"
            },
            "@type": "oslc_cm:State"
        },
        {
            "@id": "oslc_cm:relatedTestCase",
            "rdfs:comment": "Related test case resource. It is likely that the\ntarget resource will be an oslc_qm:TestCase.",
            "rdfs:label": "relatedTestCase",
            "rdfs:isDefinedBy": {
                "@id": "http://open-services.net/ns/cm#"
            },
            "@type": "rdf:Property"
        },
        {
            "@id": "oslc_cm:relatedTestPlan",
            "rdfs:comment": "Related test plan resource. It is likely that the\ntarget resource will be an oslc_qm:TestPlan.",
            "rdfs:label": "relatedTestPlan",
            "rdfs:isDefinedBy": {
                "@id": "http://open-services.net/ns/cm#"
            },
            "@type": "rdf:Property"
        },
        {
            "@id": "oslc_cm:parent",
            "rdfs:comment": "The related parent change requests of the subject change request.",
            "rdfs:label": "parent",
            "rdfs:isDefinedBy": {
                "@id": "http://open-services.net/ns/cm#"
            },
            "@type": "rdf:Property"
        },
        {
            "@id": "oslc_cm:ChangeNotice",
            "rdfs:comment": "Represents an assignment notification of a change request. May be used also to bestow authority onto the assigned user to effect the changes.",
            "rdfs:label": "ChangeNotice",
            "rdfs:isDefinedBy": {
                "@id": "http://open-services.net/ns/cm#"
            },
            "rdfs:subClassOf": {
                "@id": "oslc_cm:ChangeRequest"
            },
            "@type": "rdfs:Class"
        },
        {
            "@id": "oslc_cm:Approved",
            "rdfs:comment": "Whether or not the Change Request has been approved.",
            "rdfs:label": "approved",
            "rdfs:isDefinedBy": {
                "@id": "http://open-services.net/ns/cm#"
            },
            "@type": "oslc_cm:State"
        },
        {
            "@id": "oslc_cm:tracksChangeSet",
            "rdfs:comment": "Tracks a change set resource. It is likely that the\ntarget resource will be an oslc_config:ChangeSet.",
            "rdfs:label": "tracksChangeSet",
            "rdfs:isDefinedBy": {
                "@id": "http://open-services.net/ns/cm#"
            },
            "@type": "rdf:Property"
        },
        {
            "@id": "oslc_cm:implementsRequirement",
            "rdfs:comment": "The ChangeRequest implements the associated Requirement. It is likely that the\ntarget resource will be an oslc_rm:Requirement.",
            "rdfs:label": "implementsRequirement",
            "rdfs:isDefinedBy": {
                "@id": "http://open-services.net/ns/cm#"
            },
            "@type": "rdf:Property"
        },
        {
            "@id": "oslc_cm:relatedTestScript",
            "rdfs:comment": "Related test script resource. It is likely that the\ntarget resource will be an oslc_qm:TestScript.",
            "rdfs:label": "relatedTestScript",
            "rdfs:isDefinedBy": {
                "@id": "http://open-services.net/ns/cm#"
            },
            "@type": "rdf:Property"
        },
        {
            "@id": "oslc_cm:Major",
            "rdfs:comment": "Prevents function from being used. There is a workaround.",
            "rdfs:label": "Major",
            "rdfs:isDefinedBy": {
                "@id": "http://open-services.net/ns/cm#"
            },
            "@type": "oslc_cm:Severity"
        },
        {
            "@id": "oslc_cm:Minor",
            "rdfs:comment": "Minimal impact.",
            "rdfs:label": "Minor",
            "rdfs:isDefinedBy": {
                "@id": "http://open-services.net/ns/cm#"
            },
            "@type": "oslc_cm:Severity"
        },
        {
            "@id": "oslc_cm:Defect",
            "rdfs:comment": "A software or product defect.",
            "rdfs:label": "Defect",
            "rdfs:isDefinedBy": {
                "@id": "http://open-services.net/ns/cm#"
            },
            "rdfs:subClassOf": {
                "@id": "oslc_cm:ChangeRequest"
            },
            "@type": "rdfs:Class"
        },
        {
            "@id": "oslc_cm:High",
            "rdfs:comment": "Highest priority, action on the change request highly recommended.",
            "rdfs:label": "High",
            "rdfs:isDefinedBy": {
                "@id": "http://open-services.net/ns/cm#"
            },
            "@type": "oslc_cm:Priority"
        },
        {
            "@id": "oslc_cm:Inprogress",
            "rdfs:comment": "Whether or not the Change Request in a state indicating that active work is occurring.",
            "rdfs:label": "inprogress",
            "rdfs:isDefinedBy": {
                "@id": "http://open-services.net/ns/cm#"
            },
            "@type": "oslc_cm:State"
        },
        {
            "@id": "oslc_cm:task",
            "rdfs:comment": "Used for associating change requests into executable and track-able items.",
            "rdfs:label": "task",
            "rdfs:isDefinedBy": {
                "@id": "http://open-services.net/ns/cm#"
            },
            "@type": "rdfs:Resource"
        },
        {
            "@id": "oslc_cm:approved",
            "rdfs:comment": "Whether or not the Change Request has been approved.",
            "rdfs:label": "approved",
            "rdfs:isDefinedBy": {
                "@id": "http://open-services.net/ns/cm#"
            },
            "@type": "rdf:Property"
        },
        {
            "@id": "oslc_cm:fixed",
            "rdfs:comment": "Whether or not the Change Request has been fixed.",
            "rdfs:label": "fixed",
            "rdfs:isDefinedBy": {
                "@id": "http://open-services.net/ns/cm#"
            },
            "@type": "rdf:Property"
        },
        {
            "@id": "oslc_cm:blocksTestExecutionRecord",
            "rdfs:comment": "Associated resource that is blocked by this Change\nRequest. It is likely that the target resource will be an\noslc_qm:TestExecutionRecord.",
            "rdfs:label": "blocksTestExecutionRecord",
            "rdfs:isDefinedBy": {
                "@id": "http://open-services.net/ns/cm#"
            },
            "@type": "rdf:Property"
        },
        {
            "@id": "oslc_cm:inProgress",
            "rdfs:comment": "Whether or not the Change Request in a state indicating that active work is occurring.",
            "rdfs:label": "inProgress",
            "rdfs:isDefinedBy": {
                "@id": "http://open-services.net/ns/cm#"
            },
            "@type": "rdf:Property"
        },
        {
            "@id": "oslc_cm:Verified",
            "rdfs:comment": "Whether or not the resolution or fix of the Change Request has been verified.",
            "rdfs:label": "verified",
            "rdfs:isDefinedBy": {
                "@id": "http://open-services.net/ns/cm#"
            },
            "@type": "oslc_cm:State"
        },
        {
            "@id": "oslc_cm:closed",
            "rdfs:comment": "Whether or not the Change Request is completely done, no further fixes or fix verification is needed.",
            "rdfs:label": "closed",
            "rdfs:isDefinedBy": {
                "@id": "http://open-services.net/ns/cm#"
            },
            "@type": "rdf:Property"
        },
        {
            "@id": "oslc_cm:relatedTestExecutionRecord",
            "rdfs:comment": "Related to a test execution resource. It is likely\nthat the target resource will be an oslc_qm:TestExecutionRecord.",
            "rdfs:label": "relatedTestExecutionRecord",
            "rdfs:isDefinedBy": {
                "@id": "http://open-services.net/ns/cm#"
            },
            "@type": "rdf:Property"
        },
        {
            "@id": "oslc_cm:PriorityUnassigned",
            "rdfs:comment": "The priority of the change request is intentionally not set.",
            "rdfs:label": "PriorityUnassigned",
            "rdfs:isDefinedBy": {
                "@id": "http://open-services.net/ns/cm#"
            },
            "@type": "oslc_cm:Priority"
        },
        {
            "@id": "oslc_cm:Medium",
            "rdfs:comment": "Acting on the change request can wait, but not forever.",
            "rdfs:label": "Medium",
            "rdfs:isDefinedBy": {
                "@id": "http://open-services.net/ns/cm#"
            },
            "@type": "oslc_cm:Priority"
        }
    ],
    "@context": {
        "owl": "http://www.w3.org/2002/07/owl#",
        "rdf": "http://www.w3.org/1999/02/22-rdf-syntax-ns#",
        "dcterms": "http://purl.org/dc/terms/",
        "rdfs": "http://www.w3.org/2000/01/rdf-schema#",
        "vann": "http://purl.org/vocab/vann/",
        "vs": "http://www.w3.org/2003/06/sw-vocab-status/ns#",
        "oslc_cm": "http://open-services.net/ns/cm#"
    }
}
