<rdf:RDF
    xmlns:rdf="http://www.w3.org/1999/02/22-rdf-syntax-ns#"
    xmlns:dcterms="http://purl.org/dc/terms/"
    xmlns:owl="http://www.w3.org/2002/07/owl#"
    xmlns:oslc_am="http://open-services.net/ns/am#"
    xmlns:rdfs="http://www.w3.org/2000/01/rdf-schema#"
    xmlns:oslc_sysmlv2="http://open-services.net/ns/sysmlv2#"
    xmlns:vann="http://purl.org/vocab/vann/"
    xmlns:xsd="http://www.w3.org/2001/XMLSchema#">
  <owl:Ontology rdf:about="http://open-services.net/ns/sysmlv2#">
    <dcterms:license rdf:resource="http://www.apache.org/licenses/LICENSE-2.0"/>
    <vann:preferredNamespacePrefix>oslc_sysmlv2</vann:preferredNamespacePrefix>
    <dcterms:description rdf:parseType="Literal">All vocabulary URIs defined in the OSLC SysML v2 namespace.</dcterms:description>
    <dcterms:dateCopyrighted>2012-2024</dcterms:dateCopyrighted>
    <dcterms:publisher rdf:resource="https://open-services.net/about/"/>
    <dcterms:issued rdf:datatype="http://www.w3.org/2001/XMLSchema#date"
    >2024-08-01</dcterms:issued>
    <dcterms:hasVersion>PSD01</dcterms:hasVersion>
    <rdfs:label>OSLC SysML v2 Vocabulary</rdfs:label>
    <dcterms:title>OSLC SysML v2 Vocabulary</dcterms:title>
    <dcterms:source rdf:resource="https://docs.oasis-open-projects.org/oslc-op/sysml/v2.0/os/sysml-vocab.ttl"/>
    <dcterms:isPartOf rdf:resource="https://docs.oasis-open-projects.org/oslc-op/sysml/v2.0/os/sysml-spec.html"/>
  </owl:Ontology>
  <rdfs:Class rdf:about="http://open-services.net/ns/sysmlv2#ViewpointUsage">
    <rdfs:subClassOf>
      <rdfs:Class rdf:about="http://open-services.net/ns/sysmlv2#RequirementUsage"/>
    </rdfs:subClassOf>
    <rdfs:isDefinedBy rdf:resource="http://open-services.net/ns/sysmlv2#"/>
    <rdfs:comment>A ViewpointUsage is a Usage of a ViewpointDefinition.</rdfs:comment>
    <rdfs:label>ViewpointUsage</rdfs:label>
  </rdfs:Class>
  <rdfs:Class rdf:about="http://open-services.net/ns/sysmlv2#ForkNode">
    <rdfs:subClassOf>
      <rdfs:Class rdf:about="http://open-services.net/ns/sysmlv2#ControlNode"/>
    </rdfs:subClassOf>
    <rdfs:isDefinedBy rdf:resource="http://open-services.net/ns/sysmlv2#"/>
    <rdfs:comment>A ForkNode is a ControlNode that must be followed by successor Actions as given by all its outgoing Successions.</rdfs:comment>
    <rdfs:label>ForkNode</rdfs:label>
  </rdfs:Class>
  <rdfs:Class rdf:about="http://open-services.net/ns/sysmlv2#FeatureReferenceExpression">
    <rdfs:subClassOf>
      <rdfs:Class rdf:about="http://open-services.net/ns/sysmlv2#Expression"/>
    </rdfs:subClassOf>
    <rdfs:isDefinedBy rdf:resource="http://open-services.net/ns/sysmlv2#"/>
    <rdfs:comment>A FeatureReferenceExpression is an Expression whose result is bound to a referent Feature.</rdfs:comment>
    <rdfs:label>FeatureReferenceExpression</rdfs:label>
  </rdfs:Class>
  <rdfs:Class rdf:about="http://open-services.net/ns/sysmlv2#EnumerationUsage">
    <rdfs:subClassOf>
      <rdfs:Class rdf:about="http://open-services.net/ns/sysmlv2#AttributeUsage"/>
    </rdfs:subClassOf>
    <rdfs:isDefinedBy rdf:resource="http://open-services.net/ns/sysmlv2#"/>
    <rdfs:comment>An EnumerationUsage is an AttributeUsage whose attributeDefinition is an EnumerationDefinition.</rdfs:comment>
    <rdfs:label>EnumerationUsage</rdfs:label>
  </rdfs:Class>
  <rdfs:Class rdf:about="http://open-services.net/ns/sysmlv2#Behavior">
    <rdfs:subClassOf>
      <rdfs:Class rdf:about="http://open-services.net/ns/sysmlv2#Class"/>
    </rdfs:subClassOf>
    <rdfs:isDefinedBy rdf:resource="http://open-services.net/ns/sysmlv2#"/>
    <rdfs:comment>A Behavior coordinates occurrences of other Behaviors, as well as changes in objects. Behaviors can be decomposed into Steps and be characterized by parameters.</rdfs:comment>
    <rdfs:label>Behavior</rdfs:label>
  </rdfs:Class>
  <rdfs:Class rdf:about="http://open-services.net/ns/sysmlv2#SubjectMembership">
    <rdfs:subClassOf>
      <rdfs:Class rdf:about="http://open-services.net/ns/sysmlv2#ParameterMembership"/>
    </rdfs:subClassOf>
    <rdfs:isDefinedBy rdf:resource="http://open-services.net/ns/sysmlv2#"/>
    <rdfs:comment>A SubjectMembership is a ParameterMembership that indicates that its ownedSubjectParameter is the subject of its owningType. The owningType of a SubjectMembership must be a RequirementDefinition, RequirementUsage, CaseDefinition, or CaseUsage.</rdfs:comment>
    <rdfs:label>SubjectMembership</rdfs:label>
  </rdfs:Class>
  <rdfs:Class rdf:about="http://open-services.net/ns/sysmlv2#RenderingDefinition">
    <rdfs:subClassOf>
      <rdfs:Class rdf:about="http://open-services.net/ns/sysmlv2#PartDefinition"/>
    </rdfs:subClassOf>
    <rdfs:isDefinedBy rdf:resource="http://open-services.net/ns/sysmlv2#"/>
    <rdfs:comment>A RenderingDefinition is a PartDefinition that defines a specific rendering of the content of a model view (e.g., symbols, style, layout, etc.).</rdfs:comment>
    <rdfs:label>RenderingDefinition</rdfs:label>
  </rdfs:Class>
  <rdfs:Class rdf:about="http://open-services.net/ns/sysmlv2#LifeClass">
    <rdfs:subClassOf>
      <rdfs:Class rdf:about="http://open-services.net/ns/sysmlv2#Class"/>
    </rdfs:subClassOf>
    <rdfs:isDefinedBy rdf:resource="http://open-services.net/ns/sysmlv2#"/>
    <rdfs:comment>A LifeClass is a Class that specializes both the Class Occurrences::Life from the Kernel Semantic Library and a single OccurrenceDefinition, and has a multiplicity of 0..1. This constrains the OccurrenceDefinition being specialized to have at most one instance that is a complete Life.</rdfs:comment>
    <rdfs:label>LifeClass</rdfs:label>
  </rdfs:Class>
  <rdfs:Class rdf:about="http://open-services.net/ns/sysmlv2#MetadataFeature">
    <rdfs:subClassOf>
      <rdfs:Class rdf:about="http://open-services.net/ns/sysmlv2#Feature"/>
    </rdfs:subClassOf>
    <rdfs:subClassOf>
      <rdfs:Class rdf:about="http://open-services.net/ns/sysmlv2#AnnotatingElement"/>
    </rdfs:subClassOf>
    <rdfs:isDefinedBy rdf:resource="http://open-services.net/ns/sysmlv2#"/>
    <rdfs:comment>A MetadataFeature is a Feature that is an AnnotatingElement used to annotate another Element with metadata. It is typed by a Metaclass. All its ownedFeatures must redefine features of its metaclass and any feature bindings must be model-level evaluable.</rdfs:comment>
    <rdfs:label>MetadataFeature</rdfs:label>
  </rdfs:Class>
  <rdfs:Class rdf:about="http://open-services.net/ns/sysmlv2#BindingConnector">
    <rdfs:subClassOf>
      <rdfs:Class rdf:about="http://open-services.net/ns/sysmlv2#Connector"/>
    </rdfs:subClassOf>
    <rdfs:isDefinedBy rdf:resource="http://open-services.net/ns/sysmlv2#"/>
    <rdfs:comment>A BindingConnector is a binary Connector that requires its relatedFeatures to identify the same things (have the same values).</rdfs:comment>
    <rdfs:label>BindingConnector</rdfs:label>
  </rdfs:Class>
  <rdfs:Class rdf:about="http://open-services.net/ns/sysmlv2#FramedConcernMembership">
    <rdfs:subClassOf>
      <rdfs:Class rdf:about="http://open-services.net/ns/sysmlv2#RequirementConstraintMembership"/>
    </rdfs:subClassOf>
    <rdfs:isDefinedBy rdf:resource="http://open-services.net/ns/sysmlv2#"/>
    <rdfs:comment>A FramedConcernMembership is a RequirementConstraintMembership for a framed ConcernUsage of a RequirementDefinition or RequirementUsage.</rdfs:comment>
    <rdfs:label>FramedConcernMembership</rdfs:label>
  </rdfs:Class>
  <rdfs:Class rdf:about="http://open-services.net/ns/sysmlv2#Usage">
    <rdfs:subClassOf>
      <rdfs:Class rdf:about="http://open-services.net/ns/sysmlv2#Feature"/>
    </rdfs:subClassOf>
    <rdfs:isDefinedBy rdf:resource="http://open-services.net/ns/sysmlv2#"/>
    <rdfs:comment>A Usage is a usage of a Definition. A Usage may only be an ownedFeature of a Definition or another Usage.</rdfs:comment>
    <rdfs:label>Usage</rdfs:label>
  </rdfs:Class>
  <rdfs:Class rdf:about="http://open-services.net/ns/sysmlv2#Classifier">
    <rdfs:subClassOf>
      <rdfs:Class rdf:about="http://open-services.net/ns/sysmlv2#Type"/>
    </rdfs:subClassOf>
    <rdfs:isDefinedBy rdf:resource="http://open-services.net/ns/sysmlv2#"/>
    <rdfs:comment>A Classifier is a Type that classifies:.</rdfs:comment>
    <rdfs:label>Classifier</rdfs:label>
  </rdfs:Class>
  <rdfs:Class rdf:about="http://open-services.net/ns/sysmlv2#AssertConstraintUsage">
    <rdfs:subClassOf>
      <rdfs:Class rdf:about="http://open-services.net/ns/sysmlv2#Invariant"/>
    </rdfs:subClassOf>
    <rdfs:subClassOf>
      <rdfs:Class rdf:about="http://open-services.net/ns/sysmlv2#ConstraintUsage"/>
    </rdfs:subClassOf>
    <rdfs:isDefinedBy rdf:resource="http://open-services.net/ns/sysmlv2#"/>
    <rdfs:comment>An AssertConstraintUsage is a ConstraintUsage that is also an Invariant and, so, is asserted to be true (by default). Unless it is the AssertConstraintUsage itself, the asserted ConstraintUsage is related to the AssertConstraintUsage by a ReferenceSubsetting Relationship.</rdfs:comment>
    <rdfs:label>AssertConstraintUsage</rdfs:label>
  </rdfs:Class>
  <rdfs:Class rdf:about="http://open-services.net/ns/sysmlv2#ActionUsage">
    <rdfs:subClassOf>
      <rdfs:Class rdf:about="http://open-services.net/ns/sysmlv2#Step"/>
    </rdfs:subClassOf>
    <rdfs:subClassOf>
      <rdfs:Class rdf:about="http://open-services.net/ns/sysmlv2#OccurrenceUsage"/>
    </rdfs:subClassOf>
    <rdfs:isDefinedBy rdf:resource="http://open-services.net/ns/sysmlv2#"/>
    <rdfs:comment>An ActionUsage is a Usage that is also a Step, and, so, is typed by a Behavior. Nominally, if the type is an ActionDefinition, an ActionUsage is a Usage of that ActionDefinition within a system. However, other kinds of kernel Behaviors are also allowed, to permit use of Behaviors from the Kernel Model Libraries.</rdfs:comment>
    <rdfs:label>ActionUsage</rdfs:label>
  </rdfs:Class>
  <rdfs:Class rdf:about="http://open-services.net/ns/sysmlv2#CalculationUsage">
    <rdfs:subClassOf>
      <rdfs:Class rdf:about="http://open-services.net/ns/sysmlv2#Expression"/>
    </rdfs:subClassOf>
    <rdfs:subClassOf rdf:resource="http://open-services.net/ns/sysmlv2#ActionUsage"/>
    <rdfs:isDefinedBy rdf:resource="http://open-services.net/ns/sysmlv2#"/>
    <rdfs:comment>A CalculationUsage is an ActionUsage that is also an Expression, and, so, is typed by a Function. Nominally, if the type is a CalculationDefinition, a CalculationUsage is a Usage of that CalculationDefinition within a system. However, other kinds of kernel Functions are also allowed, to permit use of Functions from the Kernel Model Libraries.</rdfs:comment>
    <rdfs:label>CalculationUsage</rdfs:label>
  </rdfs:Class>
  <rdfs:Class rdf:about="http://open-services.net/ns/sysmlv2#AnalysisCaseUsage">
    <rdfs:subClassOf>
      <rdfs:Class rdf:about="http://open-services.net/ns/sysmlv2#CaseUsage"/>
    </rdfs:subClassOf>
    <rdfs:isDefinedBy rdf:resource="http://open-services.net/ns/sysmlv2#"/>
    <rdfs:comment>An AnalysisCaseUsage is a Usage of an AnalysisCaseDefinition.</rdfs:comment>
    <rdfs:label>AnalysisCaseUsage</rdfs:label>
  </rdfs:Class>
  <rdfs:Class rdf:about="http://open-services.net/ns/sysmlv2#CalculationDefinition">
    <rdfs:subClassOf>
      <rdfs:Class rdf:about="http://open-services.net/ns/sysmlv2#Function"/>
    </rdfs:subClassOf>
    <rdfs:subClassOf>
      <rdfs:Class rdf:about="http://open-services.net/ns/sysmlv2#ActionDefinition"/>
    </rdfs:subClassOf>
    <rdfs:isDefinedBy rdf:resource="http://open-services.net/ns/sysmlv2#"/>
    <rdfs:comment>A CalculationDefinition is an ActionDefinition that also defines a Function producing a result.</rdfs:comment>
    <rdfs:label>CalculationDefinition</rdfs:label>
  </rdfs:Class>
  <rdfs:Class rdf:about="http://open-services.net/ns/sysmlv2#Redefinition">
    <rdfs:subClassOf>
      <rdfs:Class rdf:about="http://open-services.net/ns/sysmlv2#Subsetting"/>
    </rdfs:subClassOf>
    <rdfs:isDefinedBy rdf:resource="http://open-services.net/ns/sysmlv2#"/>
    <rdfs:comment>Redefinition is a kind of Subsetting that requires the redefinedFeature and the redefiningFeature to have the same values (on each instance of the domain of the redefiningFeature). This means any restrictions on the redefiningFeature, such as type or multiplicity, also apply to the redefinedFeature (on each instance of the domain of the redefiningFeature), and vice versa. The redefinedFeature might have values for instances of the domain of the redefiningFeature, but only as instances of the domain of the redefinedFeature that happen to also be instances of the domain of the redefiningFeature. This is supported by the constraints inherited from Subsetting on the domains of the redefiningFeature and redefinedFeature. However, these constraints are narrowed for Redefinition to require the owningTypes of the redefiningFeature and redefinedFeature to be different and the redefinedFeature to not be inherited into the owningNamespace of the redefiningFeature.This enables the redefiningFeature to have the same name as the redefinedFeature, if desired.</rdfs:comment>
    <rdfs:label>Redefinition</rdfs:label>
  </rdfs:Class>
  <rdfs:Class rdf:about="http://open-services.net/ns/sysmlv2#Succession">
    <rdfs:subClassOf>
      <rdfs:Class rdf:about="http://open-services.net/ns/sysmlv2#Connector"/>
    </rdfs:subClassOf>
    <rdfs:isDefinedBy rdf:resource="http://open-services.net/ns/sysmlv2#"/>
    <rdfs:comment>A Succession is a binary Connector that requires its relatedFeatures to happen separately in time.</rdfs:comment>
    <rdfs:label>Succession</rdfs:label>
  </rdfs:Class>
  <rdfs:Class rdf:about="http://open-services.net/ns/sysmlv2#AssociationStructure">
    <rdfs:subClassOf>
      <rdfs:Class rdf:about="http://open-services.net/ns/sysmlv2#Structure"/>
    </rdfs:subClassOf>
    <rdfs:subClassOf>
      <rdfs:Class rdf:about="http://open-services.net/ns/sysmlv2#Association"/>
    </rdfs:subClassOf>
    <rdfs:isDefinedBy rdf:resource="http://open-services.net/ns/sysmlv2#"/>
    <rdfs:comment>An AssociationStructure is an Association that is also a Structure, classifying link objects that are both links and objects. As objects, link objects can be created and destroyed, and their non-end Features can change over time. However, the values of the end Features of a link object are fixed and cannot change over its lifetime.</rdfs:comment>
    <rdfs:label>AssociationStructure</rdfs:label>
  </rdfs:Class>
  <rdfs:Class rdf:about="http://open-services.net/ns/sysmlv2#Step">
    <rdfs:subClassOf>
      <rdfs:Class rdf:about="http://open-services.net/ns/sysmlv2#Feature"/>
    </rdfs:subClassOf>
    <rdfs:isDefinedBy rdf:resource="http://open-services.net/ns/sysmlv2#"/>
    <rdfs:comment>A Step is a Feature that is typed by one or more Behaviors. Steps may be used by one Behavior to coordinate the performance of other Behaviors, supporting a steady refinement of behavioral descriptions. Steps can be ordered in time and can be connected using ItemFlows to specify things flowing between their parameters.</rdfs:comment>
    <rdfs:label>Step</rdfs:label>
  </rdfs:Class>
  <rdfs:Class rdf:about="http://open-services.net/ns/sysmlv2#ReferenceUsage">
    <rdfs:subClassOf rdf:resource="http://open-services.net/ns/sysmlv2#Usage"/>
    <rdfs:isDefinedBy rdf:resource="http://open-services.net/ns/sysmlv2#"/>
    <rdfs:comment>A ReferenceUsage is a Usage that specifies a non-compositional (isComposite = false) reference to something. The definition of a ReferenceUsage can be any kind of Classifier, with the default being the top-level Classifier Base::Anything from the Kernel Semantic Library. This allows the specification of a generic reference without distinguishing if the thing referenced is an attribute value, item, action, etc.</rdfs:comment>
    <rdfs:label>ReferenceUsage</rdfs:label>
  </rdfs:Class>
  <rdfs:Class rdf:about="http://open-services.net/ns/sysmlv2#Element">
    <rdfs:subClassOf rdf:resource="http://open-services.net/ns/am#Resource"/>
    <rdfs:isDefinedBy rdf:resource="http://open-services.net/ns/sysmlv2#"/>
    <rdfs:comment>An Element is a constituent of a model that is uniquely identified relative to all other Elements. It can have Relationships with other Elements. Some of these Relationships might imply ownership of other Elements, which means that if an Element is deleted from a model, then so are all the Elements that it owns.</rdfs:comment>
    <rdfs:label>Element</rdfs:label>
  </rdfs:Class>
  <rdfs:Class rdf:about="http://open-services.net/ns/sysmlv2#ConcernDefinition">
    <rdfs:subClassOf>
      <rdfs:Class rdf:about="http://open-services.net/ns/sysmlv2#RequirementDefinition"/>
    </rdfs:subClassOf>
    <rdfs:isDefinedBy rdf:resource="http://open-services.net/ns/sysmlv2#"/>
    <rdfs:comment>A ConcernDefinition is a RequirementDefinition that one or more stakeholders may be interested in having addressed. These stakeholders are identified by the ownedStakeholdersof the ConcernDefinition.</rdfs:comment>
    <rdfs:label>ConcernDefinition</rdfs:label>
  </rdfs:Class>
  <rdfs:Class rdf:about="http://open-services.net/ns/sysmlv2#Multiplicity">
    <rdfs:subClassOf>
      <rdfs:Class rdf:about="http://open-services.net/ns/sysmlv2#Feature"/>
    </rdfs:subClassOf>
    <rdfs:isDefinedBy rdf:resource="http://open-services.net/ns/sysmlv2#"/>
    <rdfs:comment>A Multiplicity is a Feature whose co-domain is a set of natural numbers giving the allowed cardinalities of each typeWithMultiplicity. The cardinality of a Type is defined as follows, depending on whether the Type is a Classifier or Feature.
.</rdfs:comment>
    <rdfs:label>Multiplicity</rdfs:label>
  </rdfs:Class>
  <rdfs:Class rdf:about="http://open-services.net/ns/sysmlv2#AnnotatingElement">
    <rdfs:subClassOf rdf:resource="http://open-services.net/ns/sysmlv2#Element"/>
    <rdfs:isDefinedBy rdf:resource="http://open-services.net/ns/sysmlv2#"/>
    <rdfs:comment>An AnnotatingElement is an Element that provides additional description of or metadata on some other Element. An AnnotatingElement is either attached to its annotatedElements by Annotation Relationships, or it implicitly annotates its owningNamespace.</rdfs:comment>
    <rdfs:label>AnnotatingElement</rdfs:label>
  </rdfs:Class>
  <rdfs:Class rdf:about="http://open-services.net/ns/sysmlv2#Feature">
    <rdfs:subClassOf>
      <rdfs:Class rdf:about="http://open-services.net/ns/sysmlv2#Type"/>
    </rdfs:subClassOf>
    <rdfs:isDefinedBy rdf:resource="http://open-services.net/ns/sysmlv2#"/>
    <rdfs:comment>A Feature is a Type that classifies relations between multiple things (in the universe). The domain of the relation is the intersection of the featuringTypes of the Feature. (The domain of a Feature with no featuringTyps is implicitly the most general Type Base::Anything from the Kernel Semantic Library.) The co-domain of the relation is the intersection of the types of the Feature.

.</rdfs:comment>
    <rdfs:label>Feature</rdfs:label>
  </rdfs:Class>
  <rdfs:Class rdf:about="http://open-services.net/ns/sysmlv2#PortConjugation">
    <rdfs:subClassOf>
      <rdfs:Class rdf:about="http://open-services.net/ns/sysmlv2#Conjugation"/>
    </rdfs:subClassOf>
    <rdfs:isDefinedBy rdf:resource="http://open-services.net/ns/sysmlv2#"/>
    <rdfs:comment>A PortConjugation is a Conjugation Relationship between a PortDefinition and its corresponding ConjugatedPortDefinition. As a result of this Relationship, the ConjugatedPortDefinition inherits all the features of the original PortDefinition, but input flows of the original PortDefinition become outputs on the ConjugatedPortDefinition and output flows of the original PortDefinition become inputs on the ConjugatedPortDefinition.</rdfs:comment>
    <rdfs:label>PortConjugation</rdfs:label>
  </rdfs:Class>
  <rdfs:Class rdf:about="http://open-services.net/ns/sysmlv2#MetadataDefinition">
    <rdfs:subClassOf>
      <rdfs:Class rdf:about="http://open-services.net/ns/sysmlv2#Metaclass"/>
    </rdfs:subClassOf>
    <rdfs:subClassOf>
      <rdfs:Class rdf:about="http://open-services.net/ns/sysmlv2#ItemDefinition"/>
    </rdfs:subClassOf>
    <rdfs:isDefinedBy rdf:resource="http://open-services.net/ns/sysmlv2#"/>
    <rdfs:comment>A MetadataDefinition is an ItemDefinition that is also a Metaclass.</rdfs:comment>
    <rdfs:label>MetadataDefinition</rdfs:label>
  </rdfs:Class>
  <rdfs:Class rdf:about="http://open-services.net/ns/sysmlv2#Membership">
    <rdfs:subClassOf>
      <rdfs:Class rdf:about="http://open-services.net/ns/sysmlv2#Relationship"/>
    </rdfs:subClassOf>
    <rdfs:isDefinedBy rdf:resource="http://open-services.net/ns/sysmlv2#"/>
    <rdfs:comment>A Membership is a Relationship between a Namespace and an Element that indicates the Element is a member of (i.e., is contained in) the Namespace. Any memberNames specify how the memberElement is identified in the Namespace and the visibility specifies whether or not the memberElement is publicly visible from outside the Namespace.</rdfs:comment>
    <rdfs:label>Membership</rdfs:label>
  </rdfs:Class>
  <rdfs:Class rdf:about="http://open-services.net/ns/sysmlv2#VerificationCaseDefinition">
    <rdfs:subClassOf>
      <rdfs:Class rdf:about="http://open-services.net/ns/sysmlv2#CaseDefinition"/>
    </rdfs:subClassOf>
    <rdfs:isDefinedBy rdf:resource="http://open-services.net/ns/sysmlv2#"/>
    <rdfs:comment>A VerificationCaseDefinition is a CaseDefinition for the purpose of verification of the subject of the case against its requirements.</rdfs:comment>
    <rdfs:label>VerificationCaseDefinition</rdfs:label>
  </rdfs:Class>
  <rdfs:Class rdf:about="http://open-services.net/ns/sysmlv2#DecisionNode">
    <rdfs:subClassOf>
      <rdfs:Class rdf:about="http://open-services.net/ns/sysmlv2#ControlNode"/>
    </rdfs:subClassOf>
    <rdfs:isDefinedBy rdf:resource="http://open-services.net/ns/sysmlv2#"/>
    <rdfs:comment>A DecisionNode is a ControlNode that makes a selection from its outgoing Successions.</rdfs:comment>
    <rdfs:label>DecisionNode</rdfs:label>
  </rdfs:Class>
  <rdfs:Class rdf:about="http://open-services.net/ns/sysmlv2#PortUsage">
    <rdfs:subClassOf>
      <rdfs:Class rdf:about="http://open-services.net/ns/sysmlv2#OccurrenceUsage"/>
    </rdfs:subClassOf>
    <rdfs:isDefinedBy rdf:resource="http://open-services.net/ns/sysmlv2#"/>
    <rdfs:comment>A PortUsage is a usage of a PortDefinition. A PortUsage itself as well as all its nestedUsages must be referential (non-composite).</rdfs:comment>
    <rdfs:label>PortUsage</rdfs:label>
  </rdfs:Class>
  <rdfs:Class rdf:about="http://open-services.net/ns/sysmlv2#Class">
    <rdfs:subClassOf rdf:resource="http://open-services.net/ns/sysmlv2#Classifier"/>
    <rdfs:isDefinedBy rdf:resource="http://open-services.net/ns/sysmlv2#"/>
    <rdfs:comment>A Class is a Classifier of things (in the universe) that can be distinguished without regard to how they are related to other things (via Features). This means multiple things classified by the same Class can be distinguished, even when they are related other things in exactly the same way.</rdfs:comment>
    <rdfs:label>Class</rdfs:label>
  </rdfs:Class>
  <rdfs:Class rdf:about="http://open-services.net/ns/sysmlv2#FeatureMembership">
    <rdfs:subClassOf>
      <rdfs:Class rdf:about="http://open-services.net/ns/sysmlv2#OwningMembership"/>
    </rdfs:subClassOf>
    <rdfs:subClassOf>
      <rdfs:Class rdf:about="http://open-services.net/ns/sysmlv2#Featuring"/>
    </rdfs:subClassOf>
    <rdfs:isDefinedBy rdf:resource="http://open-services.net/ns/sysmlv2#"/>
    <rdfs:comment>A FeatureMembership is an OwningMembership between a Feature in an owningType that is also a Featuring Relationship between the Feature and the Type, in which the featuringType is the source and the featureOfType is the target. A FeatureMembership is always owned by its owningType, which is the featuringType for the FeatureMembership considered as a Featuring.</rdfs:comment>
    <rdfs:label>FeatureMembership</rdfs:label>
  </rdfs:Class>
  <rdfs:Class rdf:about="http://open-services.net/ns/sysmlv2#IfActionUsage">
    <rdfs:subClassOf rdf:resource="http://open-services.net/ns/sysmlv2#ActionUsage"/>
    <rdfs:isDefinedBy rdf:resource="http://open-services.net/ns/sysmlv2#"/>
    <rdfs:comment>An IfActionUsage is an ActionUsage that specifies that the thenAction ActionUsage should be performed if the result of the ifArgument Expression is true. It may also optionally specify an elseAction ActionUsage that is performed if the result of the ifArgument is false.</rdfs:comment>
    <rdfs:label>IfActionUsage</rdfs:label>
  </rdfs:Class>
  <rdfs:Class rdf:about="http://open-services.net/ns/sysmlv2#AnalysisCaseDefinition">
    <rdfs:subClassOf>
      <rdfs:Class rdf:about="http://open-services.net/ns/sysmlv2#CaseDefinition"/>
    </rdfs:subClassOf>
    <rdfs:isDefinedBy rdf:resource="http://open-services.net/ns/sysmlv2#"/>
    <rdfs:comment>An AnalysisCaseDefinition is a CaseDefinition for the case of carrying out an analysis.</rdfs:comment>
    <rdfs:label>AnalysisCaseDefinition</rdfs:label>
  </rdfs:Class>
  <rdfs:Class rdf:about="http://open-services.net/ns/sysmlv2#PartDefinition">
    <rdfs:subClassOf>
      <rdfs:Class rdf:about="http://open-services.net/ns/sysmlv2#ItemDefinition"/>
    </rdfs:subClassOf>
    <rdfs:isDefinedBy rdf:resource="http://open-services.net/ns/sysmlv2#"/>
    <rdfs:comment>A PartDefinition is an ItemDefinition of a Class of systems or parts of systems. Note that all parts may be considered items for certain purposes, but not all items are parts that can perform actions within a system.</rdfs:comment>
    <rdfs:label>PartDefinition</rdfs:label>
  </rdfs:Class>
  <rdfs:Class rdf:about="http://open-services.net/ns/sysmlv2#ForLoopActionUsage">
    <rdfs:subClassOf>
      <rdfs:Class rdf:about="http://open-services.net/ns/sysmlv2#LoopActionUsage"/>
    </rdfs:subClassOf>
    <rdfs:isDefinedBy rdf:resource="http://open-services.net/ns/sysmlv2#"/>
    <rdfs:comment>A ForLoopActionUsage is a LoopActionUsage that specifies that its bodyAction ActionUsage should be performed once for each value, in order, from the sequence of values obtained as the result of the seqArgument Expression, with the loopVariable set to the value for each iteration.</rdfs:comment>
    <rdfs:label>ForLoopActionUsage</rdfs:label>
  </rdfs:Class>
  <rdfs:Class rdf:about="http://open-services.net/ns/sysmlv2#SuccessionItemFlow">
    <rdfs:subClassOf rdf:resource="http://open-services.net/ns/sysmlv2#Succession"/>
    <rdfs:subClassOf>
      <rdfs:Class rdf:about="http://open-services.net/ns/sysmlv2#ItemFlow"/>
    </rdfs:subClassOf>
    <rdfs:isDefinedBy rdf:resource="http://open-services.net/ns/sysmlv2#"/>
    <rdfs:comment>A SuccessionItemFlow is an ItemFlow that also provides temporal ordering. It classifies Transfers that cannot start until the source Occurrence has completed and that must complete before the target Occurrence can start.</rdfs:comment>
    <rdfs:label>SuccessionItemFlow</rdfs:label>
  </rdfs:Class>
  <rdfs:Class rdf:about="http://open-services.net/ns/sysmlv2#StateDefinition">
    <rdfs:subClassOf>
      <rdfs:Class rdf:about="http://open-services.net/ns/sysmlv2#ActionDefinition"/>
    </rdfs:subClassOf>
    <rdfs:isDefinedBy rdf:resource="http://open-services.net/ns/sysmlv2#"/>
    <rdfs:comment>A StateDefinition is the Definition of the Behavior of a system or part of a system in a certain state condition.</rdfs:comment>
    <rdfs:label>StateDefinition</rdfs:label>
  </rdfs:Class>
  <rdfs:Class rdf:about="http://open-services.net/ns/sysmlv2#Documentation">
    <rdfs:subClassOf>
      <rdfs:Class rdf:about="http://open-services.net/ns/sysmlv2#Comment"/>
    </rdfs:subClassOf>
    <rdfs:isDefinedBy rdf:resource="http://open-services.net/ns/sysmlv2#"/>
    <rdfs:comment>Documentation is a Comment that specifically documents a documentedElement, which must be its owner.</rdfs:comment>
    <rdfs:label>Documentation</rdfs:label>
  </rdfs:Class>
  <rdfs:Class rdf:about="http://open-services.net/ns/sysmlv2#ConstraintDefinition">
    <rdfs:subClassOf>
      <rdfs:Class rdf:about="http://open-services.net/ns/sysmlv2#Predicate"/>
    </rdfs:subClassOf>
    <rdfs:subClassOf>
      <rdfs:Class rdf:about="http://open-services.net/ns/sysmlv2#OccurrenceDefinition"/>
    </rdfs:subClassOf>
    <rdfs:isDefinedBy rdf:resource="http://open-services.net/ns/sysmlv2#"/>
    <rdfs:comment>A ConstraintDefinition is an OccurrenceDefinition that is also a Predicate that defines a constraint that may be asserted to hold on a system or part of a system.</rdfs:comment>
    <rdfs:label>ConstraintDefinition</rdfs:label>
  </rdfs:Class>
  <rdfs:Class rdf:about="http://open-services.net/ns/sysmlv2#EnumerationDefinition">
    <rdfs:subClassOf>
      <rdfs:Class rdf:about="http://open-services.net/ns/sysmlv2#AttributeDefinition"/>
    </rdfs:subClassOf>
    <rdfs:isDefinedBy rdf:resource="http://open-services.net/ns/sysmlv2#"/>
    <rdfs:comment>An EnumerationDefinition is an AttributeDefinition all of whose instances are given by an explicit list of enumeratedValues. This is realized by requiring that the EnumerationDefinition have isVariation = true, with the enumeratedValues being its variants.</rdfs:comment>
    <rdfs:label>EnumerationDefinition</rdfs:label>
  </rdfs:Class>
  <rdfs:Class rdf:about="http://open-services.net/ns/sysmlv2#ItemDefinition">
    <rdfs:subClassOf>
      <rdfs:Class rdf:about="http://open-services.net/ns/sysmlv2#Structure"/>
    </rdfs:subClassOf>
    <rdfs:subClassOf>
      <rdfs:Class rdf:about="http://open-services.net/ns/sysmlv2#OccurrenceDefinition"/>
    </rdfs:subClassOf>
    <rdfs:isDefinedBy rdf:resource="http://open-services.net/ns/sysmlv2#"/>
    <rdfs:comment>An ItemDefinition is an OccurrenceDefinition of the Structure of things that may themselves be systems or parts of systems, but may also be things that are acted on by a system or parts of a system, but which do not necessarily perform actions themselves. This includes items that can be exchanged between parts of a system, such as water or electrical signals.</rdfs:comment>
    <rdfs:label>ItemDefinition</rdfs:label>
  </rdfs:Class>
  <rdfs:Class rdf:about="http://open-services.net/ns/sysmlv2#TransitionFeatureKind">
    <rdfs:isDefinedBy rdf:resource="http://open-services.net/ns/sysmlv2#"/>
    <rdfs:comment>A TransitionActionKind indicates whether the transitionFeature of a TransitionFeatureMembership is a trigger, guard or effect.</rdfs:comment>
    <rdfs:label>TransitionFeatureKind</rdfs:label>
  </rdfs:Class>
  <rdfs:Class rdf:about="http://open-services.net/ns/sysmlv2#ParameterMembership">
    <rdfs:subClassOf rdf:resource="http://open-services.net/ns/sysmlv2#FeatureMembership"/>
    <rdfs:isDefinedBy rdf:resource="http://open-services.net/ns/sysmlv2#"/>
    <rdfs:comment>A ParameterMembership is a FeatureMembership that identifies its memberFeature as a parameter, which is always owned, and must have a direction. A ParameterMembership must be owned by a Behavior or a Step.</rdfs:comment>
    <rdfs:label>ParameterMembership</rdfs:label>
  </rdfs:Class>
  <rdfs:Class rdf:about="http://open-services.net/ns/sysmlv2#Conjugation">
    <rdfs:subClassOf>
      <rdfs:Class rdf:about="http://open-services.net/ns/sysmlv2#Relationship"/>
    </rdfs:subClassOf>
    <rdfs:isDefinedBy rdf:resource="http://open-services.net/ns/sysmlv2#"/>
    <rdfs:comment>Conjugation is a Relationship between two types in which the conjugatedType inherits all the Features of the originalType, but with all input and output Features reversed. That is, any Features with a direction in relative to the originalType are considered to have an effective direction of out relative to the conjugatedType and, similarly, Features with direction out in the originalType are considered to have an effective direction of in in the conjugatedType. Features with direction inout, or with no direction, in the originalType, are inherited without change.</rdfs:comment>
    <rdfs:label>Conjugation</rdfs:label>
  </rdfs:Class>
  <rdfs:Class rdf:about="http://open-services.net/ns/sysmlv2#VisibilityKind">
    <rdfs:isDefinedBy rdf:resource="http://open-services.net/ns/sysmlv2#"/>
    <rdfs:comment>VisibilityKind is an enumeration whose literals specify the visibility of a Membership of an Element in a Namespace outside of that Namespace. Note that "visibility" specifically restricts whether an Element in a Namespace may be referenced by name from outside the Namespace and only otherwise restricts access to an Element as provided by specific constraints in the abstract syntax (e.g., preventing the import or inheritance of private Elements).</rdfs:comment>
    <rdfs:label>VisibilityKind</rdfs:label>
  </rdfs:Class>
  <rdfs:Class rdf:about="http://open-services.net/ns/sysmlv2#MetadataUsage">
    <rdfs:subClassOf rdf:resource="http://open-services.net/ns/sysmlv2#MetadataFeature"/>
    <rdfs:subClassOf>
      <rdfs:Class rdf:about="http://open-services.net/ns/sysmlv2#ItemUsage"/>
    </rdfs:subClassOf>
    <rdfs:isDefinedBy rdf:resource="http://open-services.net/ns/sysmlv2#"/>
    <rdfs:comment>A  MetadataUsage is a Usage and a MetadataFeature, used to annotate other Elements in a system model with metadata. As a MetadataFeature, its type must be a Metaclass, which will nominally be a MetadataDefinition. However, any kernel Metaclass is also allowed, to permit use of Metaclasses from the Kernel Model Libraries.</rdfs:comment>
    <rdfs:label>MetadataUsage</rdfs:label>
  </rdfs:Class>
  <rdfs:Class rdf:about="http://open-services.net/ns/sysmlv2#BooleanExpression">
    <rdfs:subClassOf>
      <rdfs:Class rdf:about="http://open-services.net/ns/sysmlv2#Expression"/>
    </rdfs:subClassOf>
    <rdfs:isDefinedBy rdf:resource="http://open-services.net/ns/sysmlv2#"/>
    <rdfs:comment>A BooleanExpression is a Boolean-valued Expression whose type is a Predicate. It represents a logical condition resulting from the evaluation of the Predicate.</rdfs:comment>
    <rdfs:label>BooleanExpression</rdfs:label>
  </rdfs:Class>
  <rdfs:Class rdf:about="http://open-services.net/ns/sysmlv2#NullExpression">
    <rdfs:subClassOf>
      <rdfs:Class rdf:about="http://open-services.net/ns/sysmlv2#Expression"/>
    </rdfs:subClassOf>
    <rdfs:isDefinedBy rdf:resource="http://open-services.net/ns/sysmlv2#"/>
    <rdfs:comment>A NullExpression is an Expression that results in a null value.</rdfs:comment>
    <rdfs:label>NullExpression</rdfs:label>
  </rdfs:Class>
  <rdfs:Class rdf:about="http://open-services.net/ns/sysmlv2#ConnectionUsage">
    <rdfs:subClassOf>
      <rdfs:Class rdf:about="http://open-services.net/ns/sysmlv2#PartUsage"/>
    </rdfs:subClassOf>
    <rdfs:subClassOf>
      <rdfs:Class rdf:about="http://open-services.net/ns/sysmlv2#ConnectorAsUsage"/>
    </rdfs:subClassOf>
    <rdfs:isDefinedBy rdf:resource="http://open-services.net/ns/sysmlv2#"/>
    <rdfs:comment>A ConnectionUsage is a ConnectorAsUsage that is also a PartUsage. Nominally, if its type is a ConnectionDefinition, then a ConnectionUsage is a Usage of that ConnectionDefinition, representing a connection between parts of a system. However, other kinds of kernel AssociationStructures are also allowed, to permit use of AssociationStructures from the Kernel Model Libraries.</rdfs:comment>
    <rdfs:label>ConnectionUsage</rdfs:label>
  </rdfs:Class>
  <rdfs:Class rdf:about="http://open-services.net/ns/sysmlv2#StateSubactionKind">
    <rdfs:isDefinedBy rdf:resource="http://open-services.net/ns/sysmlv2#"/>
    <rdfs:comment>A StateSubactionKind indicates whether the action of a StateSubactionMembership is an entry, do or exit action.</rdfs:comment>
    <rdfs:label>StateSubactionKind</rdfs:label>
  </rdfs:Class>
  <rdfs:Class rdf:about="http://open-services.net/ns/sysmlv2#FeatureInverting">
    <rdfs:subClassOf>
      <rdfs:Class rdf:about="http://open-services.net/ns/sysmlv2#Relationship"/>
    </rdfs:subClassOf>
    <rdfs:isDefinedBy rdf:resource="http://open-services.net/ns/sysmlv2#"/>
    <rdfs:comment>A FeatureInverting is a Relationship between Features asserting that their interpretations (sequences) are the reverse of each other, identified as featureInverted and invertingFeature. For example, a Feature identifying each person's parents is the inverse of a Feature identifying each person's children. A person identified as a parent of another will identify that other as one of their children.</rdfs:comment>
    <rdfs:label>FeatureInverting</rdfs:label>
  </rdfs:Class>
  <rdfs:Class rdf:about="http://open-services.net/ns/sysmlv2#PortDefinition">
    <rdfs:subClassOf>
      <rdfs:Class rdf:about="http://open-services.net/ns/sysmlv2#Structure"/>
    </rdfs:subClassOf>
    <rdfs:subClassOf>
      <rdfs:Class rdf:about="http://open-services.net/ns/sysmlv2#OccurrenceDefinition"/>
    </rdfs:subClassOf>
    <rdfs:isDefinedBy rdf:resource="http://open-services.net/ns/sysmlv2#"/>
    <rdfs:comment>A PortDefinition defines a point at which external entities can connect to and interact with a system or part of a system. Any ownedUsages of a PortDefinition, other than PortUsages, must not be composite.</rdfs:comment>
    <rdfs:label>PortDefinition</rdfs:label>
  </rdfs:Class>
  <rdfs:Class rdf:about="http://open-services.net/ns/sysmlv2#Featuring">
    <rdfs:subClassOf>
      <rdfs:Class rdf:about="http://open-services.net/ns/sysmlv2#Relationship"/>
    </rdfs:subClassOf>
    <rdfs:isDefinedBy rdf:resource="http://open-services.net/ns/sysmlv2#"/>
    <rdfs:comment>Featuring is a Relationship between a Type and a Feature that is featured by that Type. It asserts that every instance in the domain of the feature must be classified by the type.</rdfs:comment>
    <rdfs:label>Featuring</rdfs:label>
  </rdfs:Class>
  <rdfs:Class rdf:about="http://open-services.net/ns/sysmlv2#Structure">
    <rdfs:subClassOf rdf:resource="http://open-services.net/ns/sysmlv2#Class"/>
    <rdfs:isDefinedBy rdf:resource="http://open-services.net/ns/sysmlv2#"/>
    <rdfs:comment>A Structure is a Class of objects in the modeled universe that are primarily structural in nature. While such an object is not itself behavioral, it may be involved in and acted on by Behaviors, and it may be the performer of some of them.</rdfs:comment>
    <rdfs:label>Structure</rdfs:label>
  </rdfs:Class>
  <rdfs:Class rdf:about="http://open-services.net/ns/sysmlv2#BindingConnectorAsUsage">
    <rdfs:subClassOf>
      <rdfs:Class rdf:about="http://open-services.net/ns/sysmlv2#ConnectorAsUsage"/>
    </rdfs:subClassOf>
    <rdfs:subClassOf rdf:resource="http://open-services.net/ns/sysmlv2#BindingConnector"/>
    <rdfs:isDefinedBy rdf:resource="http://open-services.net/ns/sysmlv2#"/>
    <rdfs:comment>A BindingConnectorAsUsage is both a BindingConnector and a ConnectorAsUsage.</rdfs:comment>
    <rdfs:label>BindingConnectorAsUsage</rdfs:label>
  </rdfs:Class>
  <rdfs:Class rdf:about="http://open-services.net/ns/sysmlv2#ItemUsage">
    <rdfs:subClassOf>
      <rdfs:Class rdf:about="http://open-services.net/ns/sysmlv2#OccurrenceUsage"/>
    </rdfs:subClassOf>
    <rdfs:isDefinedBy rdf:resource="http://open-services.net/ns/sysmlv2#"/>
    <rdfs:comment>An ItemUsage is a ItemUsage whose definition is a Structure. Nominally, if the definition is an ItemDefinition, an ItemUsage is a ItemUsage of that ItemDefinition within a system. However, other kinds of Kernel Structures are also allowed, to permit use of Structures from the Kernel Model Libraries.</rdfs:comment>
    <rdfs:label>ItemUsage</rdfs:label>
  </rdfs:Class>
  <rdfs:Class rdf:about="http://open-services.net/ns/sysmlv2#Annotation">
    <rdfs:subClassOf>
      <rdfs:Class rdf:about="http://open-services.net/ns/sysmlv2#Relationship"/>
    </rdfs:subClassOf>
    <rdfs:isDefinedBy rdf:resource="http://open-services.net/ns/sysmlv2#"/>
    <rdfs:comment>An Annotation is a Relationship between an AnnotatingElement and the Element that is annotated by that AnnotatingElement.</rdfs:comment>
    <rdfs:label>Annotation</rdfs:label>
  </rdfs:Class>
  <rdfs:Class rdf:about="http://open-services.net/ns/sysmlv2#OwningMembership">
    <rdfs:subClassOf rdf:resource="http://open-services.net/ns/sysmlv2#Membership"/>
    <rdfs:isDefinedBy rdf:resource="http://open-services.net/ns/sysmlv2#"/>
    <rdfs:comment>An OwningMembership is a Membership that owns its memberElement as a ownedRelatedElement. The ownedMemberElement becomes an ownedMember of the membershipOwningNamespace.</rdfs:comment>
    <rdfs:label>OwningMembership</rdfs:label>
  </rdfs:Class>
  <rdfs:Class rdf:about="http://open-services.net/ns/sysmlv2#UseCaseUsage">
    <rdfs:subClassOf>
      <rdfs:Class rdf:about="http://open-services.net/ns/sysmlv2#CaseUsage"/>
    </rdfs:subClassOf>
    <rdfs:isDefinedBy rdf:resource="http://open-services.net/ns/sysmlv2#"/>
    <rdfs:comment>A UseCaseUsage is a Usage of a UseCaseDefinition.</rdfs:comment>
    <rdfs:label>UseCaseUsage</rdfs:label>
  </rdfs:Class>
  <rdfs:Class rdf:about="http://open-services.net/ns/sysmlv2#NamespaceImport">
    <rdfs:subClassOf>
      <rdfs:Class rdf:about="http://open-services.net/ns/sysmlv2#Import"/>
    </rdfs:subClassOf>
    <rdfs:isDefinedBy rdf:resource="http://open-services.net/ns/sysmlv2#"/>
    <rdfs:comment>A NamespaceImport is an Import that imports Memberships from its importedNamespace into the importOwningNamespace. If  isRecursive = false, then only the visible Memberships of the importedNamespace are imported. If  isRecursive = true, then, in addition, Memberships are recursively imported from any ownedMembers of the importedNamespace that are Namespaces.</rdfs:comment>
    <rdfs:label>NamespaceImport</rdfs:label>
  </rdfs:Class>
  <rdfs:Class rdf:about="http://open-services.net/ns/sysmlv2#RenderingUsage">
    <rdfs:subClassOf>
      <rdfs:Class rdf:about="http://open-services.net/ns/sysmlv2#PartUsage"/>
    </rdfs:subClassOf>
    <rdfs:isDefinedBy rdf:resource="http://open-services.net/ns/sysmlv2#"/>
    <rdfs:comment>A RenderingUsage is the usage of a RenderingDefinition to specify the rendering of a specific model view to produce a physical view artifact.</rdfs:comment>
    <rdfs:label>RenderingUsage</rdfs:label>
  </rdfs:Class>
  <rdfs:Class rdf:about="http://open-services.net/ns/sysmlv2#TriggerKind">
    <rdfs:isDefinedBy rdf:resource="http://open-services.net/ns/sysmlv2#"/>
    <rdfs:comment>TriggerKind enumerates the kinds of triggers that can be represented by a TriggerInvocationExpression.</rdfs:comment>
    <rdfs:label>TriggerKind</rdfs:label>
  </rdfs:Class>
  <rdfs:Class rdf:about="http://open-services.net/ns/sysmlv2#TransitionFeatureMembership">
    <rdfs:subClassOf rdf:resource="http://open-services.net/ns/sysmlv2#FeatureMembership"/>
    <rdfs:isDefinedBy rdf:resource="http://open-services.net/ns/sysmlv2#"/>
    <rdfs:comment>A TransitionFeatureMembership is a FeatureMembership for a trigger, guard or effect of a TransitionUsage, whose transitionFeature is a AcceptActionUsage, Boolean-valued Expression or ActionUsage, depending on its kind. .</rdfs:comment>
    <rdfs:label>TransitionFeatureMembership</rdfs:label>
  </rdfs:Class>
  <rdfs:Class rdf:about="http://open-services.net/ns/sysmlv2#SatisfyRequirementUsage">
    <rdfs:subClassOf>
      <rdfs:Class rdf:about="http://open-services.net/ns/sysmlv2#RequirementUsage"/>
    </rdfs:subClassOf>
    <rdfs:subClassOf rdf:resource="http://open-services.net/ns/sysmlv2#AssertConstraintUsage"/>
    <rdfs:isDefinedBy rdf:resource="http://open-services.net/ns/sysmlv2#"/>
    <rdfs:comment>A SatisfyRequirementUsage is an AssertConstraintUsage that asserts, by default, that a satisfied RequirementUsage is true for a specific satisfyingFeature, or, if isNegated = true, that the RequirementUsage is false. The satisfied RequirementUsage is related to the SatisfyRequirementUsage by a ReferenceSubsetting Relationship.</rdfs:comment>
    <rdfs:label>SatisfyRequirementUsage</rdfs:label>
  </rdfs:Class>
  <rdfs:Class rdf:about="http://open-services.net/ns/sysmlv2#RequirementUsage">
    <rdfs:subClassOf>
      <rdfs:Class rdf:about="http://open-services.net/ns/sysmlv2#ConstraintUsage"/>
    </rdfs:subClassOf>
    <rdfs:isDefinedBy rdf:resource="http://open-services.net/ns/sysmlv2#"/>
    <rdfs:comment>A RequirementUsage is a Usage of a RequirementDefinition.</rdfs:comment>
    <rdfs:label>RequirementUsage</rdfs:label>
  </rdfs:Class>
  <rdfs:Class rdf:about="http://open-services.net/ns/sysmlv2#TriggerInvocationExpression">
    <rdfs:subClassOf>
      <rdfs:Class rdf:about="http://open-services.net/ns/sysmlv2#InvocationExpression"/>
    </rdfs:subClassOf>
    <rdfs:isDefinedBy rdf:resource="http://open-services.net/ns/sysmlv2#"/>
    <rdfs:comment>A TriggerInvocationExpression is an InvocationExpression that invokes one of the trigger Functions from the Kernel Semantic Library Triggers package, as indicated by its kind.</rdfs:comment>
    <rdfs:label>TriggerInvocationExpression</rdfs:label>
  </rdfs:Class>
  <rdfs:Class rdf:about="http://open-services.net/ns/sysmlv2#ItemFlow">
    <rdfs:subClassOf rdf:resource="http://open-services.net/ns/sysmlv2#Step"/>
    <rdfs:subClassOf>
      <rdfs:Class rdf:about="http://open-services.net/ns/sysmlv2#Connector"/>
    </rdfs:subClassOf>
    <rdfs:isDefinedBy rdf:resource="http://open-services.net/ns/sysmlv2#"/>
    <rdfs:comment>An ItemFlow is a Step that represents the transfer of objects or data values from one Feature to another. ItemFlows can take non-zero time to complete.</rdfs:comment>
    <rdfs:label>ItemFlow</rdfs:label>
  </rdfs:Class>
  <rdfs:Class rdf:about="http://open-services.net/ns/sysmlv2#ViewRenderingMembership">
    <rdfs:subClassOf rdf:resource="http://open-services.net/ns/sysmlv2#FeatureMembership"/>
    <rdfs:isDefinedBy rdf:resource="http://open-services.net/ns/sysmlv2#"/>
    <rdfs:comment>A ViewRenderingMembership is a FeatureMembership that identifies the viewRendering of a ViewDefinition or ViewUsage.</rdfs:comment>
    <rdfs:label>ViewRenderingMembership</rdfs:label>
  </rdfs:Class>
  <rdfs:Class rdf:about="http://open-services.net/ns/sysmlv2#ConcernUsage">
    <rdfs:subClassOf rdf:resource="http://open-services.net/ns/sysmlv2#RequirementUsage"/>
    <rdfs:isDefinedBy rdf:resource="http://open-services.net/ns/sysmlv2#"/>
    <rdfs:comment>A ConcernUsage is a Usage of a ConcernDefinition.</rdfs:comment>
    <rdfs:label>ConcernUsage</rdfs:label>
  </rdfs:Class>
  <rdfs:Class rdf:about="http://open-services.net/ns/sysmlv2#DataType">
    <rdfs:subClassOf rdf:resource="http://open-services.net/ns/sysmlv2#Classifier"/>
    <rdfs:isDefinedBy rdf:resource="http://open-services.net/ns/sysmlv2#"/>
    <rdfs:comment>A DataType is a Classifier of things (in the universe) that can only be distinguished by how they are related to other things (via Features). This means multiple things classified by the same DataType.</rdfs:comment>
    <rdfs:label>DataType</rdfs:label>
  </rdfs:Class>
  <rdfs:Class rdf:about="http://open-services.net/ns/sysmlv2#InterfaceDefinition">
    <rdfs:subClassOf>
      <rdfs:Class rdf:about="http://open-services.net/ns/sysmlv2#ConnectionDefinition"/>
    </rdfs:subClassOf>
    <rdfs:isDefinedBy rdf:resource="http://open-services.net/ns/sysmlv2#"/>
    <rdfs:comment>An InterfaceDefinition is a ConnectionDefinition all of whose ends are PortUsages, defining an interface between elements that interact through such ports.</rdfs:comment>
    <rdfs:label>InterfaceDefinition</rdfs:label>
  </rdfs:Class>
  <rdfs:Class rdf:about="http://open-services.net/ns/sysmlv2#AttributeUsage">
    <rdfs:subClassOf rdf:resource="http://open-services.net/ns/sysmlv2#Usage"/>
    <rdfs:isDefinedBy rdf:resource="http://open-services.net/ns/sysmlv2#"/>
    <rdfs:comment>An AttributeUsage is a Usage whose type is a DataType. Nominally, if the type is an AttributeDefinition, an AttributeUsage is a usage of a AttributeDefinition to represent the value of some system quality or characteristic. However, other kinds of kernel DataTypes are also allowed, to permit use of DataTypes from the Kernel Model Libraries. An AttributeUsage itself as well as all its nested features must be referential (non-composite).</rdfs:comment>
    <rdfs:label>AttributeUsage</rdfs:label>
  </rdfs:Class>
  <rdfs:Class rdf:about="http://open-services.net/ns/sysmlv2#ItemFlowEnd">
    <rdfs:subClassOf rdf:resource="http://open-services.net/ns/sysmlv2#Feature"/>
    <rdfs:isDefinedBy rdf:resource="http://open-services.net/ns/sysmlv2#"/>
    <rdfs:comment>An ItemFlowEnd is a Feature that is one of the connectorEnds giving the source or target of an ItemFlow. For ItemFlows typed by FlowTransfer or its specializations, ItemFlowEnds must have exactly one ownedFeature, which redefines Transfer::source::sourceOutput or Transfer::target::targetInput and redefines the corresponding feature of the relatedElement for its end.</rdfs:comment>
    <rdfs:label>ItemFlowEnd</rdfs:label>
  </rdfs:Class>
  <rdfs:Class rdf:about="http://open-services.net/ns/sysmlv2#ObjectiveMembership">
    <rdfs:subClassOf rdf:resource="http://open-services.net/ns/sysmlv2#FeatureMembership"/>
    <rdfs:isDefinedBy rdf:resource="http://open-services.net/ns/sysmlv2#"/>
    <rdfs:comment>An ObjectiveMembership is a FeatureMembership that indicates that its ownedObjectiveRequirement is the objective RequirementUsage for its owningType, which must be a CaseDefinition or CaseUsage.</rdfs:comment>
    <rdfs:label>ObjectiveMembership</rdfs:label>
  </rdfs:Class>
  <rdfs:Class rdf:about="http://open-services.net/ns/sysmlv2#WhileLoopActionUsage">
    <rdfs:subClassOf>
      <rdfs:Class rdf:about="http://open-services.net/ns/sysmlv2#LoopActionUsage"/>
    </rdfs:subClassOf>
    <rdfs:isDefinedBy rdf:resource="http://open-services.net/ns/sysmlv2#"/>
    <rdfs:comment>A WhileLoopActionUsage is a LoopActionUsage that specifies that the bodyAction ActionUsage should be performed repeatedly while the result of the whileArgument Expression is true or until the result of the untilArgument Expression (if provided) is true. The whileArgument Expression is evaluated before each (possible) performance of the bodyAction, and the untilArgument Expression is evaluated after each performance of the bodyAction.</rdfs:comment>
    <rdfs:label>WhileLoopActionUsage</rdfs:label>
  </rdfs:Class>
  <rdfs:Class rdf:about="http://open-services.net/ns/sysmlv2#ReferenceSubsetting">
    <rdfs:subClassOf>
      <rdfs:Class rdf:about="http://open-services.net/ns/sysmlv2#Subsetting"/>
    </rdfs:subClassOf>
    <rdfs:isDefinedBy rdf:resource="http://open-services.net/ns/sysmlv2#"/>
    <rdfs:comment>ReferenceSubsetting is a kind of Subsetting in which the referencedFeature is syntactically distinguished from other Features subsetted by the referencingFeature. ReferenceSubsetting has the same semantics as Subsetting, but the referenceFeature may have a special purpose relative to the referencingFeature. For instance, ReferenceSubsetting is used to identify the relatedFeatures of a Connector.</rdfs:comment>
    <rdfs:label>ReferenceSubsetting</rdfs:label>
  </rdfs:Class>
  <rdfs:Class rdf:about="http://open-services.net/ns/sysmlv2#Differencing">
    <rdfs:subClassOf>
      <rdfs:Class rdf:about="http://open-services.net/ns/sysmlv2#Relationship"/>
    </rdfs:subClassOf>
    <rdfs:isDefinedBy rdf:resource="http://open-services.net/ns/sysmlv2#"/>
    <rdfs:comment>Differencing is a Relationship that makes its differencingType one of the differencingTypes of its typeDifferenced.</rdfs:comment>
    <rdfs:label>Differencing</rdfs:label>
  </rdfs:Class>
  <rdfs:Class rdf:about="http://open-services.net/ns/sysmlv2#NamespaceExpose">
    <rdfs:subClassOf rdf:resource="http://open-services.net/ns/sysmlv2#NamespaceImport"/>
    <rdfs:subClassOf>
      <rdfs:Class rdf:about="http://open-services.net/ns/sysmlv2#Expose"/>
    </rdfs:subClassOf>
    <rdfs:isDefinedBy rdf:resource="http://open-services.net/ns/sysmlv2#"/>
    <rdfs:comment>A NamespaceExpose is an Expose Relationship that exposes the Memberships of a specific importedNamespace and, if isRecursive = true, additional Memberships recursively.</rdfs:comment>
    <rdfs:label>NamespaceExpose</rdfs:label>
  </rdfs:Class>
  <rdfs:Class rdf:about="http://open-services.net/ns/sysmlv2#Connector">
    <rdfs:subClassOf>
      <rdfs:Class rdf:about="http://open-services.net/ns/sysmlv2#Relationship"/>
    </rdfs:subClassOf>
    <rdfs:subClassOf rdf:resource="http://open-services.net/ns/sysmlv2#Feature"/>
    <rdfs:isDefinedBy rdf:resource="http://open-services.net/ns/sysmlv2#"/>
    <rdfs:comment>A Connector is a usage of Associations, with links restricted according to instances of the Type in which they are used (domain of the Connector). The associations of the Connector restrict what kinds of things might be linked. The Connector further restricts these links to be between values of Features on instances of its domain.</rdfs:comment>
    <rdfs:label>Connector</rdfs:label>
  </rdfs:Class>
  <rdfs:Class rdf:about="http://open-services.net/ns/sysmlv2#PerformActionUsage">
    <rdfs:subClassOf>
      <rdfs:Class rdf:about="http://open-services.net/ns/sysmlv2#EventOccurrenceUsage"/>
    </rdfs:subClassOf>
    <rdfs:subClassOf rdf:resource="http://open-services.net/ns/sysmlv2#ActionUsage"/>
    <rdfs:isDefinedBy rdf:resource="http://open-services.net/ns/sysmlv2#"/>
    <rdfs:comment>A PerformActionUsage is an ActionUsage that represents the performance of an ActionUsage. Unless it is the PerformActionUsage itself, the ActionUsage to be performed is related to the PerformActionUsage by a ReferenceSubsetting relationship. A PerformActionUsage is also an EventOccurrenceUsage, with its performedAction as the eventOccurrence.</rdfs:comment>
    <rdfs:label>PerformActionUsage</rdfs:label>
  </rdfs:Class>
  <rdfs:Class rdf:about="http://open-services.net/ns/sysmlv2#StakeholderMembership">
    <rdfs:subClassOf rdf:resource="http://open-services.net/ns/sysmlv2#ParameterMembership"/>
    <rdfs:isDefinedBy rdf:resource="http://open-services.net/ns/sysmlv2#"/>
    <rdfs:comment>A StakeholderMembership is a ParameterMembership that identifies a PartUsage as a stakeholderParameter of a RequirementDefinition or RequirementUsage, which specifies a role played by an entity with concerns framed by the owningType.</rdfs:comment>
    <rdfs:label>StakeholderMembership</rdfs:label>
  </rdfs:Class>
  <rdfs:Class rdf:about="http://open-services.net/ns/sysmlv2#AcceptActionUsage">
    <rdfs:subClassOf rdf:resource="http://open-services.net/ns/sysmlv2#ActionUsage"/>
    <rdfs:isDefinedBy rdf:resource="http://open-services.net/ns/sysmlv2#"/>
    <rdfs:comment>An AcceptActionUsage is an ActionUsage that specifies the acceptance of an incomingTransfer from the Occurrence given by the result of its receiverArgument Expression. (If no receiverArgument is provided, the default is the this context of the AcceptActionUsage.) The payload of the accepted Transfer is output on its payloadParameter. Which Transfers may be accepted is determined by conformance to the typing and (potentially) binding of the payloadParameter.</rdfs:comment>
    <rdfs:label>AcceptActionUsage</rdfs:label>
  </rdfs:Class>
  <rdfs:Class rdf:about="http://open-services.net/ns/sysmlv2#SelectExpression">
    <rdfs:subClassOf>
      <rdfs:Class rdf:about="http://open-services.net/ns/sysmlv2#OperatorExpression"/>
    </rdfs:subClassOf>
    <rdfs:isDefinedBy rdf:resource="http://open-services.net/ns/sysmlv2#"/>
    <rdfs:comment>A SelectExpression is an OperatorExpression whose operator is "select", which resolves to the Function ControlFunctions::select from the Kernel Functions Library.</rdfs:comment>
    <rdfs:label>SelectExpression</rdfs:label>
  </rdfs:Class>
  <rdfs:Class rdf:about="http://open-services.net/ns/sysmlv2#JoinNode">
    <rdfs:subClassOf>
      <rdfs:Class rdf:about="http://open-services.net/ns/sysmlv2#ControlNode"/>
    </rdfs:subClassOf>
    <rdfs:isDefinedBy rdf:resource="http://open-services.net/ns/sysmlv2#"/>
    <rdfs:comment>A JoinNode is a ControlNode that waits for the completion of all the predecessor Actions given by incoming Successions.</rdfs:comment>
    <rdfs:label>JoinNode</rdfs:label>
  </rdfs:Class>
  <rdfs:Class rdf:about="http://open-services.net/ns/sysmlv2#LiteralInteger">
    <rdfs:subClassOf>
      <rdfs:Class rdf:about="http://open-services.net/ns/sysmlv2#LiteralExpression"/>
    </rdfs:subClassOf>
    <rdfs:isDefinedBy rdf:resource="http://open-services.net/ns/sysmlv2#"/>
    <rdfs:comment>A LiteralInteger is a LiteralExpression that provides an Integer value as a result. Its result parameter must have the type Integer.</rdfs:comment>
    <rdfs:label>LiteralInteger</rdfs:label>
  </rdfs:Class>
  <rdfs:Class rdf:about="http://open-services.net/ns/sysmlv2#LiteralString">
    <rdfs:subClassOf>
      <rdfs:Class rdf:about="http://open-services.net/ns/sysmlv2#LiteralExpression"/>
    </rdfs:subClassOf>
    <rdfs:isDefinedBy rdf:resource="http://open-services.net/ns/sysmlv2#"/>
    <rdfs:comment>A LiteralString is a LiteralExpression that provides a String value as a result. Its result parameter must have the type String.</rdfs:comment>
    <rdfs:label>LiteralString</rdfs:label>
  </rdfs:Class>
  <rdfs:Class rdf:about="http://open-services.net/ns/sysmlv2#Comment">
    <rdfs:subClassOf rdf:resource="http://open-services.net/ns/sysmlv2#AnnotatingElement"/>
    <rdfs:isDefinedBy rdf:resource="http://open-services.net/ns/sysmlv2#"/>
    <rdfs:comment>A Comment is an AnnotatingElement whose body in some way describes its annotatedElements.</rdfs:comment>
    <rdfs:label>Comment</rdfs:label>
  </rdfs:Class>
  <rdfs:Class rdf:about="http://open-services.net/ns/sysmlv2#TransitionUsage">
    <rdfs:subClassOf rdf:resource="http://open-services.net/ns/sysmlv2#ActionUsage"/>
    <rdfs:isDefinedBy rdf:resource="http://open-services.net/ns/sysmlv2#"/>
    <rdfs:comment>A TransitionUsage is an ActionUsage representing a triggered transition between ActionUsages or StateUsages. When triggered by a triggerAction, when its guardExpression is true, the TransitionUsage asserts that its source is exited, then its effectAction (if any) is performed, and then its target is entered.</rdfs:comment>
    <rdfs:label>TransitionUsage</rdfs:label>
  </rdfs:Class>
  <rdfs:Class rdf:about="http://open-services.net/ns/sysmlv2#CaseDefinition">
    <rdfs:subClassOf rdf:resource="http://open-services.net/ns/sysmlv2#CalculationDefinition"/>
    <rdfs:isDefinedBy rdf:resource="http://open-services.net/ns/sysmlv2#"/>
    <rdfs:comment>A CaseDefinition is a CalculationDefinition for a process, often involving collecting evidence or data, relative to a subject, possibly involving the collaboration of one or more other actors, producing a result that meets an objective.</rdfs:comment>
    <rdfs:label>CaseDefinition</rdfs:label>
  </rdfs:Class>
  <rdfs:Class rdf:about="http://open-services.net/ns/sysmlv2#ConjugatedPortDefinition">
    <rdfs:subClassOf rdf:resource="http://open-services.net/ns/sysmlv2#PortDefinition"/>
    <rdfs:isDefinedBy rdf:resource="http://open-services.net/ns/sysmlv2#"/>
    <rdfs:comment>A ConjugatedPortDefinition is a PortDefinition that is a PortDefinition of its original PortDefinition. That is, a ConjugatedPortDefinition inherits all the features of the original PortDefinition, but input flows of the original PortDefinition become outputs on the ConjugatedPortDefinition and output flows of the original PortDefinition become inputs on the ConjugatedPortDefinition. Every PortDefinition (that is not itself a ConjugatedPortDefinition) has exactly one corresponding ConjugatedPortDefinition, whose effective name is the name of the originalPortDefinition, with the character ~ prepended.</rdfs:comment>
    <rdfs:label>ConjugatedPortDefinition</rdfs:label>
  </rdfs:Class>
  <rdfs:Class rdf:about="http://open-services.net/ns/sysmlv2#TextualRepresentation">
    <rdfs:subClassOf rdf:resource="http://open-services.net/ns/sysmlv2#AnnotatingElement"/>
    <rdfs:isDefinedBy rdf:resource="http://open-services.net/ns/sysmlv2#"/>
    <rdfs:comment>A TextualRepresentation is an AnnotatingElement whose body represents the representedElement in a given language. The representedElement must be the owner of the TextualRepresentation. The named language can be a natural language, in which case the body is an informal representation, or an artificial language, in which case the body is expected to be a formal, machine-parsable representation.</rdfs:comment>
    <rdfs:label>TextualRepresentation</rdfs:label>
  </rdfs:Class>
  <rdfs:Class rdf:about="http://open-services.net/ns/sysmlv2#FeatureChaining">
    <rdfs:subClassOf>
      <rdfs:Class rdf:about="http://open-services.net/ns/sysmlv2#Relationship"/>
    </rdfs:subClassOf>
    <rdfs:isDefinedBy rdf:resource="http://open-services.net/ns/sysmlv2#"/>
    <rdfs:comment>FeatureChaining is a Relationship that makes its target Feature one of the chainingFeatures of its owning Feature.</rdfs:comment>
    <rdfs:label>FeatureChaining</rdfs:label>
  </rdfs:Class>
  <rdfs:Class rdf:about="http://open-services.net/ns/sysmlv2#RequirementConstraintKind">
    <rdfs:isDefinedBy rdf:resource="http://open-services.net/ns/sysmlv2#"/>
    <rdfs:comment>A RequirementConstraintKind indicates whether a ConstraintUsage is an assumption or a requirement in a RequirementDefinition or RequirementUsage.</rdfs:comment>
    <rdfs:label>RequirementConstraintKind</rdfs:label>
  </rdfs:Class>
  <rdfs:Class rdf:about="http://open-services.net/ns/sysmlv2#OperatorExpression">
    <rdfs:subClassOf>
      <rdfs:Class rdf:about="http://open-services.net/ns/sysmlv2#InvocationExpression"/>
    </rdfs:subClassOf>
    <rdfs:isDefinedBy rdf:resource="http://open-services.net/ns/sysmlv2#"/>
    <rdfs:comment>An OperatorExpression is an InvocationExpression whose function is determined by resolving its operator in the context of one of the standard packages from the Kernel Function Library.</rdfs:comment>
    <rdfs:label>OperatorExpression</rdfs:label>
  </rdfs:Class>
  <rdfs:Class rdf:about="http://open-services.net/ns/sysmlv2#StateSubactionMembership">
    <rdfs:subClassOf rdf:resource="http://open-services.net/ns/sysmlv2#FeatureMembership"/>
    <rdfs:isDefinedBy rdf:resource="http://open-services.net/ns/sysmlv2#"/>
    <rdfs:comment>A StateSubactionMembership is a FeatureMembership for an entry, do or exit ActionUsage of a StateDefinition or StateUsage.</rdfs:comment>
    <rdfs:label>StateSubactionMembership</rdfs:label>
  </rdfs:Class>
  <rdfs:Class rdf:about="http://open-services.net/ns/sysmlv2#InterfaceUsage">
    <rdfs:subClassOf rdf:resource="http://open-services.net/ns/sysmlv2#ConnectionUsage"/>
    <rdfs:isDefinedBy rdf:resource="http://open-services.net/ns/sysmlv2#"/>
    <rdfs:comment>An InterfaceUsage is a Usage of an InterfaceDefinition to represent an interface connecting parts of a system through specific ports.</rdfs:comment>
    <rdfs:label>InterfaceUsage</rdfs:label>
  </rdfs:Class>
  <rdfs:Class rdf:about="http://open-services.net/ns/sysmlv2#CaseUsage">
    <rdfs:subClassOf rdf:resource="http://open-services.net/ns/sysmlv2#CalculationUsage"/>
    <rdfs:isDefinedBy rdf:resource="http://open-services.net/ns/sysmlv2#"/>
    <rdfs:comment>A CaseUsage is a Usage of a CaseDefinition.</rdfs:comment>
    <rdfs:label>CaseUsage</rdfs:label>
  </rdfs:Class>
  <rdfs:Class rdf:about="http://open-services.net/ns/sysmlv2#LiteralExpression">
    <rdfs:subClassOf>
      <rdfs:Class rdf:about="http://open-services.net/ns/sysmlv2#Expression"/>
    </rdfs:subClassOf>
    <rdfs:isDefinedBy rdf:resource="http://open-services.net/ns/sysmlv2#"/>
    <rdfs:comment>A LiteralExpression is an Expression that provides a basic DataValue as a result.</rdfs:comment>
    <rdfs:label>LiteralExpression</rdfs:label>
  </rdfs:Class>
  <rdfs:Class rdf:about="http://open-services.net/ns/sysmlv2#Subclassification">
    <rdfs:subClassOf>
      <rdfs:Class rdf:about="http://open-services.net/ns/sysmlv2#Specialization"/>
    </rdfs:subClassOf>
    <rdfs:isDefinedBy rdf:resource="http://open-services.net/ns/sysmlv2#"/>
    <rdfs:comment>Subclassification is Specialization in which both the specific and general Types are Classifier. This means all instances of the specific Classifier are also instances of the general Classifier.</rdfs:comment>
    <rdfs:label>Subclassification</rdfs:label>
  </rdfs:Class>
  <rdfs:Class rdf:about="http://open-services.net/ns/sysmlv2#CollectExpression">
    <rdfs:subClassOf rdf:resource="http://open-services.net/ns/sysmlv2#OperatorExpression"/>
    <rdfs:isDefinedBy rdf:resource="http://open-services.net/ns/sysmlv2#"/>
    <rdfs:comment>A CollectExpression is an OperatorExpression whose operator is "collect", which resolves to the Function ControlFunctions::collect from the Kernel Functions Library.</rdfs:comment>
    <rdfs:label>CollectExpression</rdfs:label>
  </rdfs:Class>
  <rdfs:Class rdf:about="http://open-services.net/ns/sysmlv2#EventOccurrenceUsage">
    <rdfs:subClassOf>
      <rdfs:Class rdf:about="http://open-services.net/ns/sysmlv2#OccurrenceUsage"/>
    </rdfs:subClassOf>
    <rdfs:isDefinedBy rdf:resource="http://open-services.net/ns/sysmlv2#"/>
    <rdfs:comment>An EventOccurrenceUsage is an OccurrenceUsage that represents another OccurrenceUsage occurring as a suboccurrence of the containing occurrence of the EventOccurrenceUsage. Unless it is the EventOccurrenceUsage itself, the referenced OccurrenceUsage is related to the EventOccurrenceUsage by a ReferenceSubsetting Relationship.</rdfs:comment>
    <rdfs:label>EventOccurrenceUsage</rdfs:label>
  </rdfs:Class>
  <rdfs:Class rdf:about="http://open-services.net/ns/sysmlv2#FlowConnectionDefinition">
    <rdfs:subClassOf>
      <rdfs:Class rdf:about="http://open-services.net/ns/sysmlv2#Interaction"/>
    </rdfs:subClassOf>
    <rdfs:subClassOf>
      <rdfs:Class rdf:about="http://open-services.net/ns/sysmlv2#ConnectionDefinition"/>
    </rdfs:subClassOf>
    <rdfs:subClassOf>
      <rdfs:Class rdf:about="http://open-services.net/ns/sysmlv2#ActionDefinition"/>
    </rdfs:subClassOf>
    <rdfs:isDefinedBy rdf:resource="http://open-services.net/ns/sysmlv2#"/>
    <rdfs:comment>A FlowConnectionDefinition is a ConnectionDefinition and ActionDefinition that is also an Interaction representing flows between Usages.</rdfs:comment>
    <rdfs:label>FlowConnectionDefinition</rdfs:label>
  </rdfs:Class>
  <rdfs:Class rdf:about="http://open-services.net/ns/sysmlv2#LiteralRational">
    <rdfs:subClassOf rdf:resource="http://open-services.net/ns/sysmlv2#LiteralExpression"/>
    <rdfs:isDefinedBy rdf:resource="http://open-services.net/ns/sysmlv2#"/>
    <rdfs:comment>A LiteralRational is a LiteralExpression that provides a Rational value as a result. Its result parameter must have the type Rational.</rdfs:comment>
    <rdfs:label>LiteralRational</rdfs:label>
  </rdfs:Class>
  <rdfs:Class rdf:about="http://open-services.net/ns/sysmlv2#ConnectionDefinition">
    <rdfs:subClassOf rdf:resource="http://open-services.net/ns/sysmlv2#PartDefinition"/>
    <rdfs:subClassOf rdf:resource="http://open-services.net/ns/sysmlv2#AssociationStructure"/>
    <rdfs:isDefinedBy rdf:resource="http://open-services.net/ns/sysmlv2#"/>
    <rdfs:comment>A ConnectionDefinition is a PartDefinition that is also an AssociationStructure. The end Features of a ConnectionDefinition must be Usages.</rdfs:comment>
    <rdfs:label>ConnectionDefinition</rdfs:label>
  </rdfs:Class>
  <rdfs:Class rdf:about="http://open-services.net/ns/sysmlv2#IncludeUseCaseUsage">
    <rdfs:subClassOf rdf:resource="http://open-services.net/ns/sysmlv2#UseCaseUsage"/>
    <rdfs:subClassOf rdf:resource="http://open-services.net/ns/sysmlv2#PerformActionUsage"/>
    <rdfs:isDefinedBy rdf:resource="http://open-services.net/ns/sysmlv2#"/>
    <rdfs:comment>An IncludeUseCaseUsage is a UseCaseUsage that represents the inclusion of a UseCaseUsage by a UseCaseDefinition or UseCaseUsage. Unless it is the IncludeUseCaseUsage itself, the UseCaseUsage to be included is related to the includedUseCase by a ReferenceSubsetting Relationship. An IncludeUseCaseUsage is also a PerformActionUsage, with its useCaseIncluded as the performedAction.</rdfs:comment>
    <rdfs:label>IncludeUseCaseUsage</rdfs:label>
  </rdfs:Class>
  <rdfs:Class rdf:about="http://open-services.net/ns/sysmlv2#ControlNode">
    <rdfs:subClassOf rdf:resource="http://open-services.net/ns/sysmlv2#ActionUsage"/>
    <rdfs:isDefinedBy rdf:resource="http://open-services.net/ns/sysmlv2#"/>
    <rdfs:comment>A ControlNode is an ActionUsage that does not have any inherent behavior but provides constraints on incoming and outgoing Successions that are used to control other Actions. A ControlNode must be a composite owned usage of an ActionDefinition or ActionUsage.</rdfs:comment>
    <rdfs:label>ControlNode</rdfs:label>
  </rdfs:Class>
  <rdfs:Class rdf:about="http://open-services.net/ns/sysmlv2#ActorMembership">
    <rdfs:subClassOf rdf:resource="http://open-services.net/ns/sysmlv2#ParameterMembership"/>
    <rdfs:isDefinedBy rdf:resource="http://open-services.net/ns/sysmlv2#"/>
    <rdfs:comment>An ActorMembership is a ParameterMembership that identifies a PartUsage as an actor parameter, which specifies a role played by an external entity in interaction with the owningType of the ActorMembership.</rdfs:comment>
    <rdfs:label>ActorMembership</rdfs:label>
  </rdfs:Class>
  <rdfs:Class rdf:about="http://open-services.net/ns/sysmlv2#MergeNode">
    <rdfs:subClassOf rdf:resource="http://open-services.net/ns/sysmlv2#ControlNode"/>
    <rdfs:isDefinedBy rdf:resource="http://open-services.net/ns/sysmlv2#"/>
    <rdfs:comment>A MergeNode is a ControlNode that asserts the merging of its incoming Successions. A MergeNode may have at most one outgoing Successions.</rdfs:comment>
    <rdfs:label>MergeNode</rdfs:label>
  </rdfs:Class>
  <rdfs:Class rdf:about="http://open-services.net/ns/sysmlv2#ConstraintUsage">
    <rdfs:subClassOf>
      <rdfs:Class rdf:about="http://open-services.net/ns/sysmlv2#OccurrenceUsage"/>
    </rdfs:subClassOf>
    <rdfs:subClassOf rdf:resource="http://open-services.net/ns/sysmlv2#BooleanExpression"/>
    <rdfs:isDefinedBy rdf:resource="http://open-services.net/ns/sysmlv2#"/>
    <rdfs:comment>A ConstraintUsage is an OccurrenceUsage that is also a BooleanExpression, and, so, is typed by a Predicate. Nominally, if the type is a ConstraintDefinition, a ConstraintUsage is a Usage of that ConstraintDefinition. However, other kinds of kernel Predicates are also allowed, to permit use of Predicates from the Kernel Model Libraries.</rdfs:comment>
    <rdfs:label>ConstraintUsage</rdfs:label>
  </rdfs:Class>
  <rdfs:Class rdf:about="http://open-services.net/ns/sysmlv2#Intersecting">
    <rdfs:subClassOf>
      <rdfs:Class rdf:about="http://open-services.net/ns/sysmlv2#Relationship"/>
    </rdfs:subClassOf>
    <rdfs:isDefinedBy rdf:resource="http://open-services.net/ns/sysmlv2#"/>
    <rdfs:comment>Intersecting is a Relationship that makes its intersectingType one of the intersectingTypes of its typeIntersected.</rdfs:comment>
    <rdfs:label>Intersecting</rdfs:label>
  </rdfs:Class>
  <rdfs:Class rdf:about="http://open-services.net/ns/sysmlv2#UseCaseDefinition">
    <rdfs:subClassOf rdf:resource="http://open-services.net/ns/sysmlv2#CaseDefinition"/>
    <rdfs:isDefinedBy rdf:resource="http://open-services.net/ns/sysmlv2#"/>
    <rdfs:comment>A UseCaseDefinition is a CaseDefinition that specifies a set of actions performed by its subject, in interaction with one or more actors external to the subject. The objective is to yield an observable result that is of value to one or more of the actors.</rdfs:comment>
    <rdfs:label>UseCaseDefinition</rdfs:label>
  </rdfs:Class>
  <rdfs:Class rdf:about="http://open-services.net/ns/sysmlv2#RequirementConstraintMembership">
    <rdfs:subClassOf rdf:resource="http://open-services.net/ns/sysmlv2#FeatureMembership"/>
    <rdfs:isDefinedBy rdf:resource="http://open-services.net/ns/sysmlv2#"/>
    <rdfs:comment>A RequirementConstraintMembership is a FeatureMembership for an assumed or required ConstraintUsage of a RequirementDefinition or RequirementUsage.</rdfs:comment>
    <rdfs:label>RequirementConstraintMembership</rdfs:label>
  </rdfs:Class>
  <rdfs:Class rdf:about="http://open-services.net/ns/sysmlv2#ResultExpressionMembership">
    <rdfs:subClassOf rdf:resource="http://open-services.net/ns/sysmlv2#FeatureMembership"/>
    <rdfs:isDefinedBy rdf:resource="http://open-services.net/ns/sysmlv2#"/>
    <rdfs:comment>A ResultExpressionMembership is a FeatureMembership that indicates that the ownedResultExpression provides the result values for the Function or Expression that owns it. The owning Function or Expression must contain a BindingConnector between the result parameter of the ownedResultExpression and the result parameter of the owning Function or Expression.</rdfs:comment>
    <rdfs:label>ResultExpressionMembership</rdfs:label>
  </rdfs:Class>
  <rdfs:Class rdf:about="http://open-services.net/ns/sysmlv2#MultiplicityRange">
    <rdfs:subClassOf rdf:resource="http://open-services.net/ns/sysmlv2#Multiplicity"/>
    <rdfs:isDefinedBy rdf:resource="http://open-services.net/ns/sysmlv2#"/>
    <rdfs:comment>A MultiplicityRange is a Multiplicity whose value is defined to be the (inclusive) range of natural numbers given by the result of a lowerBound Expression and the result of an upperBound Expression. The result of these Expressions shall be of type Natural. If the result of the upperBound Expression is the unbounded value *, then the specified range includes all natural numbers greater than or equal to the lowerBound value. If no lowerBound Expression, then the default is that the lower bound has the same value as the upper bound, except if the upperBound evaluates to *, in which case the default for the lower bound is 0.</rdfs:comment>
    <rdfs:label>MultiplicityRange</rdfs:label>
  </rdfs:Class>
  <rdfs:Class rdf:about="http://open-services.net/ns/sysmlv2#TypeFeaturing">
    <rdfs:subClassOf rdf:resource="http://open-services.net/ns/sysmlv2#Featuring"/>
    <rdfs:isDefinedBy rdf:resource="http://open-services.net/ns/sysmlv2#"/>
    <rdfs:comment>A TypeFeaturing is a Featuring Relationship in which the featureOfType is the source and the featuringType is the target.</rdfs:comment>
    <rdfs:label>TypeFeaturing</rdfs:label>
  </rdfs:Class>
  <rdfs:Class rdf:about="http://open-services.net/ns/sysmlv2#OccurrenceUsage">
    <rdfs:subClassOf rdf:resource="http://open-services.net/ns/sysmlv2#Usage"/>
    <rdfs:isDefinedBy rdf:resource="http://open-services.net/ns/sysmlv2#"/>
    <rdfs:comment>An OccurrenceUsage is a Usage whose types are all Classes. Nominally, if a type is an OccurrenceDefinition, an OccurrenceUsage is a Usage of that OccurrenceDefinition within a system. However, other types of Kernel Classes are also allowed, to permit use of Classes from the Kernel Model Libraries.</rdfs:comment>
    <rdfs:label>OccurrenceUsage</rdfs:label>
  </rdfs:Class>
  <rdfs:Class rdf:about="http://open-services.net/ns/sysmlv2#ConnectorAsUsage">
    <rdfs:subClassOf rdf:resource="http://open-services.net/ns/sysmlv2#Usage"/>
    <rdfs:subClassOf rdf:resource="http://open-services.net/ns/sysmlv2#Connector"/>
    <rdfs:isDefinedBy rdf:resource="http://open-services.net/ns/sysmlv2#"/>
    <rdfs:comment>A ConnectorAsUsage is both a Connector and a Usage. ConnectorAsUsage cannot itself be instantiated in a SysML model, but it is the base class for the concrete classes BindingConnectorAsUsage, SuccessionAsUsage and ConnectionUsage.</rdfs:comment>
    <rdfs:label>ConnectorAsUsage</rdfs:label>
  </rdfs:Class>
  <rdfs:Class rdf:about="http://open-services.net/ns/sysmlv2#MembershipExpose">
    <rdfs:subClassOf>
      <rdfs:Class rdf:about="http://open-services.net/ns/sysmlv2#MembershipImport"/>
    </rdfs:subClassOf>
    <rdfs:subClassOf>
      <rdfs:Class rdf:about="http://open-services.net/ns/sysmlv2#Expose"/>
    </rdfs:subClassOf>
    <rdfs:isDefinedBy rdf:resource="http://open-services.net/ns/sysmlv2#"/>
    <rdfs:comment>A MembershipExpose is an Expose  that exposes a specific importedMembership and, if isRecursive = true, additional Memberships recursively.</rdfs:comment>
    <rdfs:label>MembershipExpose</rdfs:label>
  </rdfs:Class>
  <rdfs:Class rdf:about="http://open-services.net/ns/sysmlv2#FeatureDirectionKind">
    <rdfs:isDefinedBy rdf:resource="http://open-services.net/ns/sysmlv2#"/>
    <rdfs:comment>FeatureDirectionKind enumerates the possible kinds of direction that a Feature may be given as a member of a Type.</rdfs:comment>
    <rdfs:label>FeatureDirectionKind</rdfs:label>
  </rdfs:Class>
  <rdfs:Class rdf:about="http://open-services.net/ns/sysmlv2#AllocationDefinition">
    <rdfs:subClassOf rdf:resource="http://open-services.net/ns/sysmlv2#ConnectionDefinition"/>
    <rdfs:isDefinedBy rdf:resource="http://open-services.net/ns/sysmlv2#"/>
    <rdfs:comment>An AllocationDefinition is a ConnectionDefinition that specifies that some or all of the responsibility to realize the intent of the source is allocated to the target instances. Such allocations define mappings across the various structures and hierarchies of a system model, perhaps as a precursor to more rigorous specifications and implementations. An AllocationDefinition can itself be refined using nested allocations that give a finer-grained decomposition of the containing allocation mapping.</rdfs:comment>
    <rdfs:label>AllocationDefinition</rdfs:label>
  </rdfs:Class>
  <rdfs:Class rdf:about="http://open-services.net/ns/sysmlv2#Invariant">
    <rdfs:subClassOf rdf:resource="http://open-services.net/ns/sysmlv2#BooleanExpression"/>
    <rdfs:isDefinedBy rdf:resource="http://open-services.net/ns/sysmlv2#"/>
    <rdfs:comment>An Invariant is a BooleanExpression that is asserted to have a specific Boolean result value. If isNegated = false, then the result is asserted to be true. If isNegated = true, then the result is asserted to be false.</rdfs:comment>
    <rdfs:label>Invariant</rdfs:label>
  </rdfs:Class>
  <rdfs:Class rdf:about="http://open-services.net/ns/sysmlv2#AttributeDefinition">
    <rdfs:subClassOf>
      <rdfs:Class rdf:about="http://open-services.net/ns/sysmlv2#Definition"/>
    </rdfs:subClassOf>
    <rdfs:subClassOf rdf:resource="http://open-services.net/ns/sysmlv2#DataType"/>
    <rdfs:isDefinedBy rdf:resource="http://open-services.net/ns/sysmlv2#"/>
    <rdfs:comment>An AttributeDefinition is a Definition and a DataType of information about a quality or characteristic of a system or part of a system that has no independent identity other than its value. All features of an AttributeDefinition must be referential (non-composite).</rdfs:comment>
    <rdfs:label>AttributeDefinition</rdfs:label>
  </rdfs:Class>
  <rdfs:Class rdf:about="http://open-services.net/ns/sysmlv2#LiteralInfinity">
    <rdfs:subClassOf rdf:resource="http://open-services.net/ns/sysmlv2#LiteralExpression"/>
    <rdfs:isDefinedBy rdf:resource="http://open-services.net/ns/sysmlv2#"/>
    <rdfs:comment>A LiteralInfinity is a LiteralExpression that provides the positive infinity value (*). It's result must have the type Positive.</rdfs:comment>
    <rdfs:label>LiteralInfinity</rdfs:label>
  </rdfs:Class>
  <rdfs:Class rdf:about="http://open-services.net/ns/sysmlv2#Interaction">
    <rdfs:subClassOf rdf:resource="http://open-services.net/ns/sysmlv2#Behavior"/>
    <rdfs:subClassOf>
      <rdfs:Class rdf:about="http://open-services.net/ns/sysmlv2#Association"/>
    </rdfs:subClassOf>
    <rdfs:isDefinedBy rdf:resource="http://open-services.net/ns/sysmlv2#"/>
    <rdfs:comment>An Interaction is a Behavior that is also an Association, providing a context for multiple objects that have behaviors that impact one another.</rdfs:comment>
    <rdfs:label>Interaction</rdfs:label>
  </rdfs:Class>
  <rdfs:Class rdf:about="http://open-services.net/ns/sysmlv2#ItemFeature">
    <rdfs:subClassOf rdf:resource="http://open-services.net/ns/sysmlv2#Feature"/>
    <rdfs:isDefinedBy rdf:resource="http://open-services.net/ns/sysmlv2#"/>
    <rdfs:comment>An ItemFeature is the ownedFeature of an ItemFlow that identifies the things carried by the kinds of transfers that are instances of the ItemFlow.</rdfs:comment>
    <rdfs:label>ItemFeature</rdfs:label>
  </rdfs:Class>
  <rdfs:Class rdf:about="http://open-services.net/ns/sysmlv2#ViewUsage">
    <rdfs:subClassOf>
      <rdfs:Class rdf:about="http://open-services.net/ns/sysmlv2#PartUsage"/>
    </rdfs:subClassOf>
    <rdfs:isDefinedBy rdf:resource="http://open-services.net/ns/sysmlv2#"/>
    <rdfs:comment>A ViewUsage is a usage of a ViewDefinition to specify the generation of a view of the members of a collection of exposedNamespaces. The ViewUsage can satisfy more viewpoints than its definition, and it can specialize the viewRendering specified by its definition.</rdfs:comment>
    <rdfs:label>ViewUsage</rdfs:label>
  </rdfs:Class>
  <rdfs:Class rdf:about="http://open-services.net/ns/sysmlv2#Namespace">
    <rdfs:subClassOf rdf:resource="http://open-services.net/ns/sysmlv2#Element"/>
    <rdfs:isDefinedBy rdf:resource="http://open-services.net/ns/sysmlv2#"/>
    <rdfs:comment>A Namespace is an Element that contains other Elements, known as its members, via Membership Relationships with those Elements. The members of a Namespace may be owned by the Namespace, aliased in the Namespace, or imported into the Namespace via Import Relationships.</rdfs:comment>
    <rdfs:label>Namespace</rdfs:label>
  </rdfs:Class>
  <rdfs:Class rdf:about="http://open-services.net/ns/sysmlv2#ActionDefinition">
    <rdfs:subClassOf>
      <rdfs:Class rdf:about="http://open-services.net/ns/sysmlv2#OccurrenceDefinition"/>
    </rdfs:subClassOf>
    <rdfs:subClassOf rdf:resource="http://open-services.net/ns/sysmlv2#Behavior"/>
    <rdfs:isDefinedBy rdf:resource="http://open-services.net/ns/sysmlv2#"/>
    <rdfs:comment>An ActionDefinition is a Definition that is also a Behavior that defines an Action performed by a system or part of a system.</rdfs:comment>
    <rdfs:label>ActionDefinition</rdfs:label>
  </rdfs:Class>
  <rdfs:Class rdf:about="http://open-services.net/ns/sysmlv2#Predicate">
    <rdfs:subClassOf>
      <rdfs:Class rdf:about="http://open-services.net/ns/sysmlv2#Function"/>
    </rdfs:subClassOf>
    <rdfs:isDefinedBy rdf:resource="http://open-services.net/ns/sysmlv2#"/>
    <rdfs:comment>A Predicate is a Function whose result parameter has type Boolean and multiplicity 1..1.</rdfs:comment>
    <rdfs:label>Predicate</rdfs:label>
  </rdfs:Class>
  <rdfs:Class rdf:about="http://open-services.net/ns/sysmlv2#FeatureValue">
    <rdfs:subClassOf rdf:resource="http://open-services.net/ns/sysmlv2#OwningMembership"/>
    <rdfs:isDefinedBy rdf:resource="http://open-services.net/ns/sysmlv2#"/>
    <rdfs:comment>A FeatureValue is a Membership that identifies a particular member Expression that provides the value of the Feature that owns the FeatureValue. The value is specified as either a bound value or an initial value, and as either a concrete or default value. A Feature can have at most one FeatureValue.</rdfs:comment>
    <rdfs:label>FeatureValue</rdfs:label>
  </rdfs:Class>
  <rdfs:Class rdf:about="http://open-services.net/ns/sysmlv2#Dependency">
    <rdfs:subClassOf>
      <rdfs:Class rdf:about="http://open-services.net/ns/sysmlv2#Relationship"/>
    </rdfs:subClassOf>
    <rdfs:isDefinedBy rdf:resource="http://open-services.net/ns/sysmlv2#"/>
    <rdfs:comment>A Dependency is a Relationship that indicates that one or more client Elements require one more supplier Elements for their complete specification. In general, this means that a change to one of the supplier Elements may necessitate a change to, or re-specification of, the client Elements.</rdfs:comment>
    <rdfs:label>Dependency</rdfs:label>
  </rdfs:Class>
  <rdfs:Class rdf:about="http://open-services.net/ns/sysmlv2#ConjugatedPortTyping">
    <rdfs:subClassOf>
      <rdfs:Class rdf:about="http://open-services.net/ns/sysmlv2#FeatureTyping"/>
    </rdfs:subClassOf>
    <rdfs:isDefinedBy rdf:resource="http://open-services.net/ns/sysmlv2#"/>
    <rdfs:comment>A ConjugatedPortTyping is a FeatureTyping whose type is a ConjugatedPortDefinition. (This relationship is intended to be an abstract-syntax marker for a special surface notation for conjugated typing of ports.).</rdfs:comment>
    <rdfs:label>ConjugatedPortTyping</rdfs:label>
  </rdfs:Class>
  <rdfs:Class rdf:about="http://open-services.net/ns/sysmlv2#LoopActionUsage">
    <rdfs:subClassOf rdf:resource="http://open-services.net/ns/sysmlv2#ActionUsage"/>
    <rdfs:isDefinedBy rdf:resource="http://open-services.net/ns/sysmlv2#"/>
    <rdfs:comment>A LoopActionUsage is an ActionUsage that specifies that its bodyAction should be performed repeatedly. Its subclasses WhileLoopActionUsage and ForLoopActionUsage provide different ways to determine how many times the bodyAction should be performed.</rdfs:comment>
    <rdfs:label>LoopActionUsage</rdfs:label>
  </rdfs:Class>
  <rdfs:Class rdf:about="http://open-services.net/ns/sysmlv2#MembershipImport">
    <rdfs:subClassOf>
      <rdfs:Class rdf:about="http://open-services.net/ns/sysmlv2#Import"/>
    </rdfs:subClassOf>
    <rdfs:isDefinedBy rdf:resource="http://open-services.net/ns/sysmlv2#"/>
    <rdfs:comment>A MembershipImport is an Import that imports its importedMembership into the importOwningNamespace. If isRecursive = true and the memberElement of the importedMembership is a Namespace, then the equivalent of a recursive NamespaceImport is also performed on that Namespace.</rdfs:comment>
    <rdfs:label>MembershipImport</rdfs:label>
  </rdfs:Class>
  <rdfs:Class rdf:about="http://open-services.net/ns/sysmlv2#EndFeatureMembership">
    <rdfs:subClassOf rdf:resource="http://open-services.net/ns/sysmlv2#FeatureMembership"/>
    <rdfs:isDefinedBy rdf:resource="http://open-services.net/ns/sysmlv2#"/>
    <rdfs:comment>EndFeatureMembership is a FeatureMembership that requires its memberFeature be owned and have isEnd = true.</rdfs:comment>
    <rdfs:label>EndFeatureMembership</rdfs:label>
  </rdfs:Class>
  <rdfs:Class rdf:about="http://open-services.net/ns/sysmlv2#LiteralBoolean">
    <rdfs:subClassOf rdf:resource="http://open-services.net/ns/sysmlv2#LiteralExpression"/>
    <rdfs:isDefinedBy rdf:resource="http://open-services.net/ns/sysmlv2#"/>
    <rdfs:comment>LiteralBoolean is a LiteralExpression that provides a Boolean value as a result. Its result parameter must have type Boolean.</rdfs:comment>
    <rdfs:label>LiteralBoolean</rdfs:label>
  </rdfs:Class>
  <rdfs:Class rdf:about="http://open-services.net/ns/sysmlv2#FlowConnectionUsage">
    <rdfs:subClassOf rdf:resource="http://open-services.net/ns/sysmlv2#ItemFlow"/>
    <rdfs:subClassOf rdf:resource="http://open-services.net/ns/sysmlv2#ConnectionUsage"/>
    <rdfs:subClassOf rdf:resource="http://open-services.net/ns/sysmlv2#ActionUsage"/>
    <rdfs:isDefinedBy rdf:resource="http://open-services.net/ns/sysmlv2#"/>
    <rdfs:comment>A FlowConnectionUsage is a ConnectionUsage that is also an ItemFlow.</rdfs:comment>
    <rdfs:label>FlowConnectionUsage</rdfs:label>
  </rdfs:Class>
  <rdfs:Class rdf:about="http://open-services.net/ns/sysmlv2#AssignmentActionUsage">
    <rdfs:subClassOf rdf:resource="http://open-services.net/ns/sysmlv2#ActionUsage"/>
    <rdfs:isDefinedBy rdf:resource="http://open-services.net/ns/sysmlv2#"/>
    <rdfs:comment>An AssignmentActionUsage is an ActionUsage that is defined, directly or indirectly, by the ActionDefinition AssignmentAction from the Systems Model Library. It specifies that the value of the referent Feature, relative to the target given by the result of the targetArgument Expression, should be set to the result of the valueExpression.</rdfs:comment>
    <rdfs:label>AssignmentActionUsage</rdfs:label>
  </rdfs:Class>
  <rdfs:Class rdf:about="http://open-services.net/ns/sysmlv2#Specialization">
    <rdfs:subClassOf>
      <rdfs:Class rdf:about="http://open-services.net/ns/sysmlv2#Relationship"/>
    </rdfs:subClassOf>
    <rdfs:isDefinedBy rdf:resource="http://open-services.net/ns/sysmlv2#"/>
    <rdfs:comment>Specialization is a Relationship between two Types that requires all instances of the specific type to also be instances of the general Type (i.e., the set of instances of the specific Type is a subset of those of the general Type, which might be the same set).</rdfs:comment>
    <rdfs:label>Specialization</rdfs:label>
  </rdfs:Class>
  <rdfs:Class rdf:about="http://open-services.net/ns/sysmlv2#ReturnParameterMembership">
    <rdfs:subClassOf rdf:resource="http://open-services.net/ns/sysmlv2#ParameterMembership"/>
    <rdfs:isDefinedBy rdf:resource="http://open-services.net/ns/sysmlv2#"/>
    <rdfs:comment>A ReturnParameterMembership is a ParameterMembership that indicates that the ownedMemberParameter is the result parameter of a Function or Expression. The direction of the ownedMemberParameter must be out.</rdfs:comment>
    <rdfs:label>ReturnParameterMembership</rdfs:label>
  </rdfs:Class>
  <rdfs:Class rdf:about="http://open-services.net/ns/sysmlv2#ViewpointDefinition">
    <rdfs:subClassOf>
      <rdfs:Class rdf:about="http://open-services.net/ns/sysmlv2#RequirementDefinition"/>
    </rdfs:subClassOf>
    <rdfs:isDefinedBy rdf:resource="http://open-services.net/ns/sysmlv2#"/>
    <rdfs:comment>A ViewpointDefinition is a RequirementDefinition that specifies one or more stakeholder concerns that are to be satisfied by creating a view of a model.</rdfs:comment>
    <rdfs:label>ViewpointDefinition</rdfs:label>
  </rdfs:Class>
  <rdfs:Class rdf:about="http://open-services.net/ns/sysmlv2#Package">
    <rdfs:subClassOf rdf:resource="http://open-services.net/ns/sysmlv2#Namespace"/>
    <rdfs:isDefinedBy rdf:resource="http://open-services.net/ns/sysmlv2#"/>
    <rdfs:comment>A Package is a Namespace used to group Elements, without any instance-level semantics. It may have one or more model-level evaluable filterCondition Expressions used to filter its importedMemberships. Any imported member must meet all of the filterConditions.</rdfs:comment>
    <rdfs:label>Package</rdfs:label>
  </rdfs:Class>
  <rdfs:Class rdf:about="http://open-services.net/ns/sysmlv2#Subsetting">
    <rdfs:subClassOf rdf:resource="http://open-services.net/ns/sysmlv2#Specialization"/>
    <rdfs:isDefinedBy rdf:resource="http://open-services.net/ns/sysmlv2#"/>
    <rdfs:comment>Subsetting is Specialization in which the specific and general Types are Features. This means all values of the subsettingFeature (on instances of its domain, i.e., the intersection of its featuringTypes) are values of the subsettedFeature on instances of its domain. To support this the domain of the subsettingFeature must be the same or specialize (at least indirectly) the domain of the subsettedFeature (via Specialization), and the co-domain (intersection of the types) of the subsettingFeature must specialize the co-domain of the subsettedFeature.</rdfs:comment>
    <rdfs:label>Subsetting</rdfs:label>
  </rdfs:Class>
  <rdfs:Class rdf:about="http://open-services.net/ns/sysmlv2#PortionKind">
    <rdfs:isDefinedBy rdf:resource="http://open-services.net/ns/sysmlv2#"/>
    <rdfs:comment>PortionKind is an enumeration of the specific kinds of Occurrence portions that can be represented by an OccurrenceUsage.</rdfs:comment>
    <rdfs:label>PortionKind</rdfs:label>
  </rdfs:Class>
  <rdfs:Class rdf:about="http://open-services.net/ns/sysmlv2#VerificationCaseUsage">
    <rdfs:subClassOf rdf:resource="http://open-services.net/ns/sysmlv2#CaseUsage"/>
    <rdfs:isDefinedBy rdf:resource="http://open-services.net/ns/sysmlv2#"/>
    <rdfs:comment>A VerificationCaseUsage is a Usage of a VerificationCaseDefinition.</rdfs:comment>
    <rdfs:label>VerificationCaseUsage</rdfs:label>
  </rdfs:Class>
  <rdfs:Class rdf:about="http://open-services.net/ns/sysmlv2#RequirementVerificationMembership">
    <rdfs:subClassOf rdf:resource="http://open-services.net/ns/sysmlv2#RequirementConstraintMembership"/>
    <rdfs:isDefinedBy rdf:resource="http://open-services.net/ns/sysmlv2#"/>
    <rdfs:comment>A RequirementVerificationMembership is a RequirementConstraintMembership  used in the objective of a VerificationCase to identify a RequirementUsage that is verified by the VerificationCase.</rdfs:comment>
    <rdfs:label>RequirementVerificationMembership</rdfs:label>
  </rdfs:Class>
  <rdfs:Class rdf:about="http://open-services.net/ns/sysmlv2#Expression">
    <rdfs:subClassOf rdf:resource="http://open-services.net/ns/sysmlv2#Step"/>
    <rdfs:isDefinedBy rdf:resource="http://open-services.net/ns/sysmlv2#"/>
    <rdfs:comment>An Expression is a Step that is typed by a Function. An Expression that also has a Function as its featuringType is a computational step within that Function. An Expression always has a single result parameter, which redefines the result parameter of its defining function. This allows Expressions to be interconnected in tree structures, in which inputs to each Expression in the tree are determined as the results of other Expression in the tree.</rdfs:comment>
    <rdfs:label>Expression</rdfs:label>
  </rdfs:Class>
  <rdfs:Class rdf:about="http://open-services.net/ns/sysmlv2#Metaclass">
    <rdfs:subClassOf rdf:resource="http://open-services.net/ns/sysmlv2#Structure"/>
    <rdfs:isDefinedBy rdf:resource="http://open-services.net/ns/sysmlv2#"/>
    <rdfs:comment>A Metaclass is a Structure used to type MetadataFeatures.</rdfs:comment>
    <rdfs:label>Metaclass</rdfs:label>
  </rdfs:Class>
  <rdfs:Class rdf:about="http://open-services.net/ns/sysmlv2#Expose">
    <rdfs:subClassOf>
      <rdfs:Class rdf:about="http://open-services.net/ns/sysmlv2#Import"/>
    </rdfs:subClassOf>
    <rdfs:isDefinedBy rdf:resource="http://open-services.net/ns/sysmlv2#"/>
    <rdfs:comment>An Expose is an Import of Memberships into a ViewUsage that provide the Elements to be included in a view. Visibility is always ignored for an Expose (i.e., isImportAll = true).</rdfs:comment>
    <rdfs:label>Expose</rdfs:label>
  </rdfs:Class>
  <rdfs:Class rdf:about="http://open-services.net/ns/sysmlv2#Definition">
    <rdfs:subClassOf rdf:resource="http://open-services.net/ns/sysmlv2#Classifier"/>
    <rdfs:isDefinedBy rdf:resource="http://open-services.net/ns/sysmlv2#"/>
    <rdfs:comment>A Definition is a Classifier of Usages. The actual kinds of Definition that may appear in a model are given by the subclasses of Definition (possibly as extended with user-defined SemanticMetadata).</rdfs:comment>
    <rdfs:label>Definition</rdfs:label>
  </rdfs:Class>
  <rdfs:Class rdf:about="http://open-services.net/ns/sysmlv2#ViewDefinition">
    <rdfs:subClassOf rdf:resource="http://open-services.net/ns/sysmlv2#PartDefinition"/>
    <rdfs:isDefinedBy rdf:resource="http://open-services.net/ns/sysmlv2#"/>
    <rdfs:comment>A ViewDefinition is a PartDefinition that specifies how a view artifact is constructed to satisfy a viewpoint. It specifies a viewConditions to define the model content to be presented and a viewRendering to define how the model content is presented.</rdfs:comment>
    <rdfs:label>ViewDefinition</rdfs:label>
  </rdfs:Class>
  <rdfs:Class rdf:about="http://open-services.net/ns/sysmlv2#RequirementDefinition">
    <rdfs:subClassOf rdf:resource="http://open-services.net/ns/sysmlv2#ConstraintDefinition"/>
    <rdfs:isDefinedBy rdf:resource="http://open-services.net/ns/sysmlv2#"/>
    <rdfs:comment>A RequirementDefinition is a ConstraintDefinition that defines a requirement used in the context of a specification as a constraint that a valid solution must satisfy. The specification is relative to a specified subject, possibly in collaboration with one or more external actors.</rdfs:comment>
    <rdfs:label>RequirementDefinition</rdfs:label>
  </rdfs:Class>
  <rdfs:Class rdf:about="http://open-services.net/ns/sysmlv2#FeatureTyping">
    <rdfs:subClassOf rdf:resource="http://open-services.net/ns/sysmlv2#Specialization"/>
    <rdfs:isDefinedBy rdf:resource="http://open-services.net/ns/sysmlv2#"/>
    <rdfs:comment>FeatureTyping is Specialization in which the specific Type is a Feature. This means the set of instances of the (specific) typedFeature is a subset of the set of instances of the (general) type. In the simplest case, the type is a Classifier, whereupon the typedFeature has values that are instances of the Classifier.</rdfs:comment>
    <rdfs:label>FeatureTyping</rdfs:label>
  </rdfs:Class>
  <rdfs:Class rdf:about="http://open-services.net/ns/sysmlv2#FeatureChainExpression">
    <rdfs:subClassOf rdf:resource="http://open-services.net/ns/sysmlv2#OperatorExpression"/>
    <rdfs:isDefinedBy rdf:resource="http://open-services.net/ns/sysmlv2#"/>
    <rdfs:comment>A FeatureChainExpression is an OperatorExpression whose operator is ".", which resolves to the Function ControlFunctions::'.' from the Kernel Functions Library. It evaluates to the result of chaining the result Feature of its single argument Expression with its targetFeature.</rdfs:comment>
    <rdfs:label>FeatureChainExpression</rdfs:label>
  </rdfs:Class>
  <rdfs:Class rdf:about="http://open-services.net/ns/sysmlv2#ElementFilterMembership">
    <rdfs:subClassOf rdf:resource="http://open-services.net/ns/sysmlv2#OwningMembership"/>
    <rdfs:isDefinedBy rdf:resource="http://open-services.net/ns/sysmlv2#"/>
    <rdfs:comment>ElementFilterMembership is a Membership between a Namespace and a model-level evaluable Boolean-valued Expression, asserting that imported members of the Namespace should be filtered using the condition Expression. A general Namespace does not define any specific filtering behavior, but such behavior may be defined for various specialized kinds of Namespaces.</rdfs:comment>
    <rdfs:label>ElementFilterMembership</rdfs:label>
  </rdfs:Class>
  <rdfs:Class rdf:about="http://open-services.net/ns/sysmlv2#ExhibitStateUsage">
    <rdfs:subClassOf>
      <rdfs:Class rdf:about="http://open-services.net/ns/sysmlv2#StateUsage"/>
    </rdfs:subClassOf>
    <rdfs:subClassOf rdf:resource="http://open-services.net/ns/sysmlv2#PerformActionUsage"/>
    <rdfs:isDefinedBy rdf:resource="http://open-services.net/ns/sysmlv2#"/>
    <rdfs:comment>An ExhibitStateUsage is a StateUsage that represents the exhibiting of a StateUsage. Unless it is the StateUsage itself, the StateUsage to be exhibited is related to the ExhibitStateUsage by a ReferenceSubsetting Relationship. An ExhibitStateUsage is also a PerformActionUsage, with its exhibitedState as the performedAction.</rdfs:comment>
    <rdfs:label>ExhibitStateUsage</rdfs:label>
  </rdfs:Class>
  <rdfs:Class rdf:about="http://open-services.net/ns/sysmlv2#SuccessionFlowConnectionUsage">
    <rdfs:subClassOf rdf:resource="http://open-services.net/ns/sysmlv2#SuccessionItemFlow"/>
    <rdfs:subClassOf rdf:resource="http://open-services.net/ns/sysmlv2#FlowConnectionUsage"/>
    <rdfs:isDefinedBy rdf:resource="http://open-services.net/ns/sysmlv2#"/>
    <rdfs:comment>A SuccessionFlowConnectionUsage is a FlowConnectionUsage that is also a SuccessionItemFlow.</rdfs:comment>
    <rdfs:label>SuccessionFlowConnectionUsage</rdfs:label>
  </rdfs:Class>
  <rdfs:Class rdf:about="http://open-services.net/ns/sysmlv2#PartUsage">
    <rdfs:subClassOf rdf:resource="http://open-services.net/ns/sysmlv2#ItemUsage"/>
    <rdfs:isDefinedBy rdf:resource="http://open-services.net/ns/sysmlv2#"/>
    <rdfs:comment>A PartUsage is a usage of a PartDefinition to represent a system or a part of a system. At least one of the itemDefinitions of the PartUsage must be a PartDefinition.</rdfs:comment>
    <rdfs:label>PartUsage</rdfs:label>
  </rdfs:Class>
  <rdfs:Class rdf:about="http://open-services.net/ns/sysmlv2#SendActionUsage">
    <rdfs:subClassOf rdf:resource="http://open-services.net/ns/sysmlv2#ActionUsage"/>
    <rdfs:isDefinedBy rdf:resource="http://open-services.net/ns/sysmlv2#"/>
    <rdfs:comment>A SendActionUsage is an ActionUsage that specifies the sending of a payload given by the result of its payloadArgument Expression via a MessageTransfer whose source is given by the result of the senderArgument Expression and whose target is given by the result of the receiverArgument Expression. If no senderArgument is provided, the default is the this context for the action. If no receiverArgument is given, then the receiver is to be determined by, e.g., outgoing Connections from the sender.</rdfs:comment>
    <rdfs:label>SendActionUsage</rdfs:label>
  </rdfs:Class>
  <rdfs:Class rdf:about="http://open-services.net/ns/sysmlv2#SuccessionAsUsage">
    <rdfs:subClassOf rdf:resource="http://open-services.net/ns/sysmlv2#Succession"/>
    <rdfs:subClassOf rdf:resource="http://open-services.net/ns/sysmlv2#ConnectorAsUsage"/>
    <rdfs:isDefinedBy rdf:resource="http://open-services.net/ns/sysmlv2#"/>
    <rdfs:comment>A SuccessionAsUsage is both a ConnectorAsUsage and a Succession.</rdfs:comment>
    <rdfs:label>SuccessionAsUsage</rdfs:label>
  </rdfs:Class>
  <rdfs:Class rdf:about="http://open-services.net/ns/sysmlv2#Association">
    <rdfs:subClassOf>
      <rdfs:Class rdf:about="http://open-services.net/ns/sysmlv2#Relationship"/>
    </rdfs:subClassOf>
    <rdfs:subClassOf rdf:resource="http://open-services.net/ns/sysmlv2#Classifier"/>
    <rdfs:isDefinedBy rdf:resource="http://open-services.net/ns/sysmlv2#"/>
    <rdfs:comment>An Association is a Relationship and a Classifier to enable classification of links between things (in the universe). The co-domains (types) of the associationEnd Features are the relatedTypes, as co-domain and participants (linked things) of an Association identify each other.</rdfs:comment>
    <rdfs:label>Association</rdfs:label>
  </rdfs:Class>
  <rdfs:Class rdf:about="http://open-services.net/ns/sysmlv2#VariantMembership">
    <rdfs:subClassOf rdf:resource="http://open-services.net/ns/sysmlv2#OwningMembership"/>
    <rdfs:isDefinedBy rdf:resource="http://open-services.net/ns/sysmlv2#"/>
    <rdfs:comment>A VariantMembership is a Membership between a variation point Definition or Usage and a Usage that represents a variant in the context of that variation. The membershipOwningNamespace for the VariantMembership must be either a Definition or a Usage with isVariation = true.</rdfs:comment>
    <rdfs:label>VariantMembership</rdfs:label>
  </rdfs:Class>
  <rdfs:Class rdf:about="http://open-services.net/ns/sysmlv2#StateUsage">
    <rdfs:subClassOf rdf:resource="http://open-services.net/ns/sysmlv2#ActionUsage"/>
    <rdfs:isDefinedBy rdf:resource="http://open-services.net/ns/sysmlv2#"/>
    <rdfs:comment>A StateUsage is an ActionUsage that is nominally the Usage of a StateDefinition. However, other kinds of kernel Behaviors are also allowed as types, to permit use of Behaviors
.</rdfs:comment>
    <rdfs:label>StateUsage</rdfs:label>
  </rdfs:Class>
  <rdfs:Class rdf:about="http://open-services.net/ns/sysmlv2#InvocationExpression">
    <rdfs:subClassOf rdf:resource="http://open-services.net/ns/sysmlv2#Expression"/>
    <rdfs:isDefinedBy rdf:resource="http://open-services.net/ns/sysmlv2#"/>
    <rdfs:comment>An InvocationExpression is an Expression each of whose input parameters are bound to the result of an argument Expression.</rdfs:comment>
    <rdfs:label>InvocationExpression</rdfs:label>
  </rdfs:Class>
  <rdfs:Class rdf:about="http://open-services.net/ns/sysmlv2#Unioning">
    <rdfs:subClassOf>
      <rdfs:Class rdf:about="http://open-services.net/ns/sysmlv2#Relationship"/>
    </rdfs:subClassOf>
    <rdfs:isDefinedBy rdf:resource="http://open-services.net/ns/sysmlv2#"/>
    <rdfs:comment>Unioning is a Relationship that makes its unioningType one of the unioningTypes of its typeUnioned.</rdfs:comment>
    <rdfs:label>Unioning</rdfs:label>
  </rdfs:Class>
  <rdfs:Class rdf:about="http://open-services.net/ns/sysmlv2#Import">
    <rdfs:subClassOf>
      <rdfs:Class rdf:about="http://open-services.net/ns/sysmlv2#Relationship"/>
    </rdfs:subClassOf>
    <rdfs:isDefinedBy rdf:resource="http://open-services.net/ns/sysmlv2#"/>
    <rdfs:comment>An Import is an Relationship between its importOwningNamespace and either a Membership (for a MembershipImport) or another Namespace (for a NamespaceImport), which determines a set of Memberships that become importedMemberships of the importOwningNamespace. If isImportAll = false (the default), then only public Memberships are considered "visible". If isImportAll = true, then all Memberships are considered "visible", regardless of their declared visibility. If isRecursive = true, then visible Memberships are also recursively imported from owned sub-Namespaces.</rdfs:comment>
    <rdfs:label>Import</rdfs:label>
  </rdfs:Class>
  <rdfs:Class rdf:about="http://open-services.net/ns/sysmlv2#OccurrenceDefinition">
    <rdfs:subClassOf rdf:resource="http://open-services.net/ns/sysmlv2#Definition"/>
    <rdfs:subClassOf rdf:resource="http://open-services.net/ns/sysmlv2#Class"/>
    <rdfs:isDefinedBy rdf:resource="http://open-services.net/ns/sysmlv2#"/>
    <rdfs:comment>An OccurrenceDefinition is a Definition of a Class of individuals that have an independent life over time and potentially an extent over space. This includes both structural things and behaviors that act on such structures.</rdfs:comment>
    <rdfs:label>OccurrenceDefinition</rdfs:label>
  </rdfs:Class>
  <rdfs:Class rdf:about="http://open-services.net/ns/sysmlv2#AllocationUsage">
    <rdfs:subClassOf rdf:resource="http://open-services.net/ns/sysmlv2#ConnectionUsage"/>
    <rdfs:isDefinedBy rdf:resource="http://open-services.net/ns/sysmlv2#"/>
    <rdfs:comment>An AllocationUsage is a usage of an AllocationDefinition asserting the allocation of the source feature to the target feature.</rdfs:comment>
    <rdfs:label>AllocationUsage</rdfs:label>
  </rdfs:Class>
  <rdfs:Class rdf:about="http://open-services.net/ns/sysmlv2#MetadataAccessExpression">
    <rdfs:subClassOf rdf:resource="http://open-services.net/ns/sysmlv2#Expression"/>
    <rdfs:isDefinedBy rdf:resource="http://open-services.net/ns/sysmlv2#"/>
    <rdfs:comment>A MetadataAccessExpression is an Expression whose result is a sequence of instances of Metaclasses representing all the MetadataFeature annotations of the referencedElement. In addition, the sequence includes an instance of the reflective Metaclass corresponding to the MOF class of the referencedElement, with values for all the abstract syntax properties of the referencedElement.</rdfs:comment>
    <rdfs:label>MetadataAccessExpression</rdfs:label>
  </rdfs:Class>
  <rdfs:Class rdf:about="http://open-services.net/ns/sysmlv2#LibraryPackage">
    <rdfs:subClassOf rdf:resource="http://open-services.net/ns/sysmlv2#Package"/>
    <rdfs:isDefinedBy rdf:resource="http://open-services.net/ns/sysmlv2#"/>
    <rdfs:comment>A LibraryPackage is a Package that is the container for a model library. A LibraryPackage is itself a library Element as are all Elements that are directly or indirectly contained in it.</rdfs:comment>
    <rdfs:label>LibraryPackage</rdfs:label>
  </rdfs:Class>
  <rdfs:Class rdf:about="http://open-services.net/ns/sysmlv2#Type">
    <rdfs:subClassOf rdf:resource="http://open-services.net/ns/sysmlv2#Namespace"/>
    <rdfs:isDefinedBy rdf:resource="http://open-services.net/ns/sysmlv2#"/>
    <rdfs:comment>A Type is a Namespace that is the most general kind of Element supporting the semantics of classification. A Type may be a Classifier or a Feature, defining conditions on what is classified by the Type (see also the description of isSufficient).</rdfs:comment>
    <rdfs:label>Type</rdfs:label>
  </rdfs:Class>
  <rdfs:Class rdf:about="http://open-services.net/ns/sysmlv2#Relationship">
    <rdfs:subClassOf rdf:resource="http://open-services.net/ns/sysmlv2#Element"/>
    <rdfs:isDefinedBy rdf:resource="http://open-services.net/ns/sysmlv2#"/>
    <rdfs:comment>A Relationship is an Element that relates other Element. Some of its relatedElements may be owned, in which case those ownedRelatedElements will be deleted from a model if their owningRelationship is. A Relationship may also be owned by another Element, in which case the ownedRelatedElements of the Relationship are also considered to be transitively owned by the owningRelatedElement of the Relationship.</rdfs:comment>
    <rdfs:label>Relationship</rdfs:label>
  </rdfs:Class>
  <rdfs:Class rdf:about="http://open-services.net/ns/sysmlv2#Disjoining">
    <rdfs:subClassOf rdf:resource="http://open-services.net/ns/sysmlv2#Relationship"/>
    <rdfs:isDefinedBy rdf:resource="http://open-services.net/ns/sysmlv2#"/>
    <rdfs:comment>A Disjoining is a Relationship between Types asserted to have interpretations that are not shared (disjoint) between them, identified as typeDisjoined and disjoiningType. For example, a Classifier for mammals is disjoint from a Classifier for minerals, and a Feature for people's parents is disjoint from a Feature for their children.</rdfs:comment>
    <rdfs:label>Disjoining</rdfs:label>
  </rdfs:Class>
  <rdfs:Class rdf:about="http://open-services.net/ns/sysmlv2#Function">
    <rdfs:subClassOf rdf:resource="http://open-services.net/ns/sysmlv2#Behavior"/>
    <rdfs:isDefinedBy rdf:resource="http://open-services.net/ns/sysmlv2#"/>
    <rdfs:comment>A Function is a Behavior that has an out parameter that is identified as its result. A Function represents the performance of a calculation that produces the values of its result parameter. This calculation may be decomposed into Expressions that are steps of the Function.</rdfs:comment>
    <rdfs:label>Function</rdfs:label>
  </rdfs:Class>
  <rdf:Property rdf:about="http://open-services.net/ns/sysmlv2#renderingDefinition_Rendering">
    <rdfs:isDefinedBy rdf:resource="http://open-services.net/ns/sysmlv2#"/>
    <rdfs:comment>The usages of a RenderingDefinition that are RenderingUsages.</rdfs:comment>
    <rdfs:label>renderingDefinition_Rendering</rdfs:label>
  </rdf:Property>
  <rdf:Property rdf:about="http://open-services.net/ns/sysmlv2#interfaceDefinition_InterfaceEnd">
    <rdfs:isDefinedBy rdf:resource="http://open-services.net/ns/sysmlv2#"/>
    <rdfs:comment>The PortUsages that are the connectionEnds of this InterfaceDefinition.

.</rdfs:comment>
    <rdfs:label>interfaceDefinition_InterfaceEnd</rdfs:label>
  </rdf:Property>
  <rdf:Property rdf:about="http://open-services.net/ns/sysmlv2#annotation_OwningAnnotatingElement">
    <rdfs:isDefinedBy rdf:resource="http://open-services.net/ns/sysmlv2#"/>
    <rdfs:comment>The annotatingElement of this Annotation, when it is also its owningRelatedElement.</rdfs:comment>
    <rdfs:label>annotation_OwningAnnotatingElement</rdfs:label>
  </rdf:Property>
  <rdf:Property rdf:about="http://open-services.net/ns/sysmlv2#disjoining_OwningType">
    <rdfs:isDefinedBy rdf:resource="http://open-services.net/ns/sysmlv2#"/>
    <rdfs:comment>A typeDisjoined that is also an owningRelatedElement.</rdfs:comment>
    <rdfs:label>disjoining_OwningType</rdfs:label>
  </rdf:Property>
  <rdf:Property rdf:about="http://open-services.net/ns/sysmlv2#relationship_RelatedElement">
    <rdfs:isDefinedBy rdf:resource="http://open-services.net/ns/sysmlv2#"/>
    <rdfs:comment>The Elements that are related by this Relationship, derived as the union of the source and target Elements of the Relationship.</rdfs:comment>
    <rdfs:label>relationship_RelatedElement</rdfs:label>
  </rdf:Property>
  <rdf:Property rdf:about="http://open-services.net/ns/sysmlv2#namespace_Member">
    <rdfs:isDefinedBy rdf:resource="http://open-services.net/ns/sysmlv2#"/>
    <rdfs:comment>The set of all member Elements of this Namespace, which are the memberElements of all memberships of the Namespace.</rdfs:comment>
    <rdfs:label>namespace_Member</rdfs:label>
  </rdf:Property>
  <rdf:Property rdf:about="http://open-services.net/ns/sysmlv2#redefinition_RedefinedFeature">
    <rdfs:isDefinedBy rdf:resource="http://open-services.net/ns/sysmlv2#"/>
    <rdfs:comment>The Feature that is redefined by the redefiningFeature of this Redefinition.</rdfs:comment>
    <rdfs:label>redefinition_RedefinedFeature</rdfs:label>
  </rdf:Property>
  <rdf:Property rdf:about="http://open-services.net/ns/sysmlv2#comment_Locale">
    <rdfs:isDefinedBy rdf:resource="http://open-services.net/ns/sysmlv2#"/>
    <rdfs:comment>Identification of the language of the body text and, optionally, the region and/or encoding. The format shall be a POSIX locale conformant to ISO/IEC 15897, with the format [language[_territory][.codeset][@modifier]].</rdfs:comment>
    <rdfs:label>comment_Locale</rdfs:label>
  </rdf:Property>
  <rdf:Property rdf:about="http://open-services.net/ns/sysmlv2#assignmentActionUsage_TargetArgument">
    <rdfs:isDefinedBy rdf:resource="http://open-services.net/ns/sysmlv2#"/>
    <rdfs:comment>The Expression whose value is an occurrence in the domain of the referent Feature, for which the value of the referent will be set to the result of the valueExpression by this AssignmentActionUsage.</rdfs:comment>
    <rdfs:label>assignmentActionUsage_TargetArgument</rdfs:label>
  </rdf:Property>
  <rdf:Property rdf:about="http://open-services.net/ns/sysmlv2#feature_IsUnique">
    <rdfs:isDefinedBy rdf:resource="http://open-services.net/ns/sysmlv2#"/>
    <rdfs:comment>Whether or not values for this Feature must have no duplicates or not.</rdfs:comment>
    <rdfs:label>feature_IsUnique</rdfs:label>
  </rdf:Property>
  <rdf:Property rdf:about="http://open-services.net/ns/sysmlv2#behavior_Step">
    <rdfs:isDefinedBy rdf:resource="http://open-services.net/ns/sysmlv2#"/>
    <rdfs:comment>The Steps that make up this Behavior.</rdfs:comment>
    <rdfs:label>behavior_Step</rdfs:label>
  </rdf:Property>
  <rdf:Property rdf:about="http://open-services.net/ns/sysmlv2#includeUseCaseUsage_UseCaseIncluded">
    <rdfs:isDefinedBy rdf:resource="http://open-services.net/ns/sysmlv2#"/>
    <rdfs:comment>The UseCaseUsage to be included by this IncludeUseCaseUsage. It is the performedAction of the IncludeUseCaseUsage considered as a PerformActionUsage, which must be a UseCaseUsage.</rdfs:comment>
    <rdfs:label>includeUseCaseUsage_UseCaseIncluded</rdfs:label>
  </rdf:Property>
  <rdf:Property rdf:about="http://open-services.net/ns/sysmlv2#operatorExpression_Operator">
    <rdfs:isDefinedBy rdf:resource="http://open-services.net/ns/sysmlv2#"/>
    <rdfs:comment>An operator symbol that names a corresponding Function from one of the standard packages from the Kernel Function Library .</rdfs:comment>
    <rdfs:label>operatorExpression_Operator</rdfs:label>
  </rdf:Property>
  <rdf:Property rdf:about="http://open-services.net/ns/sysmlv2#connector_RelatedFeature">
    <rdfs:isDefinedBy rdf:resource="http://open-services.net/ns/sysmlv2#"/>
    <rdfs:comment>The Features that are related by this Connector considered as a Relationship and that restrict the links it identifies, given by the referenced Features of the connectorEnds of the Connector.</rdfs:comment>
    <rdfs:label>connector_RelatedFeature</rdfs:label>
  </rdf:Property>
  <rdf:Property rdf:about="http://open-services.net/ns/sysmlv2#definition_OwnedAllocation">
    <rdfs:isDefinedBy rdf:resource="http://open-services.net/ns/sysmlv2#"/>
    <rdfs:comment>The AllocationUsages that are ownedUsages of this Definition.</rdfs:comment>
    <rdfs:label>definition_OwnedAllocation</rdfs:label>
  </rdf:Property>
  <rdf:Property rdf:about="http://open-services.net/ns/sysmlv2#stateDefinition_EntryAction">
    <rdfs:isDefinedBy rdf:resource="http://open-services.net/ns/sysmlv2#"/>
    <rdfs:comment>The ActionUsage of this StateDefinition to be performed on entry to the state defined by the StateDefinition. It is the owned ActionUsage related to the StateDefinition by a StateSubactionMembership  with kind = entry.</rdfs:comment>
    <rdfs:label>stateDefinition_EntryAction</rdfs:label>
  </rdf:Property>
  <rdf:Property rdf:about="http://open-services.net/ns/sysmlv2#viewRenderingMembership_OwnedRendering">
    <rdfs:isDefinedBy rdf:resource="http://open-services.net/ns/sysmlv2#"/>
    <rdfs:comment>The owned RenderingUsage that is either itself the referencedRendering or subsets the referencedRendering.</rdfs:comment>
    <rdfs:label>viewRenderingMembership_OwnedRendering</rdfs:label>
  </rdf:Property>
  <rdf:Property rdf:about="http://open-services.net/ns/sysmlv2#definition_OwnedInterface">
    <rdfs:isDefinedBy rdf:resource="http://open-services.net/ns/sysmlv2#"/>
    <rdfs:comment>The InterfaceUsages that are ownedUsages of this Definition.</rdfs:comment>
    <rdfs:label>definition_OwnedInterface</rdfs:label>
  </rdf:Property>
  <rdf:Property rdf:about="http://open-services.net/ns/sysmlv2#viewpointDefinition_ViewpointStakeholder">
    <rdfs:isDefinedBy rdf:resource="http://open-services.net/ns/sysmlv2#"/>
    <rdfs:comment>The PartUsages that identify the stakeholders with concerns framed by this ViewpointDefinition, which are the owned and inherited stakeholderParameters of the framedConcerns of this ViewpointDefinition.</rdfs:comment>
    <rdfs:label>viewpointDefinition_ViewpointStakeholder</rdfs:label>
  </rdf:Property>
  <rdf:Property rdf:about="http://open-services.net/ns/sysmlv2#definition_OwnedCalculation">
    <rdfs:isDefinedBy rdf:resource="http://open-services.net/ns/sysmlv2#"/>
    <rdfs:comment>The CalculationUsages that are ownedUsages of this Definition.</rdfs:comment>
    <rdfs:label>definition_OwnedCalculation</rdfs:label>
  </rdf:Property>
  <rdf:Property rdf:about="http://open-services.net/ns/sysmlv2#behavior_Parameter">
    <rdfs:isDefinedBy rdf:resource="http://open-services.net/ns/sysmlv2#"/>
    <rdfs:comment>The parameters of this Behavior, which are defined as its directedFeatures, whose values are passed into and/or out of a performance of the Behavior.</rdfs:comment>
    <rdfs:label>behavior_Parameter</rdfs:label>
  </rdf:Property>
  <rdf:Property rdf:about="http://open-services.net/ns/sysmlv2#usage_NestedView">
    <rdfs:isDefinedBy rdf:resource="http://open-services.net/ns/sysmlv2#"/>
    <rdfs:comment>The ViewUsages that are nestedUsages of this Usage.</rdfs:comment>
    <rdfs:label>usage_NestedView</rdfs:label>
  </rdf:Property>
  <rdf:Property rdf:about="http://open-services.net/ns/sysmlv2#element_IsImpliedIncluded">
    <rdfs:isDefinedBy rdf:resource="http://open-services.net/ns/sysmlv2#"/>
    <rdfs:comment>Whether all necessary implied Relationships have been included in the ownedRelationships of this Element. This property may be true, even if there are not actually any ownedRelationships with isImplied = true, meaning that no such Relationships are actually implied for this Element. However, if it is false, then ownedRelationships may not contain any implied Relationships. That is, either all required implied Relationships must be included, or none of them.</rdfs:comment>
    <rdfs:label>element_IsImpliedIncluded</rdfs:label>
  </rdf:Property>
  <rdf:Property rdf:about="http://open-services.net/ns/sysmlv2#definition_OwnedViewpoint">
    <rdfs:isDefinedBy rdf:resource="http://open-services.net/ns/sysmlv2#"/>
    <rdfs:comment>The ViewpointUsages that are ownedUsages of this Definition.</rdfs:comment>
    <rdfs:label>definition_OwnedViewpoint</rdfs:label>
  </rdf:Property>
  <rdf:Property rdf:about="http://open-services.net/ns/sysmlv2#transitionUsage_EffectAction">
    <rdfs:isDefinedBy rdf:resource="http://open-services.net/ns/sysmlv2#"/>
    <rdfs:comment>The ActionUsages that define the effects of this TransitionUsage, which are the ownedFeatures of the TransitionUsage related to it by TransitionFeatureMemberships with kind = effect, which must all be ActionUsages.</rdfs:comment>
    <rdfs:label>transitionUsage_EffectAction</rdfs:label>
  </rdf:Property>
  <rdf:Property rdf:about="http://open-services.net/ns/sysmlv2#import_Visibility">
    <rdfs:isDefinedBy rdf:resource="http://open-services.net/ns/sysmlv2#"/>
    <rdfs:comment>The visibility level of the imported members from this Import relative to the importOwningNamespace.</rdfs:comment>
    <rdfs:label>import_Visibility</rdfs:label>
  </rdf:Property>
  <rdf:Property rdf:about="http://open-services.net/ns/sysmlv2#intersecting_TypeIntersected">
    <rdfs:isDefinedBy rdf:resource="http://open-services.net/ns/sysmlv2#"/>
    <rdfs:comment>Type with interpretations partly determined by intersectingType, as described in Type::intersectingType.</rdfs:comment>
    <rdfs:label>intersecting_TypeIntersected</rdfs:label>
  </rdf:Property>
  <rdf:Property rdf:about="http://open-services.net/ns/sysmlv2#multiplicityRange_Bound">
    <rdfs:isDefinedBy rdf:resource="http://open-services.net/ns/sysmlv2#"/>
    <rdfs:comment>The owned Expressions of the MultiplicityRange whose results provide its bounds. These must be the only ownedMembers of the MultiplicityRange.</rdfs:comment>
    <rdfs:label>multiplicityRange_Bound</rdfs:label>
  </rdf:Property>
  <rdf:Property rdf:about="http://open-services.net/ns/sysmlv2#element_Owner">
    <rdfs:isDefinedBy rdf:resource="http://open-services.net/ns/sysmlv2#"/>
    <rdfs:comment>The owner of this Element, derived as the owningRelatedElement of the owningRelationship of this Element, if any.</rdfs:comment>
    <rdfs:label>element_Owner</rdfs:label>
  </rdf:Property>
  <rdf:Property rdf:about="http://open-services.net/ns/sysmlv2#type_OwnedEndFeature">
    <rdfs:isDefinedBy rdf:resource="http://open-services.net/ns/sysmlv2#"/>
    <rdfs:comment>All endFeatures of this Type that are ownedFeatures.</rdfs:comment>
    <rdfs:label>type_OwnedEndFeature</rdfs:label>
  </rdf:Property>
  <rdf:Property rdf:about="http://open-services.net/ns/sysmlv2#feature_IsComposite">
    <rdfs:isDefinedBy rdf:resource="http://open-services.net/ns/sysmlv2#"/>
    <rdfs:comment>Whether the Feature is a composite feature of its featuringType. If so, the values of the Feature cannot exist after its featuring instance no longer does.</rdfs:comment>
    <rdfs:label>feature_IsComposite</rdfs:label>
  </rdf:Property>
  <rdf:Property rdf:about="http://open-services.net/ns/sysmlv2#namespace_ImportedMembership">
    <rdfs:isDefinedBy rdf:resource="http://open-services.net/ns/sysmlv2#"/>
    <rdfs:comment>The Memberships in this Namespace that result from the ownedImports of this Namespace.</rdfs:comment>
    <rdfs:label>namespace_ImportedMembership</rdfs:label>
  </rdf:Property>
  <rdf:Property rdf:about="http://open-services.net/ns/sysmlv2#featureInverting_InvertingFeature">
    <rdfs:isDefinedBy rdf:resource="http://open-services.net/ns/sysmlv2#"/>
    <rdfs:comment>The Feature that is an inverse of the invertedFeature.</rdfs:comment>
    <rdfs:label>featureInverting_InvertingFeature</rdfs:label>
  </rdf:Property>
  <rdf:Property rdf:about="http://open-services.net/ns/sysmlv2#useCaseUsage_IncludedUseCase">
    <rdfs:isDefinedBy rdf:resource="http://open-services.net/ns/sysmlv2#"/>
    <rdfs:comment>The UseCaseUsages that are included by this UseCaseUse, which are the useCaseIncludeds of the IncludeUseCaseUsages owned by this UseCaseUsage.</rdfs:comment>
    <rdfs:label>useCaseUsage_IncludedUseCase</rdfs:label>
  </rdf:Property>
  <rdf:Property rdf:about="http://open-services.net/ns/sysmlv2#type_OwnedDifferencing">
    <rdfs:isDefinedBy rdf:resource="http://open-services.net/ns/sysmlv2#"/>
    <rdfs:comment>The ownedRelationships of this Type that are Differencings, having this Type as their typeDifferenced.</rdfs:comment>
    <rdfs:label>type_OwnedDifferencing</rdfs:label>
  </rdf:Property>
  <rdf:Property rdf:about="http://open-services.net/ns/sysmlv2#framedConcernMembership_ReferencedConcern">
    <rdfs:isDefinedBy rdf:resource="http://open-services.net/ns/sysmlv2#"/>
    <rdfs:comment> The ConcernUsage that is referenced through this FramedConcernMembership. It is the referencedConstraint of the FramedConcernMembership considered as a RequirementConstraintMembership, which must be a ConcernUsage.</rdfs:comment>
    <rdfs:label>framedConcernMembership_ReferencedConcern</rdfs:label>
  </rdf:Property>
  <rdf:Property rdf:about="http://open-services.net/ns/sysmlv2#forLoopActionUsage_SeqArgument">
    <rdfs:isDefinedBy rdf:resource="http://open-services.net/ns/sysmlv2#"/>
    <rdfs:comment>The Expression whose result provides the sequence of values to which the loopVariable is set for each iterative performance of the bodyAction. It is the Expression whose result is bound to the seq input parameter of this ForLoopActionUsage.</rdfs:comment>
    <rdfs:label>forLoopActionUsage_SeqArgument</rdfs:label>
  </rdf:Property>
  <rdf:Property rdf:about="http://open-services.net/ns/sysmlv2#conjugatedPortDefinition_OwnedPortConjugator">
    <rdfs:isDefinedBy rdf:resource="http://open-services.net/ns/sysmlv2#"/>
    <rdfs:comment>The PortConjugation that is the ownedConjugator of this ConjugatedPortDefinition, linking it to its originalPortDefinition.</rdfs:comment>
    <rdfs:label>conjugatedPortDefinition_OwnedPortConjugator</rdfs:label>
  </rdf:Property>
  <rdf:Property rdf:about="http://open-services.net/ns/sysmlv2#element_OwningMembership">
    <rdfs:isDefinedBy rdf:resource="http://open-services.net/ns/sysmlv2#"/>
    <rdfs:comment>The owningRelationship of this Element, if that Relationship is a Membership.</rdfs:comment>
    <rdfs:label>element_OwningMembership</rdfs:label>
  </rdf:Property>
  <rdf:Property rdf:about="http://open-services.net/ns/sysmlv2#element_Documentation">
    <rdfs:isDefinedBy rdf:resource="http://open-services.net/ns/sysmlv2#"/>
    <rdfs:comment>The Documentation owned by this Element.</rdfs:comment>
    <rdfs:label>element_Documentation</rdfs:label>
  </rdf:Property>
  <rdf:Property rdf:about="http://open-services.net/ns/sysmlv2#relationship_OwningRelatedElement">
    <rdfs:isDefinedBy rdf:resource="http://open-services.net/ns/sysmlv2#"/>
    <rdfs:comment>The relatedElement of this Relationship that owns the Relationship, if any.</rdfs:comment>
    <rdfs:label>relationship_OwningRelatedElement</rdfs:label>
  </rdf:Property>
  <rdf:Property rdf:about="http://open-services.net/ns/sysmlv2#stateDefinition_IsParallel">
    <rdfs:isDefinedBy rdf:resource="http://open-services.net/ns/sysmlv2#"/>
    <rdfs:comment>Whether the ownedStates of this StateDefinition are to all be performed in parallel. If true, none of the ownedActions (which includes ownedStates) may have any incoming or outgoing Transitions. If false, only one ownedState may be performed at a time.</rdfs:comment>
    <rdfs:label>stateDefinition_IsParallel</rdfs:label>
  </rdf:Property>
  <rdf:Property rdf:about="http://open-services.net/ns/sysmlv2#type_EndFeature">
    <rdfs:isDefinedBy rdf:resource="http://open-services.net/ns/sysmlv2#"/>
    <rdfs:comment>All features of this Type with isEnd = true.</rdfs:comment>
    <rdfs:label>type_EndFeature</rdfs:label>
  </rdf:Property>
  <rdf:Property rdf:about="http://open-services.net/ns/sysmlv2#expression_Result">
    <rdfs:isDefinedBy rdf:resource="http://open-services.net/ns/sysmlv2#"/>
    <rdfs:comment>result.</rdfs:comment>
    <rdfs:label>expression_Result</rdfs:label>
  </rdf:Property>
  <rdf:Property rdf:about="http://open-services.net/ns/sysmlv2#element_TextualRepresentation">
    <rdfs:isDefinedBy rdf:resource="http://open-services.net/ns/sysmlv2#"/>
    <rdfs:comment>The TextualRepresentations that annotate this Element.</rdfs:comment>
    <rdfs:label>element_TextualRepresentation</rdfs:label>
  </rdf:Property>
  <rdf:Property rdf:about="http://open-services.net/ns/sysmlv2#feature_OwningType">
    <rdfs:isDefinedBy rdf:resource="http://open-services.net/ns/sysmlv2#"/>
    <rdfs:comment>The Type that is the owningType of the owningFeatureMembership of this Feature.</rdfs:comment>
    <rdfs:label>feature_OwningType</rdfs:label>
  </rdf:Property>
  <rdf:Property rdf:about="http://open-services.net/ns/sysmlv2#invocationExpression_Operand">
    <rdfs:isDefinedBy rdf:resource="http://open-services.net/ns/sysmlv2#"/>
    <rdfs:comment>operand.</rdfs:comment>
    <rdfs:label>invocationExpression_Operand</rdfs:label>
  </rdf:Property>
  <rdf:Property rdf:about="http://open-services.net/ns/sysmlv2#expression_IsModelLevelEvaluable">
    <rdfs:isDefinedBy rdf:resource="http://open-services.net/ns/sysmlv2#"/>
    <rdfs:comment>Whether this Expression meets the constraints necessary to be evaluated at model level, that is, using metadata within the model.</rdfs:comment>
    <rdfs:label>expression_IsModelLevelEvaluable</rdfs:label>
  </rdf:Property>
  <rdf:Property rdf:about="http://open-services.net/ns/sysmlv2#literalInteger_Value">
    <rdfs:isDefinedBy rdf:resource="http://open-services.net/ns/sysmlv2#"/>
    <rdfs:comment>The Integer value that is the result of evaluating this LiteralInteger.</rdfs:comment>
    <rdfs:label>literalInteger_Value</rdfs:label>
  </rdf:Property>
  <rdf:Property rdf:about="http://open-services.net/ns/sysmlv2#type_DirectedFeature">
    <rdfs:isDefinedBy rdf:resource="http://open-services.net/ns/sysmlv2#"/>
    <rdfs:comment>The features of this Type that have a non-null direction.</rdfs:comment>
    <rdfs:label>type_DirectedFeature</rdfs:label>
  </rdf:Property>
  <rdf:Property rdf:about="http://open-services.net/ns/sysmlv2#flowConnectionUsage_FlowConnectionDefinition">
    <rdfs:isDefinedBy rdf:resource="http://open-services.net/ns/sysmlv2#"/>
    <rdfs:comment>The Interactions that are the types of this FlowConnectionUsage. Nominally, these are FlowConnectionDefinitions, but other kinds of Kernel Interactions are also allowed, to permit use of Interactions from the Kernel Model Libraries.</rdfs:comment>
    <rdfs:label>flowConnectionUsage_FlowConnectionDefinition</rdfs:label>
  </rdf:Property>
  <rdf:Property rdf:about="http://open-services.net/ns/sysmlv2#literalString_Value">
    <rdfs:isDefinedBy rdf:resource="http://open-services.net/ns/sysmlv2#"/>
    <rdfs:comment>The String value that is the result of evaluating this LiteralString.</rdfs:comment>
    <rdfs:label>literalString_Value</rdfs:label>
  </rdf:Property>
  <rdf:Property rdf:about="http://open-services.net/ns/sysmlv2#transitionUsage_TriggerAction">
    <rdfs:isDefinedBy rdf:resource="http://open-services.net/ns/sysmlv2#"/>
    <rdfs:comment>The AcceptActionUsages that define the triggers of this TransitionUsage, which are the ownedFeatures of the TransitionUsage related to it by TransitionFeatureMemberships with kind = trigger, which must all be AcceptActionUsages.</rdfs:comment>
    <rdfs:label>transitionUsage_TriggerAction</rdfs:label>
  </rdf:Property>
  <rdf:Property rdf:about="http://open-services.net/ns/sysmlv2#stateUsage_EntryAction">
    <rdfs:isDefinedBy rdf:resource="http://open-services.net/ns/sysmlv2#"/>
    <rdfs:comment>The ActionUsage of this StateUsage to be performed on entry to the state defined by the StateDefinition. It is the owned ActionUsage related to the StateUsage by a StateSubactionMembership  with kind = entry.</rdfs:comment>
    <rdfs:label>stateUsage_EntryAction</rdfs:label>
  </rdf:Property>
  <rdf:Property rdf:about="http://open-services.net/ns/sysmlv2#redefinition_RedefiningFeature">
    <rdfs:isDefinedBy rdf:resource="http://open-services.net/ns/sysmlv2#"/>
    <rdfs:comment>The Feature that is redefining the redefinedFeature of this Redefinition.</rdfs:comment>
    <rdfs:label>redefinition_RedefiningFeature</rdfs:label>
  </rdf:Property>
  <rdf:Property rdf:about="http://open-services.net/ns/sysmlv2#dependency_Client">
    <rdfs:isDefinedBy rdf:resource="http://open-services.net/ns/sysmlv2#"/>
    <rdfs:comment>The Element or Elements dependent on the supplier Elements.</rdfs:comment>
    <rdfs:label>dependency_Client</rdfs:label>
  </rdf:Property>
  <rdf:Property rdf:about="http://open-services.net/ns/sysmlv2#featureInverting_FeatureInverted">
    <rdfs:isDefinedBy rdf:resource="http://open-services.net/ns/sysmlv2#"/>
    <rdfs:comment>The Feature that is an inverse of the invertingFeature.</rdfs:comment>
    <rdfs:label>featureInverting_FeatureInverted</rdfs:label>
  </rdf:Property>
  <rdf:Property rdf:about="http://open-services.net/ns/sysmlv2#type_IsAbstract">
    <rdfs:isDefinedBy rdf:resource="http://open-services.net/ns/sysmlv2#"/>
    <rdfs:comment>Indicates whether instances of this Type must also be instances of at least one of its specialized Types.</rdfs:comment>
    <rdfs:label>type_IsAbstract</rdfs:label>
  </rdf:Property>
  <rdf:Property rdf:about="http://open-services.net/ns/sysmlv2#assignmentActionUsage_ValueExpression">
    <rdfs:isDefinedBy rdf:resource="http://open-services.net/ns/sysmlv2#"/>
    <rdfs:comment>The Expression whose result is to be assigned to the referent Feature.</rdfs:comment>
    <rdfs:label>assignmentActionUsage_ValueExpression</rdfs:label>
  </rdf:Property>
  <rdf:Property rdf:about="http://open-services.net/ns/sysmlv2#useCaseUsage_UseCaseDefinition">
    <rdfs:isDefinedBy rdf:resource="http://open-services.net/ns/sysmlv2#"/>
    <rdfs:comment>The UseCaseDefinition that is the definition of this UseCaseUsage.</rdfs:comment>
    <rdfs:label>useCaseUsage_UseCaseDefinition</rdfs:label>
  </rdf:Property>
  <rdf:Property rdf:about="http://open-services.net/ns/sysmlv2#requirementUsage_StakeholderParameter">
    <rdfs:isDefinedBy rdf:resource="http://open-services.net/ns/sysmlv2#"/>
    <rdfs:comment>The parameters of this RequirementUsage that represent stakeholders for the requirement.</rdfs:comment>
    <rdfs:label>requirementUsage_StakeholderParameter</rdfs:label>
  </rdf:Property>
  <rdf:Property rdf:about="http://open-services.net/ns/sysmlv2#unioning_UnioningType">
    <rdfs:isDefinedBy rdf:resource="http://open-services.net/ns/sysmlv2#"/>
    <rdfs:comment>Type that partly determines interpretations of typeUnioned, as described in Type::unioningType.</rdfs:comment>
    <rdfs:label>unioning_UnioningType</rdfs:label>
  </rdf:Property>
  <rdf:Property rdf:about="http://open-services.net/ns/sysmlv2#relationship_OwnedRelatedElement">
    <rdfs:isDefinedBy rdf:resource="http://open-services.net/ns/sysmlv2#"/>
    <rdfs:comment>The relatedElements of this Relationship that are owned by the Relationship.</rdfs:comment>
    <rdfs:label>relationship_OwnedRelatedElement</rdfs:label>
  </rdf:Property>
  <rdf:Property rdf:about="http://open-services.net/ns/sysmlv2#itemFlow_ItemFlowEnd">
    <rdfs:isDefinedBy rdf:resource="http://open-services.net/ns/sysmlv2#"/>
    <rdfs:comment>The connectorEnds of this ItemFlow that are ItemFlowEnds.</rdfs:comment>
    <rdfs:label>itemFlow_ItemFlowEnd</rdfs:label>
  </rdf:Property>
  <rdf:Property rdf:about="http://open-services.net/ns/sysmlv2#type_OwnedConjugator">
    <rdfs:isDefinedBy rdf:resource="http://open-services.net/ns/sysmlv2#"/>
    <rdfs:comment>A Conjugation owned by this Type for which the Type is the originalType.</rdfs:comment>
    <rdfs:label>type_OwnedConjugator</rdfs:label>
  </rdf:Property>
  <rdf:Property rdf:about="http://open-services.net/ns/sysmlv2#libraryPackage_IsStandard">
    <rdfs:isDefinedBy rdf:resource="http://open-services.net/ns/sysmlv2#"/>
    <rdfs:comment>Whether this LibraryPackage contains a standard library model. This should only be set to true for LibraryPackages in the standard Kernel Model Libraries or in normative model libraries for a language built on KerML.</rdfs:comment>
    <rdfs:label>libraryPackage_IsStandard</rdfs:label>
  </rdf:Property>
  <rdf:Property rdf:about="http://open-services.net/ns/sysmlv2#requirementConstraintMembership_Kind">
    <rdfs:isDefinedBy rdf:resource="http://open-services.net/ns/sysmlv2#"/>
    <rdfs:comment>Whether the RequirementConstraintMembership is for an assumed or required ConstraintUsage.</rdfs:comment>
    <rdfs:label>requirementConstraintMembership_Kind</rdfs:label>
  </rdf:Property>
  <rdf:Property rdf:about="http://open-services.net/ns/sysmlv2#typeFeaturing_OwningFeatureOfType">
    <rdfs:isDefinedBy rdf:resource="http://open-services.net/ns/sysmlv2#"/>
    <rdfs:comment>A featureOfType that is also the owningRelatedElement of this TypeFeaturing.</rdfs:comment>
    <rdfs:label>typeFeaturing_OwningFeatureOfType</rdfs:label>
  </rdf:Property>
  <rdf:Property rdf:about="http://open-services.net/ns/sysmlv2#renderingUsage_RenderingDefinition">
    <rdfs:isDefinedBy rdf:resource="http://open-services.net/ns/sysmlv2#"/>
    <rdfs:comment>The RenderingDefinition that is the definition of this RenderingUsage.</rdfs:comment>
    <rdfs:label>renderingUsage_RenderingDefinition</rdfs:label>
  </rdf:Property>
  <rdf:Property rdf:about="http://open-services.net/ns/sysmlv2#caseUsage_SubjectParameter">
    <rdfs:isDefinedBy rdf:resource="http://open-services.net/ns/sysmlv2#"/>
    <rdfs:comment>The parameter of this CaseUsage that represents its subject.</rdfs:comment>
    <rdfs:label>caseUsage_SubjectParameter</rdfs:label>
  </rdf:Property>
  <rdf:Property rdf:about="http://open-services.net/ns/sysmlv2#annotatingElement_AnnotatedElement">
    <rdfs:isDefinedBy rdf:resource="http://open-services.net/ns/sysmlv2#"/>
    <rdfs:comment>The Elements that are annotated by this AnnotatingElement. If annotation is not empty, these are the annotatedElements of the annotations. If annotation is empty, then it is the owningNamespace of the AnnotatingElement.</rdfs:comment>
    <rdfs:label>annotatingElement_AnnotatedElement</rdfs:label>
  </rdf:Property>
  <rdf:Property rdf:about="http://open-services.net/ns/sysmlv2#usage_DirectedUsage">
    <rdfs:isDefinedBy rdf:resource="http://open-services.net/ns/sysmlv2#"/>
    <rdfs:comment>The usages of this Usage that are directedFeatures.</rdfs:comment>
    <rdfs:label>usage_DirectedUsage</rdfs:label>
  </rdf:Property>
  <rdf:Property rdf:about="http://open-services.net/ns/sysmlv2#feature_OwningFeatureMembership">
    <rdfs:isDefinedBy rdf:resource="http://open-services.net/ns/sysmlv2#"/>
    <rdfs:comment>The FeatureMembership that owns this Feature as an ownedMemberFeature, determining its owningType.</rdfs:comment>
    <rdfs:label>feature_OwningFeatureMembership</rdfs:label>
  </rdf:Property>
  <rdf:Property rdf:about="http://open-services.net/ns/sysmlv2#association_TargetType">
    <rdfs:isDefinedBy rdf:resource="http://open-services.net/ns/sysmlv2#"/>
    <rdfs:comment>The target relatedTypes for this Association. This includes all the relatedTypes other than the sourceType.</rdfs:comment>
    <rdfs:label>association_TargetType</rdfs:label>
  </rdf:Property>
  <rdf:Property rdf:about="http://open-services.net/ns/sysmlv2#connectionUsage_ConnectionDefinition">
    <rdfs:isDefinedBy rdf:resource="http://open-services.net/ns/sysmlv2#"/>
    <rdfs:comment>The AssociationStructures that are the types of this ConnectionUsage. Nominally, these are , but other kinds of Kernel AssociationStructures are also allowed, to permit use of AssociationStructures from the Kernel Model Libraries.</rdfs:comment>
    <rdfs:label>connectionUsage_ConnectionDefinition</rdfs:label>
  </rdf:Property>
  <rdf:Property rdf:about="http://open-services.net/ns/sysmlv2#definition_OwnedAttribute">
    <rdfs:isDefinedBy rdf:resource="http://open-services.net/ns/sysmlv2#"/>
    <rdfs:comment>The AttributeUsages that are ownedUsages of this Definition.</rdfs:comment>
    <rdfs:label>definition_OwnedAttribute</rdfs:label>
  </rdf:Property>
  <rdf:Property rdf:about="http://open-services.net/ns/sysmlv2#invariant_IsNegated">
    <rdfs:isDefinedBy rdf:resource="http://open-services.net/ns/sysmlv2#"/>
    <rdfs:comment>Whether this Invariant is asserted to be false rather than true.</rdfs:comment>
    <rdfs:label>invariant_IsNegated</rdfs:label>
  </rdf:Property>
  <rdf:Property rdf:about="http://open-services.net/ns/sysmlv2#type_DifferencingType">
    <rdfs:isDefinedBy rdf:resource="http://open-services.net/ns/sysmlv2#"/>
    <rdfs:comment>The interpretations of a Type with differencingTypes are asserted to be those of the first of those Types, but not including those of the remaining Types. For example, a Classifier might be the difference of a Classifier for people and another for people of a particular nationality, leaving people who are not of that nationality. Similarly, a feature of people might be the difference between a feature for their children and a Classifier for people of a particular sex, identifying their children not of that sex (because the interpretations of the children Feature that identify those of that sex are also interpretations of the Classifier for that sex).</rdfs:comment>
    <rdfs:label>type_DifferencingType</rdfs:label>
  </rdf:Property>
  <rdf:Property rdf:about="http://open-services.net/ns/sysmlv2#feature_Direction">
    <rdfs:isDefinedBy rdf:resource="http://open-services.net/ns/sysmlv2#"/>
    <rdfs:comment>Indicates how values of this Feature are determined or used (as specified for the FeatureDirectionKind).</rdfs:comment>
    <rdfs:label>feature_Direction</rdfs:label>
  </rdf:Property>
  <rdf:Property rdf:about="http://open-services.net/ns/sysmlv2#caseDefinition_ObjectiveRequirement">
    <rdfs:isDefinedBy rdf:resource="http://open-services.net/ns/sysmlv2#"/>
    <rdfs:comment>The RequirementUsage representing the objective of this CaseDefinition.</rdfs:comment>
    <rdfs:label>caseDefinition_ObjectiveRequirement</rdfs:label>
  </rdf:Property>
  <rdf:Property rdf:about="http://open-services.net/ns/sysmlv2#viewUsage_ViewDefinition">
    <rdfs:isDefinedBy rdf:resource="http://open-services.net/ns/sysmlv2#"/>
    <rdfs:comment>The ViewDefinition that is the definition of this ViewUsage.</rdfs:comment>
    <rdfs:label>viewUsage_ViewDefinition</rdfs:label>
  </rdf:Property>
  <rdf:Property rdf:about="http://open-services.net/ns/sysmlv2#invocationExpression_Argument">
    <rdfs:isDefinedBy rdf:resource="http://open-services.net/ns/sysmlv2#"/>
    <rdfs:comment>The value Expressions of the FeatureValues of the owned input parameters of the InvocationExpression.</rdfs:comment>
    <rdfs:label>invocationExpression_Argument</rdfs:label>
  </rdf:Property>
  <rdf:Property rdf:about="http://open-services.net/ns/sysmlv2#definition_OwnedAction">
    <rdfs:isDefinedBy rdf:resource="http://open-services.net/ns/sysmlv2#"/>
    <rdfs:comment>The ActionUsages that are ownedUsages of this Definition.</rdfs:comment>
    <rdfs:label>definition_OwnedAction</rdfs:label>
  </rdf:Property>
  <rdf:Property rdf:about="http://open-services.net/ns/sysmlv2#requirementDefinition_RequiredConstraint">
    <rdfs:isDefinedBy rdf:resource="http://open-services.net/ns/sysmlv2#"/>
    <rdfs:comment>The owned ConstraintUsages that represent requirements of this RequirementDefinition, derived as the ownedConstraints of the RequirementConstraintMemberships of the RequirementDefinition with kind = requirement.</rdfs:comment>
    <rdfs:label>requirementDefinition_RequiredConstraint</rdfs:label>
  </rdf:Property>
  <rdf:Property rdf:about="http://open-services.net/ns/sysmlv2#itemFlow_ItemType">
    <rdfs:isDefinedBy rdf:resource="http://open-services.net/ns/sysmlv2#"/>
    <rdfs:comment>The type of values transferred, which is the type of the itemFeature of the ItemFlow.</rdfs:comment>
    <rdfs:label>itemFlow_ItemType</rdfs:label>
  </rdf:Property>
  <rdf:Property rdf:about="http://open-services.net/ns/sysmlv2#association_AssociationEnd">
    <rdfs:isDefinedBy rdf:resource="http://open-services.net/ns/sysmlv2#"/>
    <rdfs:comment>The features of the Association that identify the things that can be related by it. A concrete Association must have at least two associationEnds. When it has exactly two, the Association is called a binary Association.</rdfs:comment>
    <rdfs:label>association_AssociationEnd</rdfs:label>
  </rdf:Property>
  <rdf:Property rdf:about="http://open-services.net/ns/sysmlv2#element_OwnedRelationship">
    <rdfs:isDefinedBy rdf:resource="http://open-services.net/ns/sysmlv2#"/>
    <rdfs:comment>The Relationships for which this Element is the owningRelatedElement.</rdfs:comment>
    <rdfs:label>element_OwnedRelationship</rdfs:label>
  </rdf:Property>
  <rdf:Property rdf:about="http://open-services.net/ns/sysmlv2#sendActionUsage_PayloadArgument">
    <rdfs:isDefinedBy rdf:resource="http://open-services.net/ns/sysmlv2#"/>
    <rdfs:comment>An Expression whose result is bound to the payload input parameter of this SendActionUsage.</rdfs:comment>
    <rdfs:label>sendActionUsage_PayloadArgument</rdfs:label>
  </rdf:Property>
  <rdf:Property rdf:about="http://open-services.net/ns/sysmlv2#function_IsModelLevelEvaluable">
    <rdfs:isDefinedBy rdf:resource="http://open-services.net/ns/sysmlv2#"/>
    <rdfs:comment>Whether this Function can be used as the function of a model-level evaluable InvocationExpression. Certain Functions from the Kernel Functions Library are considered to have isModelLevelEvaluable = true. For all other Functions it is false.</rdfs:comment>
    <rdfs:label>function_IsModelLevelEvaluable</rdfs:label>
  </rdf:Property>
  <rdf:Property rdf:about="http://open-services.net/ns/sysmlv2#satisfyRequirementUsage_SatisfiedRequirement">
    <rdfs:isDefinedBy rdf:resource="http://open-services.net/ns/sysmlv2#"/>
    <rdfs:comment>The RequirementUsage that is satisfied by the satisfyingSubject of this SatisfyRequirementUsage. It is the assertedConstraint of the SatisfyRequirementUsage considered as an AssertConstraintUsage, which must be a RequirementUsage.</rdfs:comment>
    <rdfs:label>satisfyRequirementUsage_SatisfiedRequirement</rdfs:label>
  </rdf:Property>
  <rdf:Property rdf:about="http://open-services.net/ns/sysmlv2#requirementDefinition_ReqId">
    <rdfs:isDefinedBy rdf:resource="http://open-services.net/ns/sysmlv2#"/>
    <rdfs:comment>An optional modeler-specified identifier for this RequirementDefinition (used, e.g., to link it to an original requirement text in some source document), which is the declaredShortName for the RequirementDefinition.</rdfs:comment>
    <rdfs:label>requirementDefinition_ReqId</rdfs:label>
  </rdf:Property>
  <rdf:Property rdf:about="http://open-services.net/ns/sysmlv2#definition_OwnedRequirement">
    <rdfs:isDefinedBy rdf:resource="http://open-services.net/ns/sysmlv2#"/>
    <rdfs:comment>The RequirementUsages that are ownedUsages of this Definition.</rdfs:comment>
    <rdfs:label>definition_OwnedRequirement</rdfs:label>
  </rdf:Property>
  <rdf:Property rdf:about="http://open-services.net/ns/sysmlv2#feature_OwnedFeatureChaining">
    <rdfs:isDefinedBy rdf:resource="http://open-services.net/ns/sysmlv2#"/>
    <rdfs:comment>The ownedRelationships of this Feature that are FeatureChainings, for which the Feature will be the featureChained.</rdfs:comment>
    <rdfs:label>feature_OwnedFeatureChaining</rdfs:label>
  </rdf:Property>
  <rdf:Property rdf:about="http://open-services.net/ns/sysmlv2#usage_NestedVerificationCase">
    <rdfs:isDefinedBy rdf:resource="http://open-services.net/ns/sysmlv2#"/>
    <rdfs:comment>The VerificationCaseUsages that are nestedUsages of this Usage.</rdfs:comment>
    <rdfs:label>usage_NestedVerificationCase</rdfs:label>
  </rdf:Property>
  <rdf:Property rdf:about="http://open-services.net/ns/sysmlv2#owningMembership_OwnedMemberName">
    <rdfs:isDefinedBy rdf:resource="http://open-services.net/ns/sysmlv2#"/>
    <rdfs:comment>The name of the ownedMemberElement.</rdfs:comment>
    <rdfs:label>owningMembership_OwnedMemberName</rdfs:label>
  </rdf:Property>
  <rdf:Property rdf:about="http://open-services.net/ns/sysmlv2#viewUsage_ViewCondition">
    <rdfs:isDefinedBy rdf:resource="http://open-services.net/ns/sysmlv2#"/>
    <rdfs:comment>The Expressions related to this ViewUsage by ElementFilterMemberships, which specify conditions on Elements to be rendered in a view.</rdfs:comment>
    <rdfs:label>viewUsage_ViewCondition</rdfs:label>
  </rdf:Property>
  <rdf:Property rdf:about="http://open-services.net/ns/sysmlv2#requirementDefinition_StakeholderParameter">
    <rdfs:isDefinedBy rdf:resource="http://open-services.net/ns/sysmlv2#"/>
    <rdfs:comment>The parameters of this RequirementDefinition that represent stakeholders for th requirement.</rdfs:comment>
    <rdfs:label>requirementDefinition_StakeholderParameter</rdfs:label>
  </rdf:Property>
  <rdf:Property rdf:about="http://open-services.net/ns/sysmlv2#usage_NestedState">
    <rdfs:isDefinedBy rdf:resource="http://open-services.net/ns/sysmlv2#"/>
    <rdfs:comment>The StateUsages that are nestedUsages of this Usage.</rdfs:comment>
    <rdfs:label>usage_NestedState</rdfs:label>
  </rdf:Property>
  <rdf:Property rdf:about="http://open-services.net/ns/sysmlv2#feature_OwnedFeatureInverting">
    <rdfs:isDefinedBy rdf:resource="http://open-services.net/ns/sysmlv2#"/>
    <rdfs:comment>The ownedRelationships of this Feature that are FeatureInvertings and for which the Feature is the featureInverted.</rdfs:comment>
    <rdfs:label>feature_OwnedFeatureInverting</rdfs:label>
  </rdf:Property>
  <rdf:Property rdf:about="http://open-services.net/ns/sysmlv2#usage_NestedRendering">
    <rdfs:isDefinedBy rdf:resource="http://open-services.net/ns/sysmlv2#"/>
    <rdfs:comment>The RenderingUsages that are nestedUsages of this Usage.</rdfs:comment>
    <rdfs:label>usage_NestedRendering</rdfs:label>
  </rdf:Property>
  <rdf:Property rdf:about="http://open-services.net/ns/sysmlv2#featureTyping_TypedFeature">
    <rdfs:isDefinedBy rdf:resource="http://open-services.net/ns/sysmlv2#"/>
    <rdfs:comment>The Feature that has a type determined by this FeatureTyping.</rdfs:comment>
    <rdfs:label>featureTyping_TypedFeature</rdfs:label>
  </rdf:Property>
  <rdf:Property rdf:about="http://open-services.net/ns/sysmlv2#stateDefinition_State">
    <rdfs:isDefinedBy rdf:resource="http://open-services.net/ns/sysmlv2#"/>
    <rdfs:comment>The StateUsages, which are actions in the StateDefinition, that specify the discrete states in the behavior defined by the StateDefinition.</rdfs:comment>
    <rdfs:label>stateDefinition_State</rdfs:label>
  </rdf:Property>
  <rdf:Property rdf:about="http://open-services.net/ns/sysmlv2#subsetting_OwningFeature">
    <rdfs:isDefinedBy rdf:resource="http://open-services.net/ns/sysmlv2#"/>
    <rdfs:comment>A subsettingFeature that is also the owningRelatedElement of this Subsetting.</rdfs:comment>
    <rdfs:label>subsetting_OwningFeature</rdfs:label>
  </rdf:Property>
  <rdf:Property rdf:about="http://open-services.net/ns/sysmlv2#function_Expression">
    <rdfs:isDefinedBy rdf:resource="http://open-services.net/ns/sysmlv2#"/>
    <rdfs:comment>The Expressions that are steps in the calculation of the result of this Function.</rdfs:comment>
    <rdfs:label>function_Expression</rdfs:label>
  </rdf:Property>
  <rdf:Property rdf:about="http://open-services.net/ns/sysmlv2#requirementDefinition_FramedConcern">
    <rdfs:isDefinedBy rdf:resource="http://open-services.net/ns/sysmlv2#"/>
    <rdfs:comment>The ConcernUsages framed by this RequirementDefinition, which are the ownedConcerns of all FramedConcernMemberships of the RequirementDefinition.</rdfs:comment>
    <rdfs:label>requirementDefinition_FramedConcern</rdfs:label>
  </rdf:Property>
  <rdf:Property rdf:about="http://open-services.net/ns/sysmlv2#feature_IsNonunique">
    <rdfs:isDefinedBy rdf:resource="http://open-services.net/ns/sysmlv2#"/>
    <rdfs:comment>isNonunique.</rdfs:comment>
    <rdfs:label>feature_IsNonunique</rdfs:label>
  </rdf:Property>
  <rdf:Property rdf:about="http://open-services.net/ns/sysmlv2#usage_NestedUsage">
    <rdfs:isDefinedBy rdf:resource="http://open-services.net/ns/sysmlv2#"/>
    <rdfs:comment>The Usages that are ownedFeatures of this Usage.</rdfs:comment>
    <rdfs:label>usage_NestedUsage</rdfs:label>
  </rdf:Property>
  <rdf:Property rdf:about="http://open-services.net/ns/sysmlv2#elementFilterMembership_Condition">
    <rdfs:isDefinedBy rdf:resource="http://open-services.net/ns/sysmlv2#"/>
    <rdfs:comment>The model-level evaluable Boolean-valued Expression used to filter the imported members of the membershipOwningNamespace of this ElementFilterMembership.</rdfs:comment>
    <rdfs:label>elementFilterMembership_Condition</rdfs:label>
  </rdf:Property>
  <rdf:Property rdf:about="http://open-services.net/ns/sysmlv2#usage_NestedReference">
    <rdfs:isDefinedBy rdf:resource="http://open-services.net/ns/sysmlv2#"/>
    <rdfs:comment>The ReferenceUsages that are nestedUsages of this Usage.</rdfs:comment>
    <rdfs:label>usage_NestedReference</rdfs:label>
  </rdf:Property>
  <rdf:Property rdf:about="http://open-services.net/ns/sysmlv2#featureChaining_ChainingFeature">
    <rdfs:isDefinedBy rdf:resource="http://open-services.net/ns/sysmlv2#"/>
    <rdfs:comment>The Feature whose values partly determine values of featureChained, as described in Feature::chainingFeature.</rdfs:comment>
    <rdfs:label>featureChaining_ChainingFeature</rdfs:label>
  </rdf:Property>
  <rdf:Property rdf:about="http://open-services.net/ns/sysmlv2#featureMembership_OwnedMemberFeature">
    <rdfs:isDefinedBy rdf:resource="http://open-services.net/ns/sysmlv2#"/>
    <rdfs:comment>The Feature that this FeatureMembership relates to its owningType, making it an ownedFeature of the owningType.</rdfs:comment>
    <rdfs:label>featureMembership_OwnedMemberFeature</rdfs:label>
  </rdf:Property>
  <rdf:Property rdf:about="http://open-services.net/ns/sysmlv2#feature_IsEnd">
    <rdfs:isDefinedBy rdf:resource="http://open-services.net/ns/sysmlv2#"/>
    <rdfs:comment>Whether or not the this Feature is an end Feature, requiring a different interpretation of the multiplicity of the Feature.</rdfs:comment>
    <rdfs:label>feature_IsEnd</rdfs:label>
  </rdf:Property>
  <rdf:Property rdf:about="http://open-services.net/ns/sysmlv2#portDefinition_ConjugatedPortDefinition">
    <rdfs:isDefinedBy rdf:resource="http://open-services.net/ns/sysmlv2#"/>
    <rdfs:comment>The  that is conjugate to this PortDefinition.</rdfs:comment>
    <rdfs:label>portDefinition_ConjugatedPortDefinition</rdfs:label>
  </rdf:Property>
  <rdf:Property rdf:about="http://open-services.net/ns/sysmlv2#function_Result">
    <rdfs:isDefinedBy rdf:resource="http://open-services.net/ns/sysmlv2#"/>
    <rdfs:comment>The result parameter of the Function, which is owned by the Function via a ReturnParameterMembership.</rdfs:comment>
    <rdfs:label>function_Result</rdfs:label>
  </rdf:Property>
  <rdf:Property rdf:about="http://open-services.net/ns/sysmlv2#stateUsage_DoAction">
    <rdfs:isDefinedBy rdf:resource="http://open-services.net/ns/sysmlv2#"/>
    <rdfs:comment>The ActionUsage of this StateUsage to be performed while in the state defined by the StateDefinition. It is the owned ActionUsage related to the StateUsage by a StateSubactionMembership  with kind = do.</rdfs:comment>
    <rdfs:label>stateUsage_DoAction</rdfs:label>
  </rdf:Property>
  <rdf:Property rdf:about="http://open-services.net/ns/sysmlv2#assignmentActionUsage_Referent">
    <rdfs:isDefinedBy rdf:resource="http://open-services.net/ns/sysmlv2#"/>
    <rdfs:comment>The Feature whose value is to be set.</rdfs:comment>
    <rdfs:label>assignmentActionUsage_Referent</rdfs:label>
  </rdf:Property>
  <rdf:Property rdf:about="http://open-services.net/ns/sysmlv2#metadataFeature_Metaclass">
    <rdfs:isDefinedBy rdf:resource="http://open-services.net/ns/sysmlv2#"/>
    <rdfs:comment>The type of this MetadataFeature, which must be a Metaclass.</rdfs:comment>
    <rdfs:label>metadataFeature_Metaclass</rdfs:label>
  </rdf:Property>
  <rdf:Property rdf:about="http://open-services.net/ns/sysmlv2#concernUsage_ConcernDefinition">
    <rdfs:isDefinedBy rdf:resource="http://open-services.net/ns/sysmlv2#"/>
    <rdfs:comment>The ConcernDefinition that is the single type of this ConcernUsage.</rdfs:comment>
    <rdfs:label>concernUsage_ConcernDefinition</rdfs:label>
  </rdf:Property>
  <rdf:Property rdf:about="http://open-services.net/ns/sysmlv2#usage_NestedOccurrence">
    <rdfs:isDefinedBy rdf:resource="http://open-services.net/ns/sysmlv2#"/>
    <rdfs:comment>The OccurrenceUsages that are nestedUsages of this Usage.</rdfs:comment>
    <rdfs:label>usage_NestedOccurrence</rdfs:label>
  </rdf:Property>
  <rdf:Property rdf:about="http://open-services.net/ns/sysmlv2#succession_EffectStep">
    <rdfs:isDefinedBy rdf:resource="http://open-services.net/ns/sysmlv2#"/>
    <rdfs:comment>Steps that represent occurrences that are side effects of the transitionStep occurring.</rdfs:comment>
    <rdfs:label>succession_EffectStep</rdfs:label>
  </rdf:Property>
  <rdf:Property rdf:about="http://open-services.net/ns/sysmlv2#feature_OwnedSubsetting">
    <rdfs:isDefinedBy rdf:resource="http://open-services.net/ns/sysmlv2#"/>
    <rdfs:comment>The ownedSpecializations of this Feature that are Subsettings, for which the Feature is the subsettingFeature.</rdfs:comment>
    <rdfs:label>feature_OwnedSubsetting</rdfs:label>
  </rdf:Property>
  <rdf:Property rdf:about="http://open-services.net/ns/sysmlv2#requirementUsage_AssumedConstraint">
    <rdfs:isDefinedBy rdf:resource="http://open-services.net/ns/sysmlv2#"/>
    <rdfs:comment>The owned ConstraintUsages that represent assumptions of this RequirementUsage, derived as the ownedConstraints of the RequirementConstraintMemberships of the RequirementUsage with kind = assumption.</rdfs:comment>
    <rdfs:label>requirementUsage_AssumedConstraint</rdfs:label>
  </rdf:Property>
  <rdf:Property rdf:about="http://open-services.net/ns/sysmlv2#definition_OwnedView">
    <rdfs:isDefinedBy rdf:resource="http://open-services.net/ns/sysmlv2#"/>
    <rdfs:comment>The ViewUsages that are ownedUsages of this Definition.</rdfs:comment>
    <rdfs:label>definition_OwnedView</rdfs:label>
  </rdf:Property>
  <rdf:Property rdf:about="http://open-services.net/ns/sysmlv2#itemUsage_ItemDefinition">
    <rdfs:isDefinedBy rdf:resource="http://open-services.net/ns/sysmlv2#"/>
    <rdfs:comment>The Structures that are the definitions of this ItemUsage. Nominally, these are ItemDefinitions, but other kinds of Kernel Structures are also allowed, to permit use of Structures from the Kernel Library.</rdfs:comment>
    <rdfs:label>itemUsage_ItemDefinition</rdfs:label>
  </rdf:Property>
  <rdf:Property rdf:about="http://open-services.net/ns/sysmlv2#featureValue_IsDefault">
    <rdfs:isDefinedBy rdf:resource="http://open-services.net/ns/sysmlv2#"/>
    <rdfs:comment>Whether this FeatureValue is a concrete specification of the bound or initial value of the featureWithValue, or just a default value that may be overridden.</rdfs:comment>
    <rdfs:label>featureValue_IsDefault</rdfs:label>
  </rdf:Property>
  <rdf:Property rdf:about="http://open-services.net/ns/sysmlv2#type_Output">
    <rdfs:isDefinedBy rdf:resource="http://open-services.net/ns/sysmlv2#"/>
    <rdfs:comment>All features related to this Type by FeatureMemberships that have direction out or inout.</rdfs:comment>
    <rdfs:label>type_Output</rdfs:label>
  </rdf:Property>
  <rdf:Property rdf:about="http://open-services.net/ns/sysmlv2#import_IsImportAll">
    <rdfs:isDefinedBy rdf:resource="http://open-services.net/ns/sysmlv2#"/>
    <rdfs:comment>Whether to import memberships without regard to declared visibility.</rdfs:comment>
    <rdfs:label>import_IsImportAll</rdfs:label>
  </rdf:Property>
  <rdf:Property rdf:about="http://open-services.net/ns/sysmlv2#annotation_AnnotatedElement">
    <rdfs:isDefinedBy rdf:resource="http://open-services.net/ns/sysmlv2#"/>
    <rdfs:comment>The Element that is annotated by the annotatingElement of this Annotation.</rdfs:comment>
    <rdfs:label>annotation_AnnotatedElement</rdfs:label>
  </rdf:Property>
  <rdf:Property rdf:about="http://open-services.net/ns/sysmlv2#sendActionUsage_SenderArgument">
    <rdfs:isDefinedBy rdf:resource="http://open-services.net/ns/sysmlv2#"/>
    <rdfs:comment>An Expression whose result is bound to the sender input parameter of this SendActionUsage.</rdfs:comment>
    <rdfs:label>sendActionUsage_SenderArgument</rdfs:label>
  </rdf:Property>
  <rdf:Property rdf:about="http://open-services.net/ns/sysmlv2#metadataUsage_MetadataDefinition">
    <rdfs:isDefinedBy rdf:resource="http://open-services.net/ns/sysmlv2#"/>
    <rdfs:comment>The MetadataDefinition that is the definition of this MetadataUsage.</rdfs:comment>
    <rdfs:label>metadataUsage_MetadataDefinition</rdfs:label>
  </rdf:Property>
  <rdf:Property rdf:about="http://open-services.net/ns/sysmlv2#forLoopActionUsage_LoopVariable">
    <rdfs:isDefinedBy rdf:resource="http://open-services.net/ns/sysmlv2#"/>
    <rdfs:comment>The ownedFeature of this ForLoopActionUsage that acts as the loop variable, which is assigned the successive values of the input sequence on each iteration. It is the ownedFeature that redefines ForLoopAction::var.</rdfs:comment>
    <rdfs:label>forLoopActionUsage_LoopVariable</rdfs:label>
  </rdf:Property>
  <rdf:Property rdf:about="http://open-services.net/ns/sysmlv2#requirementVerificationMembership_VerifiedRequirement">
    <rdfs:isDefinedBy rdf:resource="http://open-services.net/ns/sysmlv2#"/>
    <rdfs:comment> The RequirementUsage that is identified as being verified. It is the referencedConstraint of the RequirementVerificationMembership considered as a RequirementConstraintMembership, which must be a RequirementUsage.</rdfs:comment>
    <rdfs:label>requirementVerificationMembership_VerifiedRequirement</rdfs:label>
  </rdf:Property>
  <rdf:Property rdf:about="http://open-services.net/ns/sysmlv2#definition_OwnedUsage">
    <rdfs:isDefinedBy rdf:resource="http://open-services.net/ns/sysmlv2#"/>
    <rdfs:comment>The Usages that are ownedFeatures of this Definition.</rdfs:comment>
    <rdfs:label>definition_OwnedUsage</rdfs:label>
  </rdf:Property>
  <rdf:Property rdf:about="http://open-services.net/ns/sysmlv2#feature_IsOrdered">
    <rdfs:isDefinedBy rdf:resource="http://open-services.net/ns/sysmlv2#"/>
    <rdfs:comment>Whether an order exists for the values of this Feature or not.</rdfs:comment>
    <rdfs:label>feature_IsOrdered</rdfs:label>
  </rdf:Property>
  <rdf:Property rdf:about="http://open-services.net/ns/sysmlv2#namespace_OwnedMembership">
    <rdfs:isDefinedBy rdf:resource="http://open-services.net/ns/sysmlv2#"/>
    <rdfs:comment>The ownedRelationships of this Namespace that are Memberships, for which the Namespace is the membershipOwningNamespace.</rdfs:comment>
    <rdfs:label>namespace_OwnedMembership</rdfs:label>
  </rdf:Property>
  <rdf:Property rdf:about="http://open-services.net/ns/sysmlv2#transitionFeatureMembership_TransitionFeature">
    <rdfs:isDefinedBy rdf:resource="http://open-services.net/ns/sysmlv2#"/>
    <rdfs:comment>The Step that is the ownedMemberFeature of this TransitionFeatureMembership.</rdfs:comment>
    <rdfs:label>transitionFeatureMembership_TransitionFeature</rdfs:label>
  </rdf:Property>
  <rdf:Property rdf:about="http://open-services.net/ns/sysmlv2#definition_OwnedItem">
    <rdfs:isDefinedBy rdf:resource="http://open-services.net/ns/sysmlv2#"/>
    <rdfs:comment>The ItemUsages that are ownedUsages of this Definition.</rdfs:comment>
    <rdfs:label>definition_OwnedItem</rdfs:label>
  </rdf:Property>
  <rdf:Property rdf:about="http://open-services.net/ns/sysmlv2#definition_VariantMembership">
    <rdfs:isDefinedBy rdf:resource="http://open-services.net/ns/sysmlv2#"/>
    <rdfs:comment>The ownedMemberships of this Definition that are VariantMemberships. If isVariation = true, then this must be all ownedMemberships of the Definition. If isVariation = false, then variantMembershipmust be empty.</rdfs:comment>
    <rdfs:label>definition_VariantMembership</rdfs:label>
  </rdf:Property>
  <rdf:Property rdf:about="http://open-services.net/ns/sysmlv2#usage_VariantMembership">
    <rdfs:isDefinedBy rdf:resource="http://open-services.net/ns/sysmlv2#"/>
    <rdfs:comment>The ownedMemberships of this Usage that are VariantMemberships. If isVariation = true, then this must be all memberships of the Usage. If isVariation = false, then variantMembershipmust be empty.</rdfs:comment>
    <rdfs:label>usage_VariantMembership</rdfs:label>
  </rdf:Property>
  <rdf:Property rdf:about="http://open-services.net/ns/sysmlv2#triggerInvocationExpression_Kind">
    <rdfs:isDefinedBy rdf:resource="http://open-services.net/ns/sysmlv2#"/>
    <rdfs:comment>Indicates which of the Functions from the Triggers model in the Kernel Semantic Library is to be invoked by this TriggerInvocationExpression.</rdfs:comment>
    <rdfs:label>triggerInvocationExpression_Kind</rdfs:label>
  </rdf:Property>
  <rdf:Property rdf:about="http://open-services.net/ns/sysmlv2#caseDefinition_SubjectParameter">
    <rdfs:isDefinedBy rdf:resource="http://open-services.net/ns/sysmlv2#"/>
    <rdfs:comment>The parameter of this CaseDefinition that represents its subject.</rdfs:comment>
    <rdfs:label>caseDefinition_SubjectParameter</rdfs:label>
  </rdf:Property>
  <rdf:Property rdf:about="http://open-services.net/ns/sysmlv2#definition_OwnedOccurrence">
    <rdfs:isDefinedBy rdf:resource="http://open-services.net/ns/sysmlv2#"/>
    <rdfs:comment>The OccurrenceUsages that are ownedUsages of this Definition.</rdfs:comment>
    <rdfs:label>definition_OwnedOccurrence</rdfs:label>
  </rdf:Property>
  <rdf:Property rdf:about="http://open-services.net/ns/sysmlv2#element_OwnedAnnotation">
    <rdfs:isDefinedBy rdf:resource="http://open-services.net/ns/sysmlv2#"/>
    <rdfs:comment>The ownedRelationships of this Element that are Annotations, for which this Element is the annotatedElement.</rdfs:comment>
    <rdfs:label>element_OwnedAnnotation</rdfs:label>
  </rdf:Property>
  <rdf:Property rdf:about="http://open-services.net/ns/sysmlv2#definition_OwnedConstraint">
    <rdfs:isDefinedBy rdf:resource="http://open-services.net/ns/sysmlv2#"/>
    <rdfs:comment>The ConstraintUsages that are ownedUsages of this Definition.</rdfs:comment>
    <rdfs:label>definition_OwnedConstraint</rdfs:label>
  </rdf:Property>
  <rdf:Property rdf:about="http://open-services.net/ns/sysmlv2#analysisCaseUsage_AnalysisCaseDefinition">
    <rdfs:isDefinedBy rdf:resource="http://open-services.net/ns/sysmlv2#"/>
    <rdfs:comment>The AnalysisCaseDefinition that is the definition of this AnalysisCaseUsage.</rdfs:comment>
    <rdfs:label>analysisCaseUsage_AnalysisCaseDefinition</rdfs:label>
  </rdf:Property>
  <rdf:Property rdf:about="http://open-services.net/ns/sysmlv2#type_Input">
    <rdfs:isDefinedBy rdf:resource="http://open-services.net/ns/sysmlv2#"/>
    <rdfs:comment>All features related to this Type by FeatureMemberships that have direction in or inout.</rdfs:comment>
    <rdfs:label>type_Input</rdfs:label>
  </rdf:Property>
  <rdf:Property rdf:about="http://open-services.net/ns/sysmlv2#textualRepresentation_Body">
    <rdfs:isDefinedBy rdf:resource="http://open-services.net/ns/sysmlv2#"/>
    <rdfs:comment>The textual representation of the representedElement in the given language.</rdfs:comment>
    <rdfs:label>textualRepresentation_Body</rdfs:label>
  </rdf:Property>
  <rdf:Property rdf:about="http://open-services.net/ns/sysmlv2#type_InheritedMembership">
    <rdfs:isDefinedBy rdf:resource="http://open-services.net/ns/sysmlv2#"/>
    <rdfs:comment>All Memberships inherited by this Type via Specialization or Conjugation. These are included in the derived union for the memberships of the Type.</rdfs:comment>
    <rdfs:label>type_InheritedMembership</rdfs:label>
  </rdf:Property>
  <rdf:Property rdf:about="http://open-services.net/ns/sysmlv2#stateDefinition_ExitAction">
    <rdfs:isDefinedBy rdf:resource="http://open-services.net/ns/sysmlv2#"/>
    <rdfs:comment>The ActionUsage of this StateDefinition to be performed on exit to the state defined by the StateDefinition. It is the owned ActionUsage related to the StateDefinition by a StateSubactionMembership  with kind = exit.</rdfs:comment>
    <rdfs:label>stateDefinition_ExitAction</rdfs:label>
  </rdf:Property>
  <rdf:Property rdf:about="http://open-services.net/ns/sysmlv2#definition_OwnedState">
    <rdfs:isDefinedBy rdf:resource="http://open-services.net/ns/sysmlv2#"/>
    <rdfs:comment>The StateUsages that are ownedUsages of this Definition.</rdfs:comment>
    <rdfs:label>definition_OwnedState</rdfs:label>
  </rdf:Property>
  <rdf:Property rdf:about="http://open-services.net/ns/sysmlv2#classifier_OwnedSubclassification">
    <rdfs:isDefinedBy rdf:resource="http://open-services.net/ns/sysmlv2#"/>
    <rdfs:comment>The ownedSpecializations of this Classifier that are Subclassifications, for which this Classifier is the subclassifier.</rdfs:comment>
    <rdfs:label>classifier_OwnedSubclassification</rdfs:label>
  </rdf:Property>
  <rdf:Property rdf:about="http://open-services.net/ns/sysmlv2#transitionUsage_Target">
    <rdfs:isDefinedBy rdf:resource="http://open-services.net/ns/sysmlv2#"/>
    <rdfs:comment>The target ActionUsage of this TransitionUsage, which is the targetFeature of the succession for the TransitionUsage.</rdfs:comment>
    <rdfs:label>transitionUsage_Target</rdfs:label>
  </rdf:Property>
  <rdf:Property rdf:about="http://open-services.net/ns/sysmlv2#requirementConstraintMembership_OwnedConstraint">
    <rdfs:isDefinedBy rdf:resource="http://open-services.net/ns/sysmlv2#"/>
    <rdfs:comment>The ConstraintUsage that is the ownedMemberFeature of this RequirementConstraintMembership.</rdfs:comment>
    <rdfs:label>requirementConstraintMembership_OwnedConstraint</rdfs:label>
  </rdf:Property>
  <rdf:Property rdf:about="http://open-services.net/ns/sysmlv2#owningMembership_OwnedMemberElementId">
    <rdfs:isDefinedBy rdf:resource="http://open-services.net/ns/sysmlv2#"/>
    <rdfs:comment>The elementId of the ownedMemberElement.</rdfs:comment>
    <rdfs:label>owningMembership_OwnedMemberElementId</rdfs:label>
  </rdf:Property>
  <rdf:Property rdf:about="http://open-services.net/ns/sysmlv2#owningMembership_OwnedMemberShortName">
    <rdfs:isDefinedBy rdf:resource="http://open-services.net/ns/sysmlv2#"/>
    <rdfs:comment>The shortName of the ownedMemberElement.</rdfs:comment>
    <rdfs:label>owningMembership_OwnedMemberShortName</rdfs:label>
  </rdf:Property>
  <rdf:Property rdf:about="http://open-services.net/ns/sysmlv2#type_OwnedFeatureMembership">
    <rdfs:isDefinedBy rdf:resource="http://open-services.net/ns/sysmlv2#"/>
    <rdfs:comment>The ownedMemberships of this Type that are FeatureMemberships, for which the Type is the owningType. Each such FeatureMembership identifies an ownedFeature of the Type.</rdfs:comment>
    <rdfs:label>type_OwnedFeatureMembership</rdfs:label>
  </rdf:Property>
  <rdf:Property rdf:about="http://open-services.net/ns/sysmlv2#definition_OwnedEnumeration">
    <rdfs:isDefinedBy rdf:resource="http://open-services.net/ns/sysmlv2#"/>
    <rdfs:comment>The EnumerationUsages that are ownedUsages of this Definition.</rdfs:comment>
    <rdfs:label>definition_OwnedEnumeration</rdfs:label>
  </rdf:Property>
  <rdf:Property rdf:about="http://open-services.net/ns/sysmlv2#connectionDefinition_ConnectionEnd">
    <rdfs:isDefinedBy rdf:resource="http://open-services.net/ns/sysmlv2#"/>
    <rdfs:comment>The Usages that define the things related by the ConnectionDefinition.</rdfs:comment>
    <rdfs:label>connectionDefinition_ConnectionEnd</rdfs:label>
  </rdf:Property>
  <rdf:Property rdf:about="http://open-services.net/ns/sysmlv2#definition_Usage">
    <rdfs:isDefinedBy rdf:resource="http://open-services.net/ns/sysmlv2#"/>
    <rdfs:comment>The Usages that are features of this Definition (not necessarily owned).</rdfs:comment>
    <rdfs:label>definition_Usage</rdfs:label>
  </rdf:Property>
  <rdf:Property rdf:about="http://open-services.net/ns/sysmlv2#element_DeclaredName">
    <rdfs:isDefinedBy rdf:resource="http://open-services.net/ns/sysmlv2#"/>
    <rdfs:comment>The declared name of this Element.</rdfs:comment>
    <rdfs:label>element_DeclaredName</rdfs:label>
  </rdf:Property>
  <rdf:Property rdf:about="http://open-services.net/ns/sysmlv2#textualRepresentation_Language">
    <rdfs:isDefinedBy rdf:resource="http://open-services.net/ns/sysmlv2#"/>
    <rdfs:comment>The natural or artifical language in which the body text is written.</rdfs:comment>
    <rdfs:label>textualRepresentation_Language</rdfs:label>
  </rdf:Property>
  <rdf:Property rdf:about="http://open-services.net/ns/sysmlv2#featureChainExpression_TargetFeature">
    <rdfs:isDefinedBy rdf:resource="http://open-services.net/ns/sysmlv2#"/>
    <rdfs:comment>The Feature that is accessed by this FeatureChainExpression, which is its first non-parameter member.</rdfs:comment>
    <rdfs:label>featureChainExpression_TargetFeature</rdfs:label>
  </rdf:Property>
  <rdf:Property rdf:about="http://open-services.net/ns/sysmlv2#feature_Type">
    <rdfs:isDefinedBy rdf:resource="http://open-services.net/ns/sysmlv2#"/>
    <rdfs:comment>Types that restrict the values of this Feature, such that the values must be instances of all the types. The types of a Feature are derived from its typings and the types of its subsettings. If the Feature is chained, then the types of the last Feature in the chain are also types of the chained Feature.</rdfs:comment>
    <rdfs:label>feature_Type</rdfs:label>
  </rdf:Property>
  <rdf:Property rdf:about="http://open-services.net/ns/sysmlv2#literalRational_Value">
    <rdfs:isDefinedBy rdf:resource="http://open-services.net/ns/sysmlv2#"/>
    <rdfs:comment>The value whose rational approximation is the result of evaluating this LiteralRational.</rdfs:comment>
    <rdfs:label>literalRational_Value</rdfs:label>
  </rdf:Property>
  <rdf:Property rdf:about="http://open-services.net/ns/sysmlv2#analysisCaseDefinition_AnalysisAction">
    <rdfs:isDefinedBy rdf:resource="http://open-services.net/ns/sysmlv2#"/>
    <rdfs:comment>The composite actions of the AnalysisCaseDefinition that are defined as AnalysisActions.</rdfs:comment>
    <rdfs:label>analysisCaseDefinition_AnalysisAction</rdfs:label>
  </rdf:Property>
  <rdf:Property rdf:about="http://open-services.net/ns/sysmlv2#definition_OwnedReference">
    <rdfs:isDefinedBy rdf:resource="http://open-services.net/ns/sysmlv2#"/>
    <rdfs:comment>The ReferenceUsages that are ownedUsages of this Definition.</rdfs:comment>
    <rdfs:label>definition_OwnedReference</rdfs:label>
  </rdf:Property>
  <rdf:Property rdf:about="http://open-services.net/ns/sysmlv2#loopActionUsage_BodyAction">
    <rdfs:isDefinedBy rdf:resource="http://open-services.net/ns/sysmlv2#"/>
    <rdfs:comment>The ActionUsage to be performed repeatedly by the LoopActionUsage. It is the second parameter of the LoopActionUsage.</rdfs:comment>
    <rdfs:label>loopActionUsage_BodyAction</rdfs:label>
  </rdf:Property>
  <rdf:Property rdf:about="http://open-services.net/ns/sysmlv2#usage_NestedTransition">
    <rdfs:isDefinedBy rdf:resource="http://open-services.net/ns/sysmlv2#"/>
    <rdfs:comment>The TransitionUsages that are nestedUsages of this Usage.</rdfs:comment>
    <rdfs:label>usage_NestedTransition</rdfs:label>
  </rdf:Property>
  <rdf:Property rdf:about="http://open-services.net/ns/sysmlv2#caseUsage_CaseDefinition">
    <rdfs:isDefinedBy rdf:resource="http://open-services.net/ns/sysmlv2#"/>
    <rdfs:comment>The CaseDefinition that is the type of this CaseUsage.</rdfs:comment>
    <rdfs:label>caseUsage_CaseDefinition</rdfs:label>
  </rdf:Property>
  <rdf:Property rdf:about="http://open-services.net/ns/sysmlv2#type_IsSufficient">
    <rdfs:isDefinedBy rdf:resource="http://open-services.net/ns/sysmlv2#"/>
    <rdfs:comment>Whether all things that meet the classification conditions of this Type must be classified by the Type.</rdfs:comment>
    <rdfs:label>type_IsSufficient</rdfs:label>
  </rdf:Property>
  <rdf:Property rdf:about="http://open-services.net/ns/sysmlv2#type_OwnedFeature">
    <rdfs:isDefinedBy rdf:resource="http://open-services.net/ns/sysmlv2#"/>
    <rdfs:comment>The ownedMemberFeatures of the ownedFeatureMemberships of this Type.</rdfs:comment>
    <rdfs:label>type_OwnedFeature</rdfs:label>
  </rdf:Property>
  <rdf:Property rdf:about="http://open-services.net/ns/sysmlv2#usage_NestedViewpoint">
    <rdfs:isDefinedBy rdf:resource="http://open-services.net/ns/sysmlv2#"/>
    <rdfs:comment>The ViewpointUsages that are nestedUsages of this Usage.</rdfs:comment>
    <rdfs:label>usage_NestedViewpoint</rdfs:label>
  </rdf:Property>
  <rdf:Property rdf:about="http://open-services.net/ns/sysmlv2#requirementDefinition_SubjectParameter">
    <rdfs:isDefinedBy rdf:resource="http://open-services.net/ns/sysmlv2#"/>
    <rdfs:comment>The parameter of this RequirementDefinition that represents its subject.</rdfs:comment>
    <rdfs:label>requirementDefinition_SubjectParameter</rdfs:label>
  </rdf:Property>
  <rdf:Property rdf:about="http://open-services.net/ns/sysmlv2#step_Behavior">
    <rdfs:isDefinedBy rdf:resource="http://open-services.net/ns/sysmlv2#"/>
    <rdfs:comment>The Behaviors that type this Step.</rdfs:comment>
    <rdfs:label>step_Behavior</rdfs:label>
  </rdf:Property>
  <rdf:Property rdf:about="http://open-services.net/ns/sysmlv2#connector_TargetFeature">
    <rdfs:isDefinedBy rdf:resource="http://open-services.net/ns/sysmlv2#"/>
    <rdfs:comment>The target relatedFeatures for this Connector. This includes all the relatedFeatures other than the sourceFeature.</rdfs:comment>
    <rdfs:label>connector_TargetFeature</rdfs:label>
  </rdf:Property>
  <rdf:Property rdf:about="http://open-services.net/ns/sysmlv2#caseUsage_ActorParameter">
    <rdfs:isDefinedBy rdf:resource="http://open-services.net/ns/sysmlv2#"/>
    <rdfs:comment>The parameters of this CaseUsage that represent actors involved in the case.</rdfs:comment>
    <rdfs:label>caseUsage_ActorParameter</rdfs:label>
  </rdf:Property>
  <rdf:Property rdf:about="http://open-services.net/ns/sysmlv2#type_FeatureMembership">
    <rdfs:isDefinedBy rdf:resource="http://open-services.net/ns/sysmlv2#"/>
    <rdfs:comment>The FeatureMemberships for features of this Type, which include all ownedFeatureMemberships and those inheritedMemberships that are FeatureMemberships (but does not include any importedMemberships).</rdfs:comment>
    <rdfs:label>type_FeatureMembership</rdfs:label>
  </rdf:Property>
  <rdf:Property rdf:about="http://open-services.net/ns/sysmlv2#feature_OwnedTypeFeaturing">
    <rdfs:isDefinedBy rdf:resource="http://open-services.net/ns/sysmlv2#"/>
    <rdfs:comment>The ownedRelationships of this Feature that are TypeFeaturings and for which the Feature is the featureOfType.</rdfs:comment>
    <rdfs:label>feature_OwnedTypeFeaturing</rdfs:label>
  </rdf:Property>
  <rdf:Property rdf:about="http://open-services.net/ns/sysmlv2#requirementUsage_RequiredConstraint">
    <rdfs:isDefinedBy rdf:resource="http://open-services.net/ns/sysmlv2#"/>
    <rdfs:comment>The owned ConstraintUsages that represent requirements of this RequirementUsage, which are the ownedConstraints of the RequirementConstraintMemberships of the RequirementUsage with kind = requirement.</rdfs:comment>
    <rdfs:label>requirementUsage_RequiredConstraint</rdfs:label>
  </rdf:Property>
  <rdf:Property rdf:about="http://open-services.net/ns/sysmlv2#featureMembership_OwningType">
    <rdfs:isDefinedBy rdf:resource="http://open-services.net/ns/sysmlv2#"/>
    <rdfs:comment>The Type that owns this FeatureMembership.</rdfs:comment>
    <rdfs:label>featureMembership_OwningType</rdfs:label>
  </rdf:Property>
  <rdf:Property rdf:about="http://open-services.net/ns/sysmlv2#namespace_OwnedMember">
    <rdfs:isDefinedBy rdf:resource="http://open-services.net/ns/sysmlv2#"/>
    <rdfs:comment>The owned members of this Namespace, which are the ownedMemberElements of the ownedMemberships of the .</rdfs:comment>
    <rdfs:label>namespace_OwnedMember</rdfs:label>
  </rdf:Property>
  <rdf:Property rdf:about="http://open-services.net/ns/sysmlv2#subsetting_SubsettedFeature">
    <rdfs:isDefinedBy rdf:resource="http://open-services.net/ns/sysmlv2#"/>
    <rdfs:comment>The Feature that is subsetted by the subsettingFeature of this Subsetting.</rdfs:comment>
    <rdfs:label>subsetting_SubsettedFeature</rdfs:label>
  </rdf:Property>
  <rdf:Property rdf:about="http://open-services.net/ns/sysmlv2#connector_ConnectorEnd">
    <rdfs:isDefinedBy rdf:resource="http://open-services.net/ns/sysmlv2#"/>
    <rdfs:comment>The endFeatures of a Connector, which redefine the endFeatures of the associations of the Connector. The connectorEnds determine via ReferenceSubsetting Relationships which Features are related by the Connector.</rdfs:comment>
    <rdfs:label>connector_ConnectorEnd</rdfs:label>
  </rdf:Property>
  <rdf:Property rdf:about="http://open-services.net/ns/sysmlv2#stateUsage_StateDefinition">
    <rdfs:isDefinedBy rdf:resource="http://open-services.net/ns/sysmlv2#"/>
    <rdfs:comment>The Behaviors that are the types of this StateUsage. Nominally, these would be StateDefinitions, but kernel Behaviors are also allowed, to permit use of Behaviors from the Kernel Model Libraries.</rdfs:comment>
    <rdfs:label>stateUsage_StateDefinition</rdfs:label>
  </rdf:Property>
  <rdf:Property rdf:about="http://open-services.net/ns/sysmlv2#stateSubactionMembership_Action">
    <rdfs:isDefinedBy rdf:resource="http://open-services.net/ns/sysmlv2#"/>
    <rdfs:comment>The ActionUsage that is the ownedMemberFeature of this StateSubactionMembership.</rdfs:comment>
    <rdfs:label>stateSubactionMembership_Action</rdfs:label>
  </rdf:Property>
  <rdf:Property rdf:about="http://open-services.net/ns/sysmlv2#usage_NestedConnection">
    <rdfs:isDefinedBy rdf:resource="http://open-services.net/ns/sysmlv2#"/>
    <rdfs:comment>The ConnectorAsUsages that are nestedUsages of this Usage. Note that this list includes BindingConnectorAsUsages and SuccessionAsUsages, even though these are ConnectorAsUsages but not ConnectionUsages.</rdfs:comment>
    <rdfs:label>usage_NestedConnection</rdfs:label>
  </rdf:Property>
  <rdf:Property rdf:about="http://open-services.net/ns/sysmlv2#namespace_Membership">
    <rdfs:isDefinedBy rdf:resource="http://open-services.net/ns/sysmlv2#"/>
    <rdfs:comment>All Memberships in this Namespace, including (at least) the union of ownedMemberships and importedMemberships.</rdfs:comment>
    <rdfs:label>namespace_Membership</rdfs:label>
  </rdf:Property>
  <rdf:Property rdf:about="http://open-services.net/ns/sysmlv2#analysisCaseUsage_AnalysisAction">
    <rdfs:isDefinedBy rdf:resource="http://open-services.net/ns/sysmlv2#"/>
    <rdfs:comment>The composite usages of the AnalysisCaseUsage that are defined as AnalysisActions.</rdfs:comment>
    <rdfs:label>analysisCaseUsage_AnalysisAction</rdfs:label>
  </rdf:Property>
  <rdf:Property rdf:about="http://open-services.net/ns/sysmlv2#type_Feature">
    <rdfs:isDefinedBy rdf:resource="http://open-services.net/ns/sysmlv2#"/>
    <rdfs:comment>The ownedMemberFeatures of the featureMemberships of this Type.</rdfs:comment>
    <rdfs:label>type_Feature</rdfs:label>
  </rdf:Property>
  <rdf:Property rdf:about="http://open-services.net/ns/sysmlv2#differencing_TypeDifferenced">
    <rdfs:isDefinedBy rdf:resource="http://open-services.net/ns/sysmlv2#"/>
    <rdfs:comment>Type with interpretations partly determined by differencingType, as described in Type::differencingType.</rdfs:comment>
    <rdfs:label>differencing_TypeDifferenced</rdfs:label>
  </rdf:Property>
  <rdf:Property rdf:about="http://open-services.net/ns/sysmlv2#association_SourceType">
    <rdfs:isDefinedBy rdf:resource="http://open-services.net/ns/sysmlv2#"/>
    <rdfs:comment>The source relatedType for this Association. It is the first relatedType of the Association.</rdfs:comment>
    <rdfs:label>association_SourceType</rdfs:label>
  </rdf:Property>
  <rdf:Property rdf:about="http://open-services.net/ns/sysmlv2#whileLoopActionUsage_UntilArgument">
    <rdfs:isDefinedBy rdf:resource="http://open-services.net/ns/sysmlv2#"/>
    <rdfs:comment>The Expression whose result, if false, determines that the bodyAction should continue to be performed. It is the (optional) third owned parameter of the WhileLoopActionUsage.</rdfs:comment>
    <rdfs:label>whileLoopActionUsage_UntilArgument</rdfs:label>
  </rdf:Property>
  <rdf:Property rdf:about="http://open-services.net/ns/sysmlv2#assertConstraintUsage_AssertedConstraint">
    <rdfs:isDefinedBy rdf:resource="http://open-services.net/ns/sysmlv2#"/>
    <rdfs:comment>The ConstraintUsage to be performed by the AssertConstraintUsage. It is the referenceFeature of the ownedReferenceSubsetting for the AssertConstraintUsage, if there is one, and, otherwise, the AssertConstraintUsage itself.</rdfs:comment>
    <rdfs:label>assertConstraintUsage_AssertedConstraint</rdfs:label>
  </rdf:Property>
  <rdf:Property rdf:about="http://open-services.net/ns/sysmlv2#usage_NestedAnalysisCase">
    <rdfs:isDefinedBy rdf:resource="http://open-services.net/ns/sysmlv2#"/>
    <rdfs:comment>The AnalysisCaseUsages that are nestedUsages of this Usage.</rdfs:comment>
    <rdfs:label>usage_NestedAnalysisCase</rdfs:label>
  </rdf:Property>
  <rdf:Property rdf:about="http://open-services.net/ns/sysmlv2#definition_OwnedCase">
    <rdfs:isDefinedBy rdf:resource="http://open-services.net/ns/sysmlv2#"/>
    <rdfs:comment>The code&gt;CaseUsages that are ownedUsages of this Definition.</rdfs:comment>
    <rdfs:label>definition_OwnedCase</rdfs:label>
  </rdf:Property>
  <rdf:Property rdf:about="http://open-services.net/ns/sysmlv2#usage_NestedAttribute">
    <rdfs:isDefinedBy rdf:resource="http://open-services.net/ns/sysmlv2#"/>
    <rdfs:comment>The code&gt;AttributeUsages that are nestedUsages of this Usage.</rdfs:comment>
    <rdfs:label>usage_NestedAttribute</rdfs:label>
  </rdf:Property>
  <rdf:Property rdf:about="http://open-services.net/ns/sysmlv2#feature_OwnedRedefinition">
    <rdfs:isDefinedBy rdf:resource="http://open-services.net/ns/sysmlv2#"/>
    <rdfs:comment>The ownedSubsettings of this Feature that are Redefinitions, for which the Feature is the redefiningFeature.</rdfs:comment>
    <rdfs:label>feature_OwnedRedefinition</rdfs:label>
  </rdf:Property>
  <rdf:Property rdf:about="http://open-services.net/ns/sysmlv2#element_Name">
    <rdfs:isDefinedBy rdf:resource="http://open-services.net/ns/sysmlv2#"/>
    <rdfs:comment>The name to be used for this Element during name resolution within its owningNamespace. This is derived using the effectiveName() operation. By default, it is the same as the declaredName, but this is overridden for certain kinds of Elements to compute a name even when the declaredName is null.</rdfs:comment>
    <rdfs:label>element_Name</rdfs:label>
  </rdf:Property>
  <rdf:Property rdf:about="http://open-services.net/ns/sysmlv2#usage_NestedFlow">
    <rdfs:isDefinedBy rdf:resource="http://open-services.net/ns/sysmlv2#"/>
    <rdfs:comment>The code&gt;FlowConnectionUsages that are nestedUsages of this Usage.</rdfs:comment>
    <rdfs:label>usage_NestedFlow</rdfs:label>
  </rdf:Property>
  <rdf:Property rdf:about="http://open-services.net/ns/sysmlv2#occurrenceUsage_OccurrenceDefinition">
    <rdfs:isDefinedBy rdf:resource="http://open-services.net/ns/sysmlv2#"/>
    <rdfs:comment>The Classes that are the types of this OccurrenceUsage. Nominally, these are OccurrenceDefinitions, but other kinds of kernel Classes are also allowed, to permit use of Classes from the Kernel Model Libraries.</rdfs:comment>
    <rdfs:label>occurrenceUsage_OccurrenceDefinition</rdfs:label>
  </rdf:Property>
  <rdf:Property rdf:about="http://open-services.net/ns/sysmlv2#itemFlow_ItemFeature">
    <rdfs:isDefinedBy rdf:resource="http://open-services.net/ns/sysmlv2#"/>
    <rdfs:comment>The ownedFeature of the ItemFlow that is an ItemFeature (if any).</rdfs:comment>
    <rdfs:label>itemFlow_ItemFeature</rdfs:label>
  </rdf:Property>
  <rdf:Property rdf:about="http://open-services.net/ns/sysmlv2#definition_OwnedAnalysisCase">
    <rdfs:isDefinedBy rdf:resource="http://open-services.net/ns/sysmlv2#"/>
    <rdfs:comment>The AnalysisCaseUsages that are ownedUsages of this Definition.</rdfs:comment>
    <rdfs:label>definition_OwnedAnalysisCase</rdfs:label>
  </rdf:Property>
  <rdf:Property rdf:about="http://open-services.net/ns/sysmlv2#featureReferenceExpression_Referent">
    <rdfs:isDefinedBy rdf:resource="http://open-services.net/ns/sysmlv2#"/>
    <rdfs:comment>The Feature that is referenced by this FeatureReferenceExpression, which is its first non-parameter member.</rdfs:comment>
    <rdfs:label>featureReferenceExpression_Referent</rdfs:label>
  </rdf:Property>
  <rdf:Property rdf:about="http://open-services.net/ns/sysmlv2#differencing_DifferencingType">
    <rdfs:isDefinedBy rdf:resource="http://open-services.net/ns/sysmlv2#"/>
    <rdfs:comment>Type that partly determines interpretations of typeDifferenced, as described in Type::differencingType.</rdfs:comment>
    <rdfs:label>differencing_DifferencingType</rdfs:label>
  </rdf:Property>
  <rdf:Property rdf:about="http://open-services.net/ns/sysmlv2#annotatingElement_Annotation">
    <rdfs:isDefinedBy rdf:resource="http://open-services.net/ns/sysmlv2#"/>
    <rdfs:comment>The Annotations that relate this AnnotatingElement to its annotatedElements.</rdfs:comment>
    <rdfs:label>annotatingElement_Annotation</rdfs:label>
  </rdf:Property>
  <rdf:Property rdf:about="http://open-services.net/ns/sysmlv2#analysisCaseDefinition_ResultExpression">
    <rdfs:isDefinedBy rdf:resource="http://open-services.net/ns/sysmlv2#"/>
    <rdfs:comment>An Expression used to compute the result of the AnalysisCaseDefinition, owned via a ResultExpressionMembership.</rdfs:comment>
    <rdfs:label>analysisCaseDefinition_ResultExpression</rdfs:label>
  </rdf:Property>
  <rdf:Property rdf:about="http://open-services.net/ns/sysmlv2#typeFeaturing_FeatureOfType">
    <rdfs:isDefinedBy rdf:resource="http://open-services.net/ns/sysmlv2#"/>
    <rdfs:comment>The Feature that is featured by the featuringType. It is the source of the TypeFeaturing.</rdfs:comment>
    <rdfs:label>typeFeaturing_FeatureOfType</rdfs:label>
  </rdf:Property>
  <rdf:Property rdf:about="http://open-services.net/ns/sysmlv2#attributeUsage_AttributeDefinition">
    <rdfs:isDefinedBy rdf:resource="http://open-services.net/ns/sysmlv2#"/>
    <rdfs:comment>The DataTypes that are the types of this AttributeUsage. Nominally, these are AttributeDefinitions, but other kinds of kernel DataTypes are also allowed, to permit use of DataTypes from the Kernel Model Libraries.</rdfs:comment>
    <rdfs:label>attributeUsage_AttributeDefinition</rdfs:label>
  </rdf:Property>
  <rdf:Property rdf:about="http://open-services.net/ns/sysmlv2#viewRenderingMembership_ReferencedRendering">
    <rdfs:isDefinedBy rdf:resource="http://open-services.net/ns/sysmlv2#"/>
    <rdfs:comment> The RenderingUsage that is referenced through this ViewRenderingMembership. It is the referencedFeature of the ownedReferenceSubsetting for the ownedRendering, if there is one, and, otherwise, the ownedRendering itself.</rdfs:comment>
    <rdfs:label>viewRenderingMembership_ReferencedRendering</rdfs:label>
  </rdf:Property>
  <rdf:Property rdf:about="http://open-services.net/ns/sysmlv2#requirementVerificationMembership_OwnedRequirement">
    <rdfs:isDefinedBy rdf:resource="http://open-services.net/ns/sysmlv2#"/>
    <rdfs:comment>The owned RequirementUsage that acts as the ownedConstraint for this RequirementVerificationMembership. This will either be the verifiedRequirement, or it will subset the verifiedRequirement.</rdfs:comment>
    <rdfs:label>requirementVerificationMembership_OwnedRequirement</rdfs:label>
  </rdf:Property>
  <rdf:Property rdf:about="http://open-services.net/ns/sysmlv2#annotation_OwningAnnotatedElement">
    <rdfs:isDefinedBy rdf:resource="http://open-services.net/ns/sysmlv2#"/>
    <rdfs:comment>The annotatedElement of this Annotation, when it is also its owningRelatedElement.</rdfs:comment>
    <rdfs:label>annotation_OwningAnnotatedElement</rdfs:label>
  </rdf:Property>
  <rdf:Property rdf:about="http://open-services.net/ns/sysmlv2#usage_NestedCase">
    <rdfs:isDefinedBy rdf:resource="http://open-services.net/ns/sysmlv2#"/>
    <rdfs:comment>The CaseUsages that are nestedUsages of this Usage.</rdfs:comment>
    <rdfs:label>usage_NestedCase</rdfs:label>
  </rdf:Property>
  <rdf:Property rdf:about="http://open-services.net/ns/sysmlv2#type_OwnedUnioning">
    <rdfs:isDefinedBy rdf:resource="http://open-services.net/ns/sysmlv2#"/>
    <rdfs:comment>The ownedRelationships of this Type that are Unionings, having the Type as their typeUnioned.</rdfs:comment>
    <rdfs:label>type_OwnedUnioning</rdfs:label>
  </rdf:Property>
  <rdf:Property rdf:about="http://open-services.net/ns/sysmlv2#specialization_Specific">
    <rdfs:isDefinedBy rdf:resource="http://open-services.net/ns/sysmlv2#"/>
    <rdfs:comment>A Type with a subset of all instances of the general Type, which might be the same set.</rdfs:comment>
    <rdfs:label>specialization_Specific</rdfs:label>
  </rdf:Property>
  <rdf:Property rdf:about="http://open-services.net/ns/sysmlv2#calculationDefinition_Calculation">
    <rdfs:isDefinedBy rdf:resource="http://open-services.net/ns/sysmlv2#"/>
    <rdfs:comment>The actions of this CalculationDefinition that are CalculationUsages.</rdfs:comment>
    <rdfs:label>calculationDefinition_Calculation</rdfs:label>
  </rdf:Property>
  <rdf:Property rdf:about="http://open-services.net/ns/sysmlv2#sendActionUsage_ReceiverArgument">
    <rdfs:isDefinedBy rdf:resource="http://open-services.net/ns/sysmlv2#"/>
    <rdfs:comment>An Expression whose result is bound to the receiver input parameter of this SendActionUsage.</rdfs:comment>
    <rdfs:label>sendActionUsage_ReceiverArgument</rdfs:label>
  </rdf:Property>
  <rdf:Property rdf:about="http://open-services.net/ns/sysmlv2#stakeholderMembership_OwnedStakeholderParameter">
    <rdfs:isDefinedBy rdf:resource="http://open-services.net/ns/sysmlv2#"/>
    <rdfs:comment>The PartUsage specifying the stakeholder.</rdfs:comment>
    <rdfs:label>stakeholderMembership_OwnedStakeholderParameter</rdfs:label>
  </rdf:Property>
  <rdf:Property rdf:about="http://open-services.net/ns/sysmlv2#requirementDefinition_ActorParameter">
    <rdfs:isDefinedBy rdf:resource="http://open-services.net/ns/sysmlv2#"/>
    <rdfs:comment>The parameters of this RequirementDefinition that represent actors involved in the requirement.</rdfs:comment>
    <rdfs:label>requirementDefinition_ActorParameter</rdfs:label>
  </rdf:Property>
  <rdf:Property rdf:about="http://open-services.net/ns/sysmlv2#booleanExpression_Predicate">
    <rdfs:isDefinedBy rdf:resource="http://open-services.net/ns/sysmlv2#"/>
    <rdfs:comment>The Predicate that types this BooleanExpression.</rdfs:comment>
    <rdfs:label>booleanExpression_Predicate</rdfs:label>
  </rdf:Property>
  <rdf:Property rdf:about="http://open-services.net/ns/sysmlv2#usage_NestedPort">
    <rdfs:isDefinedBy rdf:resource="http://open-services.net/ns/sysmlv2#"/>
    <rdfs:comment>The PortUsages that are nestedUsages of this Usage.</rdfs:comment>
    <rdfs:label>usage_NestedPort</rdfs:label>
  </rdf:Property>
  <rdf:Property rdf:about="http://open-services.net/ns/sysmlv2#analysisCaseUsage_ResultExpression">
    <rdfs:isDefinedBy rdf:resource="http://open-services.net/ns/sysmlv2#"/>
    <rdfs:comment>An Expression used to compute the result of the AnalysisCaseUsage, owned via a ResultExpressionMembership.</rdfs:comment>
    <rdfs:label>analysisCaseUsage_ResultExpression</rdfs:label>
  </rdf:Property>
  <rdf:Property rdf:about="http://open-services.net/ns/sysmlv2#usage_OwningUsage">
    <rdfs:isDefinedBy rdf:resource="http://open-services.net/ns/sysmlv2#"/>
    <rdfs:comment>The Usage in which this Usage is nested (if any).</rdfs:comment>
    <rdfs:label>usage_OwningUsage</rdfs:label>
  </rdf:Property>
  <rdf:Property rdf:about="http://open-services.net/ns/sysmlv2#verificationCaseDefinition_VerifiedRequirement">
    <rdfs:isDefinedBy rdf:resource="http://open-services.net/ns/sysmlv2#"/>
    <rdfs:comment>The RequirementUsages verified by this VerificationCaseDefinition, which are the verifiedRequirements of all RequirementVerificationMemberships of the objectiveRequirement.</rdfs:comment>
    <rdfs:label>verificationCaseDefinition_VerifiedRequirement</rdfs:label>
  </rdf:Property>
  <rdf:Property rdf:about="http://open-services.net/ns/sysmlv2#viewpointUsage_ViewpointStakeholder">
    <rdfs:isDefinedBy rdf:resource="http://open-services.net/ns/sysmlv2#"/>
    <rdfs:comment>The PartUsages that identify the stakeholders with concerns framed by this ViewpointUsage, which are the owned and inherited stakeholderParameters of the framedConcerns of this ViewpointUsage.</rdfs:comment>
    <rdfs:label>viewpointUsage_ViewpointStakeholder</rdfs:label>
  </rdf:Property>
  <rdf:Property rdf:about="http://open-services.net/ns/sysmlv2#partUsage_PartDefinition">
    <rdfs:isDefinedBy rdf:resource="http://open-services.net/ns/sysmlv2#"/>
    <rdfs:comment>The itemDefinitions of this PartUsage that are PartDefinitions.</rdfs:comment>
    <rdfs:label>partUsage_PartDefinition</rdfs:label>
  </rdf:Property>
  <rdf:Property rdf:about="http://open-services.net/ns/sysmlv2#viewUsage_ViewRendering">
    <rdfs:isDefinedBy rdf:resource="http://open-services.net/ns/sysmlv2#"/>
    <rdfs:comment>The RenderingUsage to be used to render views defined by this ViewUsage, which is the referencedRendering of the ViewRenderingMembership of the ViewUsage.</rdfs:comment>
    <rdfs:label>viewUsage_ViewRendering</rdfs:label>
  </rdf:Property>
  <rdf:Property rdf:about="http://open-services.net/ns/sysmlv2#import_ImportOwningNamespace">
    <rdfs:isDefinedBy rdf:resource="http://open-services.net/ns/sysmlv2#"/>
    <rdfs:comment>The Namespace into which Memberships are imported by this Import, which must be the owningRelatedElement of the Import.</rdfs:comment>
    <rdfs:label>import_ImportOwningNamespace</rdfs:label>
  </rdf:Property>
  <rdf:Property rdf:about="http://open-services.net/ns/sysmlv2#type_UnioningType">
    <rdfs:isDefinedBy rdf:resource="http://open-services.net/ns/sysmlv2#"/>
    <rdfs:comment>The interpretations of a Type with unioningTypes are asserted to be the same as those of all the unioningTypes together, which are the Types derived from the unioningType of the ownedUnionings of this Type. For example, a Classifier for people might be the union of Classifiers for all the sexes. Similarly, a feature for people's children might be the union of features dividing them in the same ways as people in general.</rdfs:comment>
    <rdfs:label>type_UnioningType</rdfs:label>
  </rdf:Property>
  <rdf:Property rdf:about="http://open-services.net/ns/sysmlv2#definition_OwnedPart">
    <rdfs:isDefinedBy rdf:resource="http://open-services.net/ns/sysmlv2#"/>
    <rdfs:comment>The PartUsages that are ownedUsages of this Definition.</rdfs:comment>
    <rdfs:label>definition_OwnedPart</rdfs:label>
  </rdf:Property>
  <rdf:Property rdf:about="http://open-services.net/ns/sysmlv2#featureValue_Value">
    <rdfs:isDefinedBy rdf:resource="http://open-services.net/ns/sysmlv2#"/>
    <rdfs:comment>The Expression that provides the value of the featureWithValue as its result.</rdfs:comment>
    <rdfs:label>featureValue_Value</rdfs:label>
  </rdf:Property>
  <rdf:Property rdf:about="http://open-services.net/ns/sysmlv2#viewUsage_SatisfiedViewpoint">
    <rdfs:isDefinedBy rdf:resource="http://open-services.net/ns/sysmlv2#"/>
    <rdfs:comment>The nestedRequirements of this ViewUsage that are ViewpointUsages for (additional) viewpoints satisfied by the ViewUsage.</rdfs:comment>
    <rdfs:label>viewUsage_SatisfiedViewpoint</rdfs:label>
  </rdf:Property>
  <rdf:Property rdf:about="http://open-services.net/ns/sysmlv2#allocationUsage_AllocationDefinition">
    <rdfs:isDefinedBy rdf:resource="http://open-services.net/ns/sysmlv2#"/>
    <rdfs:comment>The AllocationDefinitions that are the types of this AllocationUsage.</rdfs:comment>
    <rdfs:label>allocationUsage_AllocationDefinition</rdfs:label>
  </rdf:Property>
  <rdf:Property rdf:about="http://open-services.net/ns/sysmlv2#feature_FeaturingType">
    <rdfs:isDefinedBy rdf:resource="http://open-services.net/ns/sysmlv2#"/>
    <rdfs:comment>Types that feature this Feature, such that any instance in the domain of the Feature must be classified by all of these Types, including at least all the featuringTypes of its typeFeaturings.  If the Feature is chained, then the featuringTypes of the first Feature in the chain are also featuringTypes of the chained Feature.</rdfs:comment>
    <rdfs:label>feature_FeaturingType</rdfs:label>
  </rdf:Property>
  <rdf:Property rdf:about="http://open-services.net/ns/sysmlv2#subsetting_SubsettingFeature">
    <rdfs:isDefinedBy rdf:resource="http://open-services.net/ns/sysmlv2#"/>
    <rdfs:comment>The Feature that is a subset of the subsettedFeature of this Subsetting.</rdfs:comment>
    <rdfs:label>subsetting_SubsettingFeature</rdfs:label>
  </rdf:Property>
  <rdf:Property rdf:about="http://open-services.net/ns/sysmlv2#element_QualifiedName">
    <rdfs:isDefinedBy rdf:resource="http://open-services.net/ns/sysmlv2#"/>
    <rdfs:comment>The full ownership-qualified name of this Element, represented in a form that is valid according to the KerML textual concrete syntax for qualified names (including use of unrestricted name notation and escaped characters, as necessary). The qualifiedName is null if this Element has no owningNamespace or if there is not a complete ownership chain of named Namespaces from a root Namespace to this Element.</rdfs:comment>
    <rdfs:label>element_QualifiedName</rdfs:label>
  </rdf:Property>
  <rdf:Property rdf:about="http://open-services.net/ns/sysmlv2#itemFlow_Interaction">
    <rdfs:isDefinedBy rdf:resource="http://open-services.net/ns/sysmlv2#"/>
    <rdfs:comment>The Interactions that type this ItemFlow. Interactions are both Associations and Behaviors, which can type Connectors and Steps, respectively.</rdfs:comment>
    <rdfs:label>itemFlow_Interaction</rdfs:label>
  </rdf:Property>
  <rdf:Property rdf:about="http://open-services.net/ns/sysmlv2#subclassification_Subclassifier">
    <rdfs:isDefinedBy rdf:resource="http://open-services.net/ns/sysmlv2#"/>
    <rdfs:comment>The more specific Classifier in this Subclassification.</rdfs:comment>
    <rdfs:label>subclassification_Subclassifier</rdfs:label>
  </rdf:Property>
  <rdf:Property rdf:about="http://open-services.net/ns/sysmlv2#import_ImportedElement">
    <rdfs:isDefinedBy rdf:resource="http://open-services.net/ns/sysmlv2#"/>
    <rdfs:comment>The effectively imported Element for this Import. For a MembershipImport, this is the memberElement of the importedMembership. For a NamespaceImport, it is the importedNamespace.</rdfs:comment>
    <rdfs:label>import_ImportedElement</rdfs:label>
  </rdf:Property>
  <rdf:Property rdf:about="http://open-services.net/ns/sysmlv2#usage_NestedUseCase">
    <rdfs:isDefinedBy rdf:resource="http://open-services.net/ns/sysmlv2#"/>
    <rdfs:comment>The UseCaseUsages that are nestedUsages of this Usage.</rdfs:comment>
    <rdfs:label>usage_NestedUseCase</rdfs:label>
  </rdf:Property>
  <rdf:Property rdf:about="http://open-services.net/ns/sysmlv2#requirementDefinition_AssumedConstraint">
    <rdfs:isDefinedBy rdf:resource="http://open-services.net/ns/sysmlv2#"/>
    <rdfs:comment>The owned ConstraintUsages that represent assumptions of this RequirementDefinition, which are the ownedConstraints of the RequirementConstraintMemberships of the RequirementDefinition with kind = assumption.</rdfs:comment>
    <rdfs:label>requirementDefinition_AssumedConstraint</rdfs:label>
  </rdf:Property>
  <rdf:Property rdf:about="http://open-services.net/ns/sysmlv2#annotatingElement_OwnedAnnotatingRelationship">
    <rdfs:isDefinedBy rdf:resource="http://open-services.net/ns/sysmlv2#"/>
    <rdfs:comment>The ownedRelationships of this AnnotatingElement that are Annotations, for which this AnnotatingElement is the annotatingElement.</rdfs:comment>
    <rdfs:label>annotatingElement_OwnedAnnotatingRelationship</rdfs:label>
  </rdf:Property>
  <rdf:Property rdf:about="http://open-services.net/ns/sysmlv2#featureValue_FeatureWithValue">
    <rdfs:isDefinedBy rdf:resource="http://open-services.net/ns/sysmlv2#"/>
    <rdfs:comment>The Feature to be provided a value.</rdfs:comment>
    <rdfs:label>featureValue_FeatureWithValue</rdfs:label>
  </rdf:Property>
  <rdf:Property rdf:about="http://open-services.net/ns/sysmlv2#annotation_AnnotatingElement">
    <rdfs:isDefinedBy rdf:resource="http://open-services.net/ns/sysmlv2#"/>
    <rdfs:comment>The AnnotatingElement that annotates the annotatedElement of this Annotation.</rdfs:comment>
    <rdfs:label>annotation_AnnotatingElement</rdfs:label>
  </rdf:Property>
  <rdf:Property rdf:about="http://open-services.net/ns/sysmlv2#owningMembership_OwnedMemberElement">
    <rdfs:isDefinedBy rdf:resource="http://open-services.net/ns/sysmlv2#"/>
    <rdfs:comment>The Element that becomes an ownedMember of the membershipOwningNamespace due to this OwningMembership.</rdfs:comment>
    <rdfs:label>owningMembership_OwnedMemberElement</rdfs:label>
  </rdf:Property>
  <rdf:Property rdf:about="http://open-services.net/ns/sysmlv2#eventOccurrenceUsage_EventOccurrence">
    <rdfs:isDefinedBy rdf:resource="http://open-services.net/ns/sysmlv2#"/>
    <rdfs:comment>The OccurrenceUsage referenced as an event by this EventOccurrenceUsage. It is the referenceFeature of the ownedReferenceSubsetting for the EventOccurrenceUsage, if there is one, and, otherwise, the EventOccurrenceUsage itself.</rdfs:comment>
    <rdfs:label>eventOccurrenceUsage_EventOccurrence</rdfs:label>
  </rdf:Property>
  <rdf:Property rdf:about="http://open-services.net/ns/sysmlv2#metadataAccessExpression_ReferencedElement">
    <rdfs:isDefinedBy rdf:resource="http://open-services.net/ns/sysmlv2#"/>
    <rdfs:comment> The Element whose metadata is being accessed.</rdfs:comment>
    <rdfs:label>metadataAccessExpression_ReferencedElement</rdfs:label>
  </rdf:Property>
  <rdf:Property rdf:about="http://open-services.net/ns/sysmlv2#occurrenceDefinition_LifeClass">
    <rdfs:isDefinedBy rdf:resource="http://open-services.net/ns/sysmlv2#"/>
    <rdfs:comment>If isIndividual is true, a LifeClass that specializes this OccurrenceDefinition, restricting it to represent an individual.</rdfs:comment>
    <rdfs:label>occurrenceDefinition_LifeClass</rdfs:label>
  </rdf:Property>
  <rdf:Property rdf:about="http://open-services.net/ns/sysmlv2#enumerationDefinition_EnumeratedValue">
    <rdfs:isDefinedBy rdf:resource="http://open-services.net/ns/sysmlv2#"/>
    <rdfs:comment>EnumerationUsages of this EnumerationDefinitionthat have distinct, fixed values. Each enumeratedValue specifies one of the allowed instances of the EnumerationDefinition.</rdfs:comment>
    <rdfs:label>enumerationDefinition_EnumeratedValue</rdfs:label>
  </rdf:Property>
  <rdf:Property rdf:about="http://open-services.net/ns/sysmlv2#satisfyRequirementUsage_SatisfyingFeature">
    <rdfs:isDefinedBy rdf:resource="http://open-services.net/ns/sysmlv2#"/>
    <rdfs:comment>The Feature that represents the actual subject that is asserted to satisfy the satisfiedRequirement. The satisfyingFeature is bound to the subjectParameter of the SatisfyRequirementUsage.</rdfs:comment>
    <rdfs:label>satisfyRequirementUsage_SatisfyingFeature</rdfs:label>
  </rdf:Property>
  <rdf:Property rdf:about="http://open-services.net/ns/sysmlv2#actionDefinition_Action">
    <rdfs:isDefinedBy rdf:resource="http://open-services.net/ns/sysmlv2#"/>
    <rdfs:comment>The ActionUsages that are steps in this ActionDefinition, which define the actions that specify the behavior of the ActionDefinition.</rdfs:comment>
    <rdfs:label>actionDefinition_Action</rdfs:label>
  </rdf:Property>
  <rdf:Property rdf:about="http://open-services.net/ns/sysmlv2#literalBoolean_Value">
    <rdfs:isDefinedBy rdf:resource="http://open-services.net/ns/sysmlv2#"/>
    <rdfs:comment>The Boolean value that is the result of evaluating this LiteralBoolean.</rdfs:comment>
    <rdfs:label>literalBoolean_Value</rdfs:label>
  </rdf:Property>
  <rdf:Property rdf:about="http://open-services.net/ns/sysmlv2#textualRepresentation_RepresentedElement">
    <rdfs:isDefinedBy rdf:resource="http://open-services.net/ns/sysmlv2#"/>
    <rdfs:comment>The Element that is represented by this TextualRepresentation.</rdfs:comment>
    <rdfs:label>textualRepresentation_RepresentedElement</rdfs:label>
  </rdf:Property>
  <rdf:Property rdf:about="http://open-services.net/ns/sysmlv2#objectiveMembership_OwnedObjectiveRequirement">
    <rdfs:isDefinedBy rdf:resource="http://open-services.net/ns/sysmlv2#"/>
    <rdfs:comment>The RequirementUsage that is the ownedMemberFeature of this RequirementUsage.</rdfs:comment>
    <rdfs:label>objectiveMembership_OwnedObjectiveRequirement</rdfs:label>
  </rdf:Property>
  <rdf:Property rdf:about="http://open-services.net/ns/sysmlv2#ifActionUsage_IfArgument">
    <rdfs:isDefinedBy rdf:resource="http://open-services.net/ns/sysmlv2#"/>
    <rdfs:comment>The Expression whose result determines whether the thenAction or (optionally) the elseAction is performed. It is the first parameter of the IfActionUsage.</rdfs:comment>
    <rdfs:label>ifActionUsage_IfArgument</rdfs:label>
  </rdf:Property>
  <rdf:Property rdf:about="http://open-services.net/ns/sysmlv2#conjugation_OwningType">
    <rdfs:isDefinedBy rdf:resource="http://open-services.net/ns/sysmlv2#"/>
    <rdfs:comment>The conjugatedType of this Conjugation that is also its owningRelatedElement.</rdfs:comment>
    <rdfs:label>conjugation_OwningType</rdfs:label>
  </rdf:Property>
  <rdf:Property rdf:about="http://open-services.net/ns/sysmlv2#relationship_Source">
    <rdfs:isDefinedBy rdf:resource="http://open-services.net/ns/sysmlv2#"/>
    <rdfs:comment>The relatedElements from which this Relationship is considered to be directed.</rdfs:comment>
    <rdfs:label>relationship_Source</rdfs:label>
  </rdf:Property>
  <rdf:Property rdf:about="http://open-services.net/ns/sysmlv2#definition_OwnedMetadata">
    <rdfs:isDefinedBy rdf:resource="http://open-services.net/ns/sysmlv2#"/>
    <rdfs:comment>The MetadataUsages that are ownedUsages of this Definition.</rdfs:comment>
    <rdfs:label>definition_OwnedMetadata</rdfs:label>
  </rdf:Property>
  <rdf:Property rdf:about="http://open-services.net/ns/sysmlv2#succession_GuardExpression">
    <rdfs:isDefinedBy rdf:resource="http://open-services.net/ns/sysmlv2#"/>
    <rdfs:comment>Expressions that must evaluate to true before the transitionStep can occur.</rdfs:comment>
    <rdfs:label>succession_GuardExpression</rdfs:label>
  </rdf:Property>
  <rdf:Property rdf:about="http://open-services.net/ns/sysmlv2#requirementUsage_ActorParameter">
    <rdfs:isDefinedBy rdf:resource="http://open-services.net/ns/sysmlv2#"/>
    <rdfs:comment>The parameters of this RequirementUsage that represent actors involved in the requirement.</rdfs:comment>
    <rdfs:label>requirementUsage_ActorParameter</rdfs:label>
  </rdf:Property>
  <rdf:Property rdf:about="http://open-services.net/ns/sysmlv2#step_Parameter">
    <rdfs:isDefinedBy rdf:resource="http://open-services.net/ns/sysmlv2#"/>
    <rdfs:comment>The parameters of this Step, which are defined as its directedFeatures, whose values are passed into and/or out of a performance of the Step.</rdfs:comment>
    <rdfs:label>step_Parameter</rdfs:label>
  </rdf:Property>
  <rdf:Property rdf:about="http://open-services.net/ns/sysmlv2#subclassification_OwningClassifier">
    <rdfs:isDefinedBy rdf:resource="http://open-services.net/ns/sysmlv2#"/>
    <rdfs:comment>The Classifier that owns this Subclassification relationship, which must also be its subclassifier.</rdfs:comment>
    <rdfs:label>subclassification_OwningClassifier</rdfs:label>
  </rdf:Property>
  <rdf:Property rdf:about="http://open-services.net/ns/sysmlv2#caseUsage_ObjectiveRequirement">
    <rdfs:isDefinedBy rdf:resource="http://open-services.net/ns/sysmlv2#"/>
    <rdfs:comment>The RequirementUsage representing the objective of this CaseUsage.</rdfs:comment>
    <rdfs:label>caseUsage_ObjectiveRequirement</rdfs:label>
  </rdf:Property>
  <rdf:Property rdf:about="http://open-services.net/ns/sysmlv2#documentation_DocumentedElement">
    <rdfs:isDefinedBy rdf:resource="http://open-services.net/ns/sysmlv2#"/>
    <rdfs:comment>The Element that is documented by this Documentation.</rdfs:comment>
    <rdfs:label>documentation_DocumentedElement</rdfs:label>
  </rdf:Property>
  <rdf:Property rdf:about="http://open-services.net/ns/sysmlv2#requirementUsage_Text">
    <rdfs:isDefinedBy rdf:resource="http://open-services.net/ns/sysmlv2#"/>
    <rdfs:comment>An optional textual statement of the requirement represented by this RequirementUsage, derived from the bodies of the documentation of the RequirementUsage.</rdfs:comment>
    <rdfs:label>requirementUsage_Text</rdfs:label>
  </rdf:Property>
  <rdf:Property rdf:about="http://open-services.net/ns/sysmlv2#membership_MemberElementId">
    <rdfs:isDefinedBy rdf:resource="http://open-services.net/ns/sysmlv2#"/>
    <rdfs:comment>The elementId of the memberElement.</rdfs:comment>
    <rdfs:label>membership_MemberElementId</rdfs:label>
  </rdf:Property>
  <rdf:Property rdf:about="http://open-services.net/ns/sysmlv2#requirementDefinition_Text">
    <rdfs:isDefinedBy rdf:resource="http://open-services.net/ns/sysmlv2#"/>
    <rdfs:comment>An optional textual statement of the requirement represented by this RequirementDefinition, derived from the bodies of the documentation of the RequirementDefinition.</rdfs:comment>
    <rdfs:label>requirementDefinition_Text</rdfs:label>
  </rdf:Property>
  <rdf:Property rdf:about="http://open-services.net/ns/sysmlv2#portUsage_PortDefinition">
    <rdfs:isDefinedBy rdf:resource="http://open-services.net/ns/sysmlv2#"/>
    <rdfs:comment>The occurrenceDefinitions of this PortUsage, which must all be PortDefinitions.</rdfs:comment>
    <rdfs:label>portUsage_PortDefinition</rdfs:label>
  </rdf:Property>
  <rdf:Property rdf:about="http://open-services.net/ns/sysmlv2#featuring_Type">
    <rdfs:isDefinedBy rdf:resource="http://open-services.net/ns/sysmlv2#"/>
    <rdfs:comment>The Type that features the featureOfType.</rdfs:comment>
    <rdfs:label>featuring_Type</rdfs:label>
  </rdf:Property>
  <rdf:Property rdf:about="http://open-services.net/ns/sysmlv2#useCaseDefinition_IncludedUseCase">
    <rdfs:isDefinedBy rdf:resource="http://open-services.net/ns/sysmlv2#"/>
    <rdfs:comment>The UseCaseUsages that are included by this UseCaseDefinition, which are the useCaseIncludeds of the IncludeUseCaseUsages owned by this UseCaseDefinition.</rdfs:comment>
    <rdfs:label>useCaseDefinition_IncludedUseCase</rdfs:label>
  </rdf:Property>
  <rdf:Property rdf:about="http://open-services.net/ns/sysmlv2#usage_NestedConcern">
    <rdfs:isDefinedBy rdf:resource="http://open-services.net/ns/sysmlv2#"/>
    <rdfs:comment>The ConcernUsages that are nestedUsages of this Usage.</rdfs:comment>
    <rdfs:label>usage_NestedConcern</rdfs:label>
  </rdf:Property>
  <rdf:Property rdf:about="http://open-services.net/ns/sysmlv2#referenceSubsetting_ReferencedFeature">
    <rdfs:isDefinedBy rdf:resource="http://open-services.net/ns/sysmlv2#"/>
    <rdfs:comment>The Feature that is referenced by the referencingFeature of this ReferenceSubsetting.</rdfs:comment>
    <rdfs:label>referenceSubsetting_ReferencedFeature</rdfs:label>
  </rdf:Property>
  <rdf:Property rdf:about="http://open-services.net/ns/sysmlv2#ifActionUsage_ThenAction">
    <rdfs:isDefinedBy rdf:resource="http://open-services.net/ns/sysmlv2#"/>
    <rdfs:comment>The ActionUsage that is to be performed if the result of the ifArgument is true. It is the second parameter of the IfActionUsage.</rdfs:comment>
    <rdfs:label>ifActionUsage_ThenAction</rdfs:label>
  </rdf:Property>
  <rdf:Property rdf:about="http://open-services.net/ns/sysmlv2#transitionUsage_Source">
    <rdfs:isDefinedBy rdf:resource="http://open-services.net/ns/sysmlv2#"/>
    <rdfs:comment>The source ActionUsage of this TransitionUsage, which becomes the source of the succession for the TransitionUsage.</rdfs:comment>
    <rdfs:label>transitionUsage_Source</rdfs:label>
  </rdf:Property>
  <rdf:Property rdf:about="http://open-services.net/ns/sysmlv2#usage_NestedCalculation">
    <rdfs:isDefinedBy rdf:resource="http://open-services.net/ns/sysmlv2#"/>
    <rdfs:comment>The CalculationUsage that are nestedUsages of this Usage.</rdfs:comment>
    <rdfs:label>usage_NestedCalculation</rdfs:label>
  </rdf:Property>
  <rdf:Property rdf:about="http://open-services.net/ns/sysmlv2#membership_MemberElement">
    <rdfs:isDefinedBy rdf:resource="http://open-services.net/ns/sysmlv2#"/>
    <rdfs:comment>The Element that becomes a member of the membershipOwningNamespace due to this Membership.</rdfs:comment>
    <rdfs:label>membership_MemberElement</rdfs:label>
  </rdf:Property>
  <rdf:Property rdf:about="http://open-services.net/ns/sysmlv2#featureValue_IsInitial">
    <rdfs:isDefinedBy rdf:resource="http://open-services.net/ns/sysmlv2#"/>
    <rdfs:comment>Whether this FeatureValue specifies a bound value or an initial value for the featureWithValue.</rdfs:comment>
    <rdfs:label>featureValue_IsInitial</rdfs:label>
  </rdf:Property>
  <rdf:Property rdf:about="http://open-services.net/ns/sysmlv2#type_OwnedDisjoining">
    <rdfs:isDefinedBy rdf:resource="http://open-services.net/ns/sysmlv2#"/>
    <rdfs:comment>The ownedRelationships of this Type that are Disjoinings, for which the Type is the typeDisjoined Type.</rdfs:comment>
    <rdfs:label>type_OwnedDisjoining</rdfs:label>
  </rdf:Property>
  <rdf:Property rdf:about="http://open-services.net/ns/sysmlv2#viewDefinition_View">
    <rdfs:isDefinedBy rdf:resource="http://open-services.net/ns/sysmlv2#"/>
    <rdfs:comment>The usages of this ViewDefinition that are ViewUsages.</rdfs:comment>
    <rdfs:label>viewDefinition_View</rdfs:label>
  </rdf:Property>
  <rdf:Property rdf:about="http://open-services.net/ns/sysmlv2#succession_TriggerStep">
    <rdfs:isDefinedBy rdf:resource="http://open-services.net/ns/sysmlv2#"/>
    <rdfs:comment>Steps that map incoming events to the timing of occurrences of the transitionStep. The values of triggerStep subset the list of acceptable events to be received by a Behavior or the object that performs it.</rdfs:comment>
    <rdfs:label>succession_TriggerStep</rdfs:label>
  </rdf:Property>
  <rdf:Property rdf:about="http://open-services.net/ns/sysmlv2#usage_Definition">
    <rdfs:isDefinedBy rdf:resource="http://open-services.net/ns/sysmlv2#"/>
    <rdfs:comment>The Classifiers that are the types of this Usage. Nominally, these are Definitions, but other kinds of Kernel Classifiers are also allowed, to permit use of Classifiers from the Kernel Model Libraries.</rdfs:comment>
    <rdfs:label>usage_Definition</rdfs:label>
  </rdf:Property>
  <rdf:Property rdf:about="http://open-services.net/ns/sysmlv2#featuring_Feature">
    <rdfs:isDefinedBy rdf:resource="http://open-services.net/ns/sysmlv2#"/>
    <rdfs:comment>The Feature that is featured by the featuringType.</rdfs:comment>
    <rdfs:label>featuring_Feature</rdfs:label>
  </rdf:Property>
  <rdf:Property rdf:about="http://open-services.net/ns/sysmlv2#conjugatedPortDefinition_OriginalPortDefinition">
    <rdfs:isDefinedBy rdf:resource="http://open-services.net/ns/sysmlv2#"/>
    <rdfs:comment>The original PortDefinition for this ConjugatedPortDefinition, which is the owningNamespace of the ConjugatedPortDefinition.</rdfs:comment>
    <rdfs:label>conjugatedPortDefinition_OriginalPortDefinition</rdfs:label>
  </rdf:Property>
  <rdf:Property rdf:about="http://open-services.net/ns/sysmlv2#ifActionUsage_ElseAction">
    <rdfs:isDefinedBy rdf:resource="http://open-services.net/ns/sysmlv2#"/>
    <rdfs:comment>The ActionUsage that is to be performed if the result of the ifArgument is false. It is the (optional) third parameter of the IfActionUsage.</rdfs:comment>
    <rdfs:label>ifActionUsage_ElseAction</rdfs:label>
  </rdf:Property>
  <rdf:Property rdf:about="http://open-services.net/ns/sysmlv2#requirementUsage_FramedConcern">
    <rdfs:isDefinedBy rdf:resource="http://open-services.net/ns/sysmlv2#"/>
    <rdfs:comment>The ConcernUsages framed by this RequirementUsage, which are the ownedConcerns of all FramedConcernMemberships of the RequirementUsage.</rdfs:comment>
    <rdfs:label>requirementUsage_FramedConcern</rdfs:label>
  </rdf:Property>
  <rdf:Property rdf:about="http://open-services.net/ns/sysmlv2#definition_OwnedTransition">
    <rdfs:isDefinedBy rdf:resource="http://open-services.net/ns/sysmlv2#"/>
    <rdfs:comment>The TransitionUsages that are ownedUsages of this Definition.</rdfs:comment>
    <rdfs:label>definition_OwnedTransition</rdfs:label>
  </rdf:Property>
  <rdf:Property rdf:about="http://open-services.net/ns/sysmlv2#membershipImport_ImportedMembership">
    <rdfs:isDefinedBy rdf:resource="http://open-services.net/ns/sysmlv2#"/>
    <rdfs:comment>The Membership to be imported.</rdfs:comment>
    <rdfs:label>membershipImport_ImportedMembership</rdfs:label>
  </rdf:Property>
  <rdf:Property rdf:about="http://open-services.net/ns/sysmlv2#element_OwnedElement">
    <rdfs:isDefinedBy rdf:resource="http://open-services.net/ns/sysmlv2#"/>
    <rdfs:comment>The Elements owned by this Element, derived as the ownedRelatedElements of the ownedRelationships of this Element.</rdfs:comment>
    <rdfs:label>element_OwnedElement</rdfs:label>
  </rdf:Property>
  <rdf:Property rdf:about="http://open-services.net/ns/sysmlv2#featureChaining_FeatureChained">
    <rdfs:isDefinedBy rdf:resource="http://open-services.net/ns/sysmlv2#"/>
    <rdfs:comment>The Feature whose values are partly determined by values of the chainingFeature, as described in Feature::chainingFeature.</rdfs:comment>
    <rdfs:label>featureChaining_FeatureChained</rdfs:label>
  </rdf:Property>
  <rdf:Property rdf:about="http://open-services.net/ns/sysmlv2#stateSubactionMembership_Kind">
    <rdfs:isDefinedBy rdf:resource="http://open-services.net/ns/sysmlv2#"/>
    <rdfs:comment>Whether this StateSubactionMembership is for an entry, do or exit ActionUsage.</rdfs:comment>
    <rdfs:label>stateSubactionMembership_Kind</rdfs:label>
  </rdf:Property>
  <rdf:Property rdf:about="http://open-services.net/ns/sysmlv2#actorMembership_OwnedActorParameter">
    <rdfs:isDefinedBy rdf:resource="http://open-services.net/ns/sysmlv2#"/>
    <rdfs:comment>The PartUsage specifying the actor.</rdfs:comment>
    <rdfs:label>actorMembership_OwnedActorParameter</rdfs:label>
  </rdf:Property>
  <rdf:Property rdf:about="http://open-services.net/ns/sysmlv2#package_FilterCondition">
    <rdfs:isDefinedBy rdf:resource="http://open-services.net/ns/sysmlv2#"/>
    <rdfs:comment>The model-level evaluable Boolean-valued Expression used to filter the members of this Package, which are owned by the Package are via ElementFilterMemberships.</rdfs:comment>
    <rdfs:label>package_FilterCondition</rdfs:label>
  </rdf:Property>
  <rdf:Property rdf:about="http://open-services.net/ns/sysmlv2#transitionUsage_GuardExpression">
    <rdfs:isDefinedBy rdf:resource="http://open-services.net/ns/sysmlv2#"/>
    <rdfs:comment>The Expressions that define the guards of this TransitionUsage, which are the ownedFeatures of the TransitionUsage related to it by TransitionFeatureMemberships with kind = guard, which must all be Expressions.</rdfs:comment>
    <rdfs:label>transitionUsage_GuardExpression</rdfs:label>
  </rdf:Property>
  <rdf:Property rdf:about="http://open-services.net/ns/sysmlv2#definition_OwnedConnection">
    <rdfs:isDefinedBy rdf:resource="http://open-services.net/ns/sysmlv2#"/>
    <rdfs:comment>The ConnectorAsUsages that are ownedUsages of this Definition. Note that this list includes BindingConnectorAsUsages and SuccessionAsUsages, even though these are ConnectorAsUsages but not ConnectionUsages.</rdfs:comment>
    <rdfs:label>definition_OwnedConnection</rdfs:label>
  </rdf:Property>
  <rdf:Property rdf:about="http://open-services.net/ns/sysmlv2#typeFeaturing_FeaturingType">
    <rdfs:isDefinedBy rdf:resource="http://open-services.net/ns/sysmlv2#"/>
    <rdfs:comment>The Type that features the featureOfType. It is the target of the TypeFeaturing.</rdfs:comment>
    <rdfs:label>typeFeaturing_FeaturingType</rdfs:label>
  </rdf:Property>
  <rdf:Property rdf:about="http://open-services.net/ns/sysmlv2#viewpointUsage_ViewpointDefinition">
    <rdfs:isDefinedBy rdf:resource="http://open-services.net/ns/sysmlv2#"/>
    <rdfs:comment>The ViewpointDefinition that is the definition of this ViewpointUsage.</rdfs:comment>
    <rdfs:label>viewpointUsage_ViewpointDefinition</rdfs:label>
  </rdf:Property>
  <rdf:Property rdf:about="http://open-services.net/ns/sysmlv2#itemFlow_TargetInputFeature">
    <rdfs:isDefinedBy rdf:resource="http://open-services.net/ns/sysmlv2#"/>
    <rdfs:comment>The Feature that receives the values carried by the ItemFlow. It must be an owned output of the target participant of the ItemFlow.</rdfs:comment>
    <rdfs:label>itemFlow_TargetInputFeature</rdfs:label>
  </rdf:Property>
  <rdf:Property rdf:about="http://open-services.net/ns/sysmlv2#calculationUsage_CalculationDefinition">
    <rdfs:isDefinedBy rdf:resource="http://open-services.net/ns/sysmlv2#"/>
    <rdfs:comment>The Function that is the type of this CalculationUsage. Nominally, this would be a CalculationDefinition, but a kernel Function is also allowed, to permit use of Functions from the Kernel Model Libraries.</rdfs:comment>
    <rdfs:label>calculationUsage_CalculationDefinition</rdfs:label>
  </rdf:Property>
  <rdf:Property rdf:about="http://open-services.net/ns/sysmlv2#usage_NestedItem">
    <rdfs:isDefinedBy rdf:resource="http://open-services.net/ns/sysmlv2#"/>
    <rdfs:comment>The ItemUsages that are nestedUsages of this Usage.</rdfs:comment>
    <rdfs:label>usage_NestedItem</rdfs:label>
  </rdf:Property>
  <rdf:Property rdf:about="http://open-services.net/ns/sysmlv2#usage_Variant">
    <rdfs:isDefinedBy rdf:resource="http://open-services.net/ns/sysmlv2#"/>
    <rdfs:comment>The Usages which represent the variants of this Usage as a variation point Usage, if isVariation = true. If isVariation = false, then there must be no variants.</rdfs:comment>
    <rdfs:label>usage_Variant</rdfs:label>
  </rdf:Property>
  <rdf:Property rdf:about="http://open-services.net/ns/sysmlv2#verificationCaseUsage_VerificationCaseDefinition">
    <rdfs:isDefinedBy rdf:resource="http://open-services.net/ns/sysmlv2#"/>
    <rdfs:comment>The VerificationCase that is the definition of this VerificationCaseUsage.</rdfs:comment>
    <rdfs:label>verificationCaseUsage_VerificationCaseDefinition</rdfs:label>
  </rdf:Property>
  <rdf:Property rdf:about="http://open-services.net/ns/sysmlv2#definition_IsVariation">
    <rdfs:isDefinedBy rdf:resource="http://open-services.net/ns/sysmlv2#"/>
    <rdfs:comment>Whether this Definition is for a variation point or not. If true, then all the memberships of the Definition must be VariantMemberships.</rdfs:comment>
    <rdfs:label>definition_IsVariation</rdfs:label>
  </rdf:Property>
  <rdf:Property rdf:about="http://open-services.net/ns/sysmlv2#definition_OwnedConcern">
    <rdfs:isDefinedBy rdf:resource="http://open-services.net/ns/sysmlv2#"/>
    <rdfs:comment>The ConcernUsages that are ownedUsages of this Definition.</rdfs:comment>
    <rdfs:label>definition_OwnedConcern</rdfs:label>
  </rdf:Property>
  <rdf:Property rdf:about="http://open-services.net/ns/sysmlv2#stateUsage_IsParallel">
    <rdfs:isDefinedBy rdf:resource="http://open-services.net/ns/sysmlv2#"/>
    <rdfs:comment>Whether the nestedStates of this StateUsage are to all be performed in parallel. If true, none of the nestedActions (which include nestedStates) may have any incoming or outgoing Transitions. If false, only one nestedState may be performed at a time.</rdfs:comment>
    <rdfs:label>stateUsage_IsParallel</rdfs:label>
  </rdf:Property>
  <rdf:Property rdf:about="http://open-services.net/ns/sysmlv2#viewUsage_ExposedElement">
    <rdfs:isDefinedBy rdf:resource="http://open-services.net/ns/sysmlv2#"/>
    <rdfs:comment>The Elements that are exposed by this ViewUsage, which are those memberElements of the imported Memberships from all the Expose Relationships that meet all the owned and inherited viewConditions.</rdfs:comment>
    <rdfs:label>viewUsage_ExposedElement</rdfs:label>
  </rdf:Property>
  <rdf:Property rdf:about="http://open-services.net/ns/sysmlv2#expression_Function">
    <rdfs:isDefinedBy rdf:resource="http://open-services.net/ns/sysmlv2#"/>
    <rdfs:comment>The Function that types this Expression.</rdfs:comment>
    <rdfs:label>expression_Function</rdfs:label>
  </rdf:Property>
  <rdf:Property rdf:about="http://open-services.net/ns/sysmlv2#actionUsage_ActionDefinition">
    <rdfs:isDefinedBy rdf:resource="http://open-services.net/ns/sysmlv2#"/>
    <rdfs:comment>The Behaviors that are the types of this ActionUsage. Nominally, these would be ActionDefinitions, but other kinds of Kernel Behaviors are also allowed, to permit use of Behaviors from the Kernel Model Libraries.</rdfs:comment>
    <rdfs:label>actionUsage_ActionDefinition</rdfs:label>
  </rdf:Property>
  <rdf:Property rdf:about="http://open-services.net/ns/sysmlv2#conjugation_OriginalType">
    <rdfs:isDefinedBy rdf:resource="http://open-services.net/ns/sysmlv2#"/>
    <rdfs:comment>The Type to be conjugated.</rdfs:comment>
    <rdfs:label>conjugation_OriginalType</rdfs:label>
  </rdf:Property>
  <rdf:Property rdf:about="http://open-services.net/ns/sysmlv2#usage_NestedEnumeration">
    <rdfs:isDefinedBy rdf:resource="http://open-services.net/ns/sysmlv2#"/>
    <rdfs:comment>The code&gt;EnumerationUsages that are nestedUsages of this Usage.</rdfs:comment>
    <rdfs:label>usage_NestedEnumeration</rdfs:label>
  </rdf:Property>
  <rdf:Property rdf:about="http://open-services.net/ns/sysmlv2#requirementUsage_ReqId">
    <rdfs:isDefinedBy rdf:resource="http://open-services.net/ns/sysmlv2#"/>
    <rdfs:comment>An optional modeler-specified identifier for this RequirementUsage (used, e.g., to link it to an original requirement text in some source document), which is the declaredShortName for the RequirementUsage.</rdfs:comment>
    <rdfs:label>requirementUsage_ReqId</rdfs:label>
  </rdf:Property>
  <rdf:Property rdf:about="http://open-services.net/ns/sysmlv2#element_OwningNamespace">
    <rdfs:isDefinedBy rdf:resource="http://open-services.net/ns/sysmlv2#"/>
    <rdfs:comment>The Namespace that owns this Element, which is the membershipOwningNamespace of the owningMembership of this Element, if any.</rdfs:comment>
    <rdfs:label>element_OwningNamespace</rdfs:label>
  </rdf:Property>
  <rdf:Property rdf:about="http://open-services.net/ns/sysmlv2#specialization_OwningType">
    <rdfs:isDefinedBy rdf:resource="http://open-services.net/ns/sysmlv2#"/>
    <rdfs:comment>The Type that is the specific Type of this Specialization and owns it as its owningRelatedElement.</rdfs:comment>
    <rdfs:label>specialization_OwningType</rdfs:label>
  </rdf:Property>
  <rdf:Property rdf:about="http://open-services.net/ns/sysmlv2#relationship_IsImplied">
    <rdfs:isDefinedBy rdf:resource="http://open-services.net/ns/sysmlv2#"/>
    <rdfs:comment>Whether this Relationship was generated by tooling to meet semantic rules, rather than being directly created by a modeler.</rdfs:comment>
    <rdfs:label>relationship_IsImplied</rdfs:label>
  </rdf:Property>
  <rdf:Property rdf:about="http://open-services.net/ns/sysmlv2#conjugation_ConjugatedType">
    <rdfs:isDefinedBy rdf:resource="http://open-services.net/ns/sysmlv2#"/>
    <rdfs:comment>The Type that is the result of applying Conjugation to the originalType.</rdfs:comment>
    <rdfs:label>conjugation_ConjugatedType</rdfs:label>
  </rdf:Property>
  <rdf:Property rdf:about="http://open-services.net/ns/sysmlv2#featureTyping_Type">
    <rdfs:isDefinedBy rdf:resource="http://open-services.net/ns/sysmlv2#"/>
    <rdfs:comment>The Type that is being applied by this FeatureTyping.</rdfs:comment>
    <rdfs:label>featureTyping_Type</rdfs:label>
  </rdf:Property>
  <rdf:Property rdf:about="http://open-services.net/ns/sysmlv2#comment_Body">
    <rdfs:isDefinedBy rdf:resource="http://open-services.net/ns/sysmlv2#"/>
    <rdfs:comment>The annotation text for the Comment.</rdfs:comment>
    <rdfs:label>comment_Body</rdfs:label>
  </rdf:Property>
  <rdf:Property rdf:about="http://open-services.net/ns/sysmlv2#parameterMembership_OwnedMemberParameter">
    <rdfs:isDefinedBy rdf:resource="http://open-services.net/ns/sysmlv2#"/>
    <rdfs:comment>The Feature that is identified as a parameter by this ParameterMembership.</rdfs:comment>
    <rdfs:label>parameterMembership_OwnedMemberParameter</rdfs:label>
  </rdf:Property>
  <rdf:Property rdf:about="http://open-services.net/ns/sysmlv2#definition_OwnedPort">
    <rdfs:isDefinedBy rdf:resource="http://open-services.net/ns/sysmlv2#"/>
    <rdfs:comment>The PortUsages that are ownedUsages of this Definition.</rdfs:comment>
    <rdfs:label>definition_OwnedPort</rdfs:label>
  </rdf:Property>
  <rdf:Property rdf:about="http://open-services.net/ns/sysmlv2#featureInverting_OwningFeature">
    <rdfs:isDefinedBy rdf:resource="http://open-services.net/ns/sysmlv2#"/>
    <rdfs:comment>A featureInverted that is also the owningRelatedElement of this FeatureInverting.</rdfs:comment>
    <rdfs:label>featureInverting_OwningFeature</rdfs:label>
  </rdf:Property>
  <rdf:Property rdf:about="http://open-services.net/ns/sysmlv2#intersecting_IntersectingType">
    <rdfs:isDefinedBy rdf:resource="http://open-services.net/ns/sysmlv2#"/>
    <rdfs:comment>Type that partly determines interpretations of typeIntersected, as described in Type::intersectingType.</rdfs:comment>
    <rdfs:label>intersecting_IntersectingType</rdfs:label>
  </rdf:Property>
  <rdf:Property rdf:about="http://open-services.net/ns/sysmlv2#referenceSubsetting_ReferencingFeature">
    <rdfs:isDefinedBy rdf:resource="http://open-services.net/ns/sysmlv2#"/>
    <rdfs:comment>The Feature that owns this ReferenceSubsetting relationship, which is also its subsettingFeature.</rdfs:comment>
    <rdfs:label>referenceSubsetting_ReferencingFeature</rdfs:label>
  </rdf:Property>
  <rdf:Property rdf:about="http://open-services.net/ns/sysmlv2#multiplicityRange_UpperBound">
    <rdfs:isDefinedBy rdf:resource="http://open-services.net/ns/sysmlv2#"/>
    <rdfs:comment>The Expression whose result is the upper bound of the MultiplicityRange.</rdfs:comment>
    <rdfs:label>multiplicityRange_UpperBound</rdfs:label>
  </rdf:Property>
  <rdf:Property rdf:about="http://open-services.net/ns/sysmlv2#type_Multiplicity">
    <rdfs:isDefinedBy rdf:resource="http://open-services.net/ns/sysmlv2#"/>
    <rdfs:comment>An ownedMember of this Type that is a Multiplicity, which constraints the cardinality of the Type. If there is no such ownedMember, then the cardinality of this Type is constrained by all the Multiplicity constraints applicable to any direct supertypes.</rdfs:comment>
    <rdfs:label>type_Multiplicity</rdfs:label>
  </rdf:Property>
  <rdf:Property rdf:about="http://open-services.net/ns/sysmlv2#acceptActionUsage_PayloadParameter">
    <rdfs:isDefinedBy rdf:resource="http://open-services.net/ns/sysmlv2#"/>
    <rdfs:comment>The nestedReference of this AcceptActionUsage that redefines the payload output parameter of the base AcceptActionUsage AcceptAction from the Systems Model Library.</rdfs:comment>
    <rdfs:label>acceptActionUsage_PayloadParameter</rdfs:label>
  </rdf:Property>
  <rdf:Property rdf:about="http://open-services.net/ns/sysmlv2#constraintUsage_ConstraintDefinition">
    <rdfs:isDefinedBy rdf:resource="http://open-services.net/ns/sysmlv2#"/>
    <rdfs:comment>The (single) Predicate that is the type of this ConstraintUsage. Nominally, this will be a ConstraintDefinition, but other kinds of Predicates are also allowed, to permit use of Predicates from the Kernel Model Libraries.</rdfs:comment>
    <rdfs:label>constraintUsage_ConstraintDefinition</rdfs:label>
  </rdf:Property>
  <rdf:Property rdf:about="http://open-services.net/ns/sysmlv2#dependency_Supplier">
    <rdfs:isDefinedBy rdf:resource="http://open-services.net/ns/sysmlv2#"/>
    <rdfs:comment>The Element or Elements on which the client Elements depend in some respect.</rdfs:comment>
    <rdfs:label>dependency_Supplier</rdfs:label>
  </rdf:Property>
  <rdf:Property rdf:about="http://open-services.net/ns/sysmlv2#viewDefinition_SatisfiedViewpoint">
    <rdfs:isDefinedBy rdf:resource="http://open-services.net/ns/sysmlv2#"/>
    <rdfs:comment>The composite ownedRequirements of this ViewDefinition that are ViewpointUsages for viewpoints satisfied by the ViewDefinition.</rdfs:comment>
    <rdfs:label>viewDefinition_SatisfiedViewpoint</rdfs:label>
  </rdf:Property>
  <rdf:Property rdf:about="http://open-services.net/ns/sysmlv2#type_OwnedIntersecting">
    <rdfs:isDefinedBy rdf:resource="http://open-services.net/ns/sysmlv2#"/>
    <rdfs:comment>The ownedRelationships of this Type that are Intersectings, have the Type as their typeIntersected.</rdfs:comment>
    <rdfs:label>type_OwnedIntersecting</rdfs:label>
  </rdf:Property>
  <rdf:Property rdf:about="http://open-services.net/ns/sysmlv2#portConjugation_ConjugatedPortDefinition">
    <rdfs:isDefinedBy rdf:resource="http://open-services.net/ns/sysmlv2#"/>
    <rdfs:comment>The ConjugatedPortDefinition that is conjugate to the originalPortDefinition.</rdfs:comment>
    <rdfs:label>portConjugation_ConjugatedPortDefinition</rdfs:label>
  </rdf:Property>
  <rdf:Property rdf:about="http://open-services.net/ns/sysmlv2#resultExpressionMembership_OwnedResultExpression">
    <rdfs:isDefinedBy rdf:resource="http://open-services.net/ns/sysmlv2#"/>
    <rdfs:comment>The Expression that provides the result for the owner of the ResultExpressionMembership.</rdfs:comment>
    <rdfs:label>resultExpressionMembership_OwnedResultExpression</rdfs:label>
  </rdf:Property>
  <rdf:Property rdf:about="http://open-services.net/ns/sysmlv2#framedConcernMembership_OwnedConcern">
    <rdfs:isDefinedBy rdf:resource="http://open-services.net/ns/sysmlv2#"/>
    <rdfs:comment>The ConcernUsage that is the ownedConstraint of this FramedConcernMembership.</rdfs:comment>
    <rdfs:label>framedConcernMembership_OwnedConcern</rdfs:label>
  </rdf:Property>
  <rdf:Property rdf:about="http://open-services.net/ns/sysmlv2#requirementConstraintMembership_ReferencedConstraint">
    <rdfs:isDefinedBy rdf:resource="http://open-services.net/ns/sysmlv2#"/>
    <rdfs:comment> The ConstraintUsage that is referenced through this RequirementConstraintMembership. It is the referencedFeature of the ownedReferenceSubsetting of the ownedConstraint, if there is one, and, otherwise, the ownedConstraint itself.</rdfs:comment>
    <rdfs:label>requirementConstraintMembership_ReferencedConstraint</rdfs:label>
  </rdf:Property>
  <rdf:Property rdf:about="http://open-services.net/ns/sysmlv2#usage_OwningDefinition">
    <rdfs:isDefinedBy rdf:resource="http://open-services.net/ns/sysmlv2#"/>
    <rdfs:comment>The Definition that owns this Usage (if any).</rdfs:comment>
    <rdfs:label>usage_OwningDefinition</rdfs:label>
  </rdf:Property>
  <rdf:Property rdf:about="http://open-services.net/ns/sysmlv2#type_OwnedSpecialization">
    <rdfs:isDefinedBy rdf:resource="http://open-services.net/ns/sysmlv2#"/>
    <rdfs:comment>The ownedRelationships of this Type that are Specializations, for which the Type is the specific Type.</rdfs:comment>
    <rdfs:label>type_OwnedSpecialization</rdfs:label>
  </rdf:Property>
  <rdf:Property rdf:about="http://open-services.net/ns/sysmlv2#transitionFeatureMembership_Kind">
    <rdfs:isDefinedBy rdf:resource="http://open-services.net/ns/sysmlv2#"/>
    <rdfs:comment>Whether this TransitionFeatureMembership  is for a trigger, guard or effect.</rdfs:comment>
    <rdfs:label>transitionFeatureMembership_Kind</rdfs:label>
  </rdf:Property>
  <rdf:Property rdf:about="http://open-services.net/ns/sysmlv2#caseDefinition_ActorParameter">
    <rdfs:isDefinedBy rdf:resource="http://open-services.net/ns/sysmlv2#"/>
    <rdfs:comment>The parameters of this CaseDefinition that represent actors involved in the case.</rdfs:comment>
    <rdfs:label>caseDefinition_ActorParameter</rdfs:label>
  </rdf:Property>
  <rdf:Property rdf:about="http://open-services.net/ns/sysmlv2#definition_OwnedVerificationCase">
    <rdfs:isDefinedBy rdf:resource="http://open-services.net/ns/sysmlv2#"/>
    <rdfs:comment>The VerificationCaseUsages that are ownedUsages of this Definition.</rdfs:comment>
    <rdfs:label>definition_OwnedVerificationCase</rdfs:label>
  </rdf:Property>
  <rdf:Property rdf:about="http://open-services.net/ns/sysmlv2#namespaceImport_ImportedNamespace">
    <rdfs:isDefinedBy rdf:resource="http://open-services.net/ns/sysmlv2#"/>
    <rdfs:comment>The Namespace whose visible Memberships are imported by this NamespaceImport.</rdfs:comment>
    <rdfs:label>namespaceImport_ImportedNamespace</rdfs:label>
  </rdf:Property>
  <rdf:Property rdf:about="http://open-services.net/ns/sysmlv2#featureTyping_OwningFeature">
    <rdfs:isDefinedBy rdf:resource="http://open-services.net/ns/sysmlv2#"/>
    <rdfs:comment>A typedFeature that is also the owningRelatedElement of this FeatureTyping.</rdfs:comment>
    <rdfs:label>featureTyping_OwningFeature</rdfs:label>
  </rdf:Property>
  <rdf:Property rdf:about="http://open-services.net/ns/sysmlv2#viewDefinition_ViewCondition">
    <rdfs:isDefinedBy rdf:resource="http://open-services.net/ns/sysmlv2#"/>
    <rdfs:comment>The Expressions related to this ViewDefinition by ElementFilterMemberships, which specify conditions on Elements to be rendered in a view.</rdfs:comment>
    <rdfs:label>viewDefinition_ViewCondition</rdfs:label>
  </rdf:Property>
  <rdf:Property rdf:about="http://open-services.net/ns/sysmlv2#interfaceUsage_InterfaceDefinition">
    <rdfs:isDefinedBy rdf:resource="http://open-services.net/ns/sysmlv2#"/>
    <rdfs:comment>The InterfaceDefinitions that type this InterfaceUsage.</rdfs:comment>
    <rdfs:label>interfaceUsage_InterfaceDefinition</rdfs:label>
  </rdf:Property>
  <rdf:Property rdf:about="http://open-services.net/ns/sysmlv2#occurrenceUsage_PortionKind">
    <rdfs:isDefinedBy rdf:resource="http://open-services.net/ns/sysmlv2#"/>
    <rdfs:comment>The kind of (temporal) portion of the life of the occurrenceDefinition represented by this OccurrenceUsage, if it is so restricted.</rdfs:comment>
    <rdfs:label>occurrenceUsage_PortionKind</rdfs:label>
  </rdf:Property>
  <rdf:Property rdf:about="http://open-services.net/ns/sysmlv2#disjoining_DisjoiningType">
    <rdfs:isDefinedBy rdf:resource="http://open-services.net/ns/sysmlv2#"/>
    <rdfs:comment>Type asserted to be disjoint with the typeDisjoined.</rdfs:comment>
    <rdfs:label>disjoining_DisjoiningType</rdfs:label>
  </rdf:Property>
  <rdf:Property rdf:about="http://open-services.net/ns/sysmlv2#occurrenceUsage_IsIndividual">
    <rdfs:isDefinedBy rdf:resource="http://open-services.net/ns/sysmlv2#"/>
    <rdfs:comment>Whether this OccurrenceUsage represents the usage of the specific individual (or portion of it) represented by its individualDefinition.</rdfs:comment>
    <rdfs:label>occurrenceUsage_IsIndividual</rdfs:label>
  </rdf:Property>
  <rdf:Property rdf:about="http://open-services.net/ns/sysmlv2#element_DeclaredShortName">
    <rdfs:isDefinedBy rdf:resource="http://open-services.net/ns/sysmlv2#"/>
    <rdfs:comment>An optional alternative name for the Element that is intended to be shorter or in some way more succinct than its primary name. It may act as a modeler-specified identifier for the Element, though it is then the responsibility of the modeler to maintain the uniqueness of this identifier within a model or relative to some other context.</rdfs:comment>
    <rdfs:label>element_DeclaredShortName</rdfs:label>
  </rdf:Property>
  <rdf:Property rdf:about="http://open-services.net/ns/sysmlv2#allocationDefinition_Allocation">
    <rdfs:isDefinedBy rdf:resource="http://open-services.net/ns/sysmlv2#"/>
    <rdfs:comment>The AllocationUsages that refine the allocation mapping defined by this AllocationDefinition.</rdfs:comment>
    <rdfs:label>allocationDefinition_Allocation</rdfs:label>
  </rdf:Property>
  <rdf:Property rdf:about="http://open-services.net/ns/sysmlv2#conjugatedPortTyping_ConjugatedPortDefinition">
    <rdfs:isDefinedBy rdf:resource="http://open-services.net/ns/sysmlv2#"/>
    <rdfs:comment>The type of this ConjugatedPortTyping considered as a FeatureTyping, which must be a ConjugatedPortDefinition.</rdfs:comment>
    <rdfs:label>conjugatedPortTyping_ConjugatedPortDefinition</rdfs:label>
  </rdf:Property>
  <rdf:Property rdf:about="http://open-services.net/ns/sysmlv2#feature_EndOwningType">
    <rdfs:isDefinedBy rdf:resource="http://open-services.net/ns/sysmlv2#"/>
    <rdfs:comment>The Type that is related to this Feature by an EndFeatureMembership in which the Feature is an ownedMemberFeature.</rdfs:comment>
    <rdfs:label>feature_EndOwningType</rdfs:label>
  </rdf:Property>
  <rdf:Property rdf:about="http://open-services.net/ns/sysmlv2#usage_NestedRequirement">
    <rdfs:isDefinedBy rdf:resource="http://open-services.net/ns/sysmlv2#"/>
    <rdfs:comment>The RequirementUsages that are nestedUsages of this Usage.</rdfs:comment>
    <rdfs:label>usage_NestedRequirement</rdfs:label>
  </rdf:Property>
  <rdf:Property rdf:about="http://open-services.net/ns/sysmlv2#usage_NestedConstraint">
    <rdfs:isDefinedBy rdf:resource="http://open-services.net/ns/sysmlv2#"/>
    <rdfs:comment>The ConstraintUsages that are nestedUsages of this Usage.</rdfs:comment>
    <rdfs:label>usage_NestedConstraint</rdfs:label>
  </rdf:Property>
  <rdf:Property rdf:about="http://open-services.net/ns/sysmlv2#whileLoopActionUsage_WhileArgument">
    <rdfs:isDefinedBy rdf:resource="http://open-services.net/ns/sysmlv2#"/>
    <rdfs:comment>The Expression whose result, if true, determines that the bodyAction should continue to be performed. It is the first owned parameter of the WhileLoopActionUsage.</rdfs:comment>
    <rdfs:label>whileLoopActionUsage_WhileArgument</rdfs:label>
  </rdf:Property>
  <rdf:Property rdf:about="http://open-services.net/ns/sysmlv2#usage_NestedPart">
    <rdfs:isDefinedBy rdf:resource="http://open-services.net/ns/sysmlv2#"/>
    <rdfs:comment>The PartUsages that are nestedUsages of this Usage.</rdfs:comment>
    <rdfs:label>usage_NestedPart</rdfs:label>
  </rdf:Property>
  <rdf:Property rdf:about="http://open-services.net/ns/sysmlv2#type_IsConjugated">
    <rdfs:isDefinedBy rdf:resource="http://open-services.net/ns/sysmlv2#"/>
    <rdfs:comment>Indicates whether this Type has an ownedConjugator.</rdfs:comment>
    <rdfs:label>type_IsConjugated</rdfs:label>
  </rdf:Property>
  <rdf:Property rdf:about="http://open-services.net/ns/sysmlv2#relationship_Target">
    <rdfs:isDefinedBy rdf:resource="http://open-services.net/ns/sysmlv2#"/>
    <rdfs:comment>The relatedElements to which this Relationship is considered to be directed.</rdfs:comment>
    <rdfs:label>relationship_Target</rdfs:label>
  </rdf:Property>
  <rdf:Property rdf:about="http://open-services.net/ns/sysmlv2#acceptActionUsage_ReceiverArgument">
    <rdfs:isDefinedBy rdf:resource="http://open-services.net/ns/sysmlv2#"/>
    <rdfs:comment>An Expression whose result is bound to the receiver input parameter of this AcceptActionUsage.</rdfs:comment>
    <rdfs:label>acceptActionUsage_ReceiverArgument</rdfs:label>
  </rdf:Property>
  <rdf:Property rdf:about="http://open-services.net/ns/sysmlv2#feature_IsPortion">
    <rdfs:isDefinedBy rdf:resource="http://open-services.net/ns/sysmlv2#"/>
    <rdfs:comment>Whether the values of this Feature are contained in the space and time of instances of the domain of the Feature and represent the same thing as those instances.</rdfs:comment>
    <rdfs:label>feature_IsPortion</rdfs:label>
  </rdf:Property>
  <rdf:Property rdf:about="http://open-services.net/ns/sysmlv2#definition_OwnedUseCase">
    <rdfs:isDefinedBy rdf:resource="http://open-services.net/ns/sysmlv2#"/>
    <rdfs:comment>The UseCaseUsages that are ownedUsages of this Definition.</rdfs:comment>
    <rdfs:label>definition_OwnedUseCase</rdfs:label>
  </rdf:Property>
  <rdf:Property rdf:about="http://open-services.net/ns/sysmlv2#membership_MemberShortName">
    <rdfs:isDefinedBy rdf:resource="http://open-services.net/ns/sysmlv2#"/>
    <rdfs:comment>The short name of the memberElement relative to the membershipOwningNamespace.</rdfs:comment>
    <rdfs:label>membership_MemberShortName</rdfs:label>
  </rdf:Property>
  <rdf:Property rdf:about="http://open-services.net/ns/sysmlv2#exhibitStateUsage_ExhibitedState">
    <rdfs:isDefinedBy rdf:resource="http://open-services.net/ns/sysmlv2#"/>
    <rdfs:comment>The StateUsage to be exhibited by the ExhibitStateUsage. It is the performedAction of the ExhibitStateUsage considered as a PerformActionUsage, which must be a StateUsage.</rdfs:comment>
    <rdfs:label>exhibitStateUsage_ExhibitedState</rdfs:label>
  </rdf:Property>
  <rdf:Property rdf:about="http://open-services.net/ns/sysmlv2#succession_TransitionStep">
    <rdfs:isDefinedBy rdf:resource="http://open-services.net/ns/sysmlv2#"/>
    <rdfs:comment>A Step that is typed by the Behavior TransitionPerformances::TransitionPerformance (from the Kernel Semantic Library) that has this Succession as its transitionLink.</rdfs:comment>
    <rdfs:label>succession_TransitionStep</rdfs:label>
  </rdf:Property>
  <rdf:Property rdf:about="http://open-services.net/ns/sysmlv2#subjectMembership_OwnedSubjectParameter">
    <rdfs:isDefinedBy rdf:resource="http://open-services.net/ns/sysmlv2#"/>
    <rdfs:comment>The UsageownedMemberParameter of this SubjectMembership.</rdfs:comment>
    <rdfs:label>subjectMembership_OwnedSubjectParameter</rdfs:label>
  </rdf:Property>
  <rdf:Property rdf:about="http://open-services.net/ns/sysmlv2#usage_NestedInterface">
    <rdfs:isDefinedBy rdf:resource="http://open-services.net/ns/sysmlv2#"/>
    <rdfs:comment>The InterfaceUsages that are nestedUsages of this Usage.</rdfs:comment>
    <rdfs:label>usage_NestedInterface</rdfs:label>
  </rdf:Property>
  <rdf:Property rdf:about="http://open-services.net/ns/sysmlv2#conjugatedPortTyping_PortDefinition">
    <rdfs:isDefinedBy rdf:resource="http://open-services.net/ns/sysmlv2#"/>
    <rdfs:comment>The originalPortDefinition of the conjugatedPortDefinition of this ConjugatedPortTyping.</rdfs:comment>
    <rdfs:label>conjugatedPortTyping_PortDefinition</rdfs:label>
  </rdf:Property>
  <rdf:Property rdf:about="http://open-services.net/ns/sysmlv2#association_RelatedType">
    <rdfs:isDefinedBy rdf:resource="http://open-services.net/ns/sysmlv2#"/>
    <rdfs:comment>The types of the associationEnds of the Association, which are the relatedElements of the Association considered as a Relationship.</rdfs:comment>
    <rdfs:label>association_RelatedType</rdfs:label>
  </rdf:Property>
  <rdf:Property rdf:about="http://open-services.net/ns/sysmlv2#feature_IsDerived">
    <rdfs:isDefinedBy rdf:resource="http://open-services.net/ns/sysmlv2#"/>
    <rdfs:comment>Whether the values of this Feature can always be computed from the values of other Features.</rdfs:comment>
    <rdfs:label>feature_IsDerived</rdfs:label>
  </rdf:Property>
  <rdf:Property rdf:about="http://open-services.net/ns/sysmlv2#multiplicityRange_LowerBound">
    <rdfs:isDefinedBy rdf:resource="http://open-services.net/ns/sysmlv2#"/>
    <rdfs:comment>The Expression whose result provides the lower bound of the MultiplicityRange. If no lowerBound Expression is given, then the lower bound shall have the same value as the upper bound, unless the upper bound is unbounded (*), in which case the lower bound shall be 0.</rdfs:comment>
    <rdfs:label>multiplicityRange_LowerBound</rdfs:label>
  </rdf:Property>
  <rdf:Property rdf:about="http://open-services.net/ns/sysmlv2#connector_SourceFeature">
    <rdfs:isDefinedBy rdf:resource="http://open-services.net/ns/sysmlv2#"/>
    <rdfs:comment>The source relatedFeature for this Connector. It is the first relatedFeature.</rdfs:comment>
    <rdfs:label>connector_SourceFeature</rdfs:label>
  </rdf:Property>
  <rdf:Property rdf:about="http://open-services.net/ns/sysmlv2#element_ShortName">
    <rdfs:isDefinedBy rdf:resource="http://open-services.net/ns/sysmlv2#"/>
    <rdfs:comment>The short name to be used for this Element during name resolution within its owningNamespace. This is derived using the effectiveShortName() operation. By default, it is the same as the declaredShortName, but this is overridden for certain kinds of Elements to compute a shortName even when the declaredName is null.</rdfs:comment>
    <rdfs:label>element_ShortName</rdfs:label>
  </rdf:Property>
  <rdf:Property rdf:about="http://open-services.net/ns/sysmlv2#usage_IsReference">
    <rdfs:isDefinedBy rdf:resource="http://open-services.net/ns/sysmlv2#"/>
    <rdfs:comment>Whether this Usage is a referential Usage, that is, it has isComposite = false.</rdfs:comment>
    <rdfs:label>usage_IsReference</rdfs:label>
  </rdf:Property>
  <rdf:Property rdf:about="http://open-services.net/ns/sysmlv2#element_ElementId">
    <rdfs:isDefinedBy rdf:resource="http://open-services.net/ns/sysmlv2#"/>
    <rdfs:comment>The globally unique identifier for this Element. This is intended to be set by tooling, and it must not change during the lifetime of the Element.</rdfs:comment>
    <rdfs:label>element_ElementId</rdfs:label>
  </rdf:Property>
  <rdf:Property rdf:about="http://open-services.net/ns/sysmlv2#feature_OwnedTyping">
    <rdfs:isDefinedBy rdf:resource="http://open-services.net/ns/sysmlv2#"/>
    <rdfs:comment>The ownedSpecializations of this Feature that are FeatureTypings, for which the Feature is the typedFeature.</rdfs:comment>
    <rdfs:label>feature_OwnedTyping</rdfs:label>
  </rdf:Property>
  <rdf:Property rdf:about="http://open-services.net/ns/sysmlv2#usage_NestedMetadata">
    <rdfs:isDefinedBy rdf:resource="http://open-services.net/ns/sysmlv2#"/>
    <rdfs:comment>The MetadataUsages that are nestedUsages of this of this Usage.</rdfs:comment>
    <rdfs:label>usage_NestedMetadata</rdfs:label>
  </rdf:Property>
  <rdf:Property rdf:about="http://open-services.net/ns/sysmlv2#definition_OwnedFlow">
    <rdfs:isDefinedBy rdf:resource="http://open-services.net/ns/sysmlv2#"/>
    <rdfs:comment>The FlowConnectionUsages that are ownedUsages of this Definition.</rdfs:comment>
    <rdfs:label>definition_OwnedFlow</rdfs:label>
  </rdf:Property>
  <rdf:Property rdf:about="http://open-services.net/ns/sysmlv2#namespace_OwnedImport">
    <rdfs:isDefinedBy rdf:resource="http://open-services.net/ns/sysmlv2#"/>
    <rdfs:comment>The ownedRelationships of this Namespace that are Imports, for which the Namespace is the importOwningNamespace.</rdfs:comment>
    <rdfs:label>namespace_OwnedImport</rdfs:label>
  </rdf:Property>
  <rdf:Property rdf:about="http://open-services.net/ns/sysmlv2#usage_NestedAction">
    <rdfs:isDefinedBy rdf:resource="http://open-services.net/ns/sysmlv2#"/>
    <rdfs:comment>The ActionUsages that are nestedUsages of this Usage.</rdfs:comment>
    <rdfs:label>usage_NestedAction</rdfs:label>
  </rdf:Property>
  <rdf:Property rdf:about="http://open-services.net/ns/sysmlv2#enumerationUsage_EnumerationDefinition">
    <rdfs:isDefinedBy rdf:resource="http://open-services.net/ns/sysmlv2#"/>
    <rdfs:comment>The single EnumerationDefinition that is the type of this EnumerationUsage.</rdfs:comment>
    <rdfs:label>enumerationUsage_EnumerationDefinition</rdfs:label>
  </rdf:Property>
  <rdf:Property rdf:about="http://open-services.net/ns/sysmlv2#element_AliasIds">
    <rdfs:isDefinedBy rdf:resource="http://open-services.net/ns/sysmlv2#"/>
    <rdfs:comment>Various alternative identifiers for this Element. Generally, these will be set by tools.</rdfs:comment>
    <rdfs:label>element_AliasIds</rdfs:label>
  </rdf:Property>
  <rdf:Property rdf:about="http://open-services.net/ns/sysmlv2#itemFlow_SourceOutputFeature">
    <rdfs:isDefinedBy rdf:resource="http://open-services.net/ns/sysmlv2#"/>
    <rdfs:comment>The Feature that provides the items carried by the ItemFlow. It must be an owned output of the source of the ItemFlow.</rdfs:comment>
    <rdfs:label>itemFlow_SourceOutputFeature</rdfs:label>
  </rdf:Property>
  <rdf:Property rdf:about="http://open-services.net/ns/sysmlv2#usage_Usage">
    <rdfs:isDefinedBy rdf:resource="http://open-services.net/ns/sysmlv2#"/>
    <rdfs:comment>The Usages that are features of this Usage (not necessarily owned).</rdfs:comment>
    <rdfs:label>usage_Usage</rdfs:label>
  </rdf:Property>
  <rdf:Property rdf:about="http://open-services.net/ns/sysmlv2#verificationCaseUsage_VerifiedRequirement">
    <rdfs:isDefinedBy rdf:resource="http://open-services.net/ns/sysmlv2#"/>
    <rdfs:comment>The RequirementUsages verified by this VerificationCaseUsage, which are the verifiedRequirements of all RequirementVerificationMemberships of the objectiveRequirement.</rdfs:comment>
    <rdfs:label>verificationCaseUsage_VerifiedRequirement</rdfs:label>
  </rdf:Property>
  <rdf:Property rdf:about="http://open-services.net/ns/sysmlv2#acceptActionUsage_PayloadArgument">
    <rdfs:isDefinedBy rdf:resource="http://open-services.net/ns/sysmlv2#"/>
    <rdfs:comment>An Expression whose result is bound to the payload parameter of this AcceptActionUsage. If provided, the AcceptActionUsage will only accept a Transfer with exactly this payload.</rdfs:comment>
    <rdfs:label>acceptActionUsage_PayloadArgument</rdfs:label>
  </rdf:Property>
  <rdf:Property rdf:about="http://open-services.net/ns/sysmlv2#feature_OwnedReferenceSubsetting">
    <rdfs:isDefinedBy rdf:resource="http://open-services.net/ns/sysmlv2#"/>
    <rdfs:comment>The one ownedSubsetting of this Feature, if any, that is a ReferenceSubsetting, for which the Feature is the referencingFeature.</rdfs:comment>
    <rdfs:label>feature_OwnedReferenceSubsetting</rdfs:label>
  </rdf:Property>
  <rdf:Property rdf:about="http://open-services.net/ns/sysmlv2#transitionUsage_Succession">
    <rdfs:isDefinedBy rdf:resource="http://open-services.net/ns/sysmlv2#"/>
    <rdfs:comment>The Succession that is the ownedFeature of this TransitionUsage, which, if the TransitionUsage is triggered, asserts the temporal ordering of the source and target.</rdfs:comment>
    <rdfs:label>transitionUsage_Succession</rdfs:label>
  </rdf:Property>
  <rdf:Property rdf:about="http://open-services.net/ns/sysmlv2#connector_Association">
    <rdfs:isDefinedBy rdf:resource="http://open-services.net/ns/sysmlv2#"/>
    <rdfs:comment>The Associations that type the Connector.</rdfs:comment>
    <rdfs:label>connector_Association</rdfs:label>
  </rdf:Property>
  <rdf:Property rdf:about="http://open-services.net/ns/sysmlv2#usage_IsVariation">
    <rdfs:isDefinedBy rdf:resource="http://open-services.net/ns/sysmlv2#"/>
    <rdfs:comment>Whether this Usage is for a variation point or not. If true, then all the memberships of the Usage must be VariantMemberships.</rdfs:comment>
    <rdfs:label>usage_IsVariation</rdfs:label>
  </rdf:Property>
  <rdf:Property rdf:about="http://open-services.net/ns/sysmlv2#feature_ChainingFeature">
    <rdfs:isDefinedBy rdf:resource="http://open-services.net/ns/sysmlv2#"/>
    <rdfs:comment>The Feature that are chained together to determine the values of this Feature, derived from the chainingFeatures of the ownedFeatureChainings of this Feature, in the same order. The values of a Feature with chainingFeatures are the same as values of the last Feature in the chain, which can be found by starting with the values of the first Feature (for each instance of the domain of the original Feature), then using each of those as domain instances to find the values of the second Feature in chainingFeatures, and so on, to values of the last Feature.</rdfs:comment>
    <rdfs:label>feature_ChainingFeature</rdfs:label>
  </rdf:Property>
  <rdf:Property rdf:about="http://open-services.net/ns/sysmlv2#viewDefinition_ViewRendering">
    <rdfs:isDefinedBy rdf:resource="http://open-services.net/ns/sysmlv2#"/>
    <rdfs:comment>The RenderingUsage to be used to render views defined by this ViewDefinition, which is the referencedRendering of the ViewRenderingMembership of the ViewDefinition.</rdfs:comment>
    <rdfs:label>viewDefinition_ViewRendering</rdfs:label>
  </rdf:Property>
  <rdf:Property rdf:about="http://open-services.net/ns/sysmlv2#membership_MemberName">
    <rdfs:isDefinedBy rdf:resource="http://open-services.net/ns/sysmlv2#"/>
    <rdfs:comment>The name of the memberElement relative to the membershipOwningNamespace.</rdfs:comment>
    <rdfs:label>membership_MemberName</rdfs:label>
  </rdf:Property>
  <rdf:Property rdf:about="http://open-services.net/ns/sysmlv2#type_InheritedFeature">
    <rdfs:isDefinedBy rdf:resource="http://open-services.net/ns/sysmlv2#"/>
    <rdfs:comment>All the memberFeatures of the inheritedMemberships of this Type that are FeatureMemberships.</rdfs:comment>
    <rdfs:label>type_InheritedFeature</rdfs:label>
  </rdf:Property>
  <rdf:Property rdf:about="http://open-services.net/ns/sysmlv2#disjoining_TypeDisjoined">
    <rdfs:isDefinedBy rdf:resource="http://open-services.net/ns/sysmlv2#"/>
    <rdfs:comment>Type asserted to be disjoint with the disjoiningType.</rdfs:comment>
    <rdfs:label>disjoining_TypeDisjoined</rdfs:label>
  </rdf:Property>
  <rdf:Property rdf:about="http://open-services.net/ns/sysmlv2#element_OwningRelationship">
    <rdfs:isDefinedBy rdf:resource="http://open-services.net/ns/sysmlv2#"/>
    <rdfs:comment>The Relationship for which this Element is an ownedRelatedElement, if any.</rdfs:comment>
    <rdfs:label>element_OwningRelationship</rdfs:label>
  </rdf:Property>
  <rdf:Property rdf:about="http://open-services.net/ns/sysmlv2#stateUsage_ExitAction">
    <rdfs:isDefinedBy rdf:resource="http://open-services.net/ns/sysmlv2#"/>
    <rdfs:comment>The ActionUsage of this StateUsage to be performed on exit to the state defined by the StateDefinition. It is the owned ActionUsage related to the StateUsage by a StateSubactionMembership  with kind = exit.</rdfs:comment>
    <rdfs:label>stateUsage_ExitAction</rdfs:label>
  </rdf:Property>
  <rdf:Property rdf:about="http://open-services.net/ns/sysmlv2#definition_Variant">
    <rdfs:isDefinedBy rdf:resource="http://open-services.net/ns/sysmlv2#"/>
    <rdfs:comment>The Usages which represent the variants of this Definition as a variation point Definition, if isVariation = true. If isVariation = false, the there must be no variants.</rdfs:comment>
    <rdfs:label>definition_Variant</rdfs:label>
  </rdf:Property>
  <rdf:Property rdf:about="http://open-services.net/ns/sysmlv2#type_IntersectingType">
    <rdfs:isDefinedBy rdf:resource="http://open-services.net/ns/sysmlv2#"/>
    <rdfs:comment>The interpretations of a Type with intersectingTypes are asserted to be those in common among the intersectingTypes, which are the Types derived from the intersectingType of the ownedIntersectings of this Type. For example, a Classifier might be an intersection of Classifiers for people of a particular sex and of a particular nationality. Similarly, a feature for people's children of a particular sex might be the intersection of a Feature for their children and a Classifier for people of that sex (because the interpretations of the children Feature that identify those of that sex are also interpretations of the Classifier for that sex).</rdfs:comment>
    <rdfs:label>type_IntersectingType</rdfs:label>
  </rdf:Property>
  <rdf:Property rdf:about="http://open-services.net/ns/sysmlv2#specialization_General">
    <rdfs:isDefinedBy rdf:resource="http://open-services.net/ns/sysmlv2#"/>
    <rdfs:comment>A Type with a superset of all instances of the specific Type, which might be the same set.</rdfs:comment>
    <rdfs:label>specialization_General</rdfs:label>
  </rdf:Property>
  <rdf:Property rdf:about="http://open-services.net/ns/sysmlv2#variantMembership_OwnedVariantUsage">
    <rdfs:isDefinedBy rdf:resource="http://open-services.net/ns/sysmlv2#"/>
    <rdfs:comment>The Usage that represents a variant in the context of the owningVariationDefinition or owningVariationUsage.</rdfs:comment>
    <rdfs:label>variantMembership_OwnedVariantUsage</rdfs:label>
  </rdf:Property>
  <rdf:Property rdf:about="http://open-services.net/ns/sysmlv2#stateDefinition_DoAction">
    <rdfs:isDefinedBy rdf:resource="http://open-services.net/ns/sysmlv2#"/>
    <rdfs:comment>The ActionUsage of this StateDefinition to be performed while in the state defined by the StateDefinition. It is the owned ActionUsage related to the StateDefinition by a StateSubactionMembership  with kind = do.</rdfs:comment>
    <rdfs:label>stateDefinition_DoAction</rdfs:label>
  </rdf:Property>
  <rdf:Property rdf:about="http://open-services.net/ns/sysmlv2#definition_OwnedRendering">
    <rdfs:isDefinedBy rdf:resource="http://open-services.net/ns/sysmlv2#"/>
    <rdfs:comment>The RenderingUsages that are ownedUsages of this Definition.</rdfs:comment>
    <rdfs:label>definition_OwnedRendering</rdfs:label>
  </rdf:Property>
  <rdf:Property rdf:about="http://open-services.net/ns/sysmlv2#performActionUsage_PerformedAction">
    <rdfs:isDefinedBy rdf:resource="http://open-services.net/ns/sysmlv2#"/>
    <rdfs:comment>The ActionUsage to be performed by this PerformedActionUsage. It is the eventOccurrence of the PerformActionUsage considered as an EventOccurrenceUsage, which must be an ActionUsage.</rdfs:comment>
    <rdfs:label>performActionUsage_PerformedAction</rdfs:label>
  </rdf:Property>
  <rdf:Property rdf:about="http://open-services.net/ns/sysmlv2#element_IsLibraryElement">
    <rdfs:isDefinedBy rdf:resource="http://open-services.net/ns/sysmlv2#"/>
    <rdfs:comment>Whether this Element is contained in the ownership tree of a library model.</rdfs:comment>
    <rdfs:label>element_IsLibraryElement</rdfs:label>
  </rdf:Property>
  <rdf:Property rdf:about="http://open-services.net/ns/sysmlv2#feature_IsReadOnly">
    <rdfs:isDefinedBy rdf:resource="http://open-services.net/ns/sysmlv2#"/>
    <rdfs:comment>Whether the values of this Feature can change over the lifetime of an instance of the domain.</rdfs:comment>
    <rdfs:label>feature_IsReadOnly</rdfs:label>
  </rdf:Property>
  <rdf:Property rdf:about="http://open-services.net/ns/sysmlv2#membership_Visibility">
    <rdfs:isDefinedBy rdf:resource="http://open-services.net/ns/sysmlv2#"/>
    <rdfs:comment>Whether or not the Membership of the memberElement in the membershipOwningNamespace is publicly visible outside that Namespace.</rdfs:comment>
    <rdfs:label>membership_Visibility</rdfs:label>
  </rdf:Property>
  <rdf:Property rdf:about="http://open-services.net/ns/sysmlv2#occurrenceDefinition_IsIndividual">
    <rdfs:isDefinedBy rdf:resource="http://open-services.net/ns/sysmlv2#"/>
    <rdfs:comment>Whether this OccurrenceDefinition is constrained to represent single individual.</rdfs:comment>
    <rdfs:label>occurrenceDefinition_IsIndividual</rdfs:label>
  </rdf:Property>
  <rdf:Property rdf:about="http://open-services.net/ns/sysmlv2#unioning_TypeUnioned">
    <rdfs:isDefinedBy rdf:resource="http://open-services.net/ns/sysmlv2#"/>
    <rdfs:comment>Type with interpretations partly determined by unioningType, as described in Type::unioningType.</rdfs:comment>
    <rdfs:label>unioning_TypeUnioned</rdfs:label>
  </rdf:Property>
  <rdf:Property rdf:about="http://open-services.net/ns/sysmlv2#portConjugation_OriginalPortDefinition">
    <rdfs:isDefinedBy rdf:resource="http://open-services.net/ns/sysmlv2#"/>
    <rdfs:comment>The PortDefinition being conjugated.</rdfs:comment>
    <rdfs:label>portConjugation_OriginalPortDefinition</rdfs:label>
  </rdf:Property>
  <rdf:Property rdf:about="http://open-services.net/ns/sysmlv2#requirementUsage_RequirementDefinition">
    <rdfs:isDefinedBy rdf:resource="http://open-services.net/ns/sysmlv2#"/>
    <rdfs:comment>The RequirementDefinition that is the single definition of this RequirementUsage.</rdfs:comment>
    <rdfs:label>requirementUsage_RequirementDefinition</rdfs:label>
  </rdf:Property>
  <rdf:Property rdf:about="http://open-services.net/ns/sysmlv2#membership_MembershipOwningNamespace">
    <rdfs:isDefinedBy rdf:resource="http://open-services.net/ns/sysmlv2#"/>
    <rdfs:comment>The Namespace of which the memberElement becomes a member due to this Membership.</rdfs:comment>
    <rdfs:label>membership_MembershipOwningNamespace</rdfs:label>
  </rdf:Property>
  <rdf:Property rdf:about="http://open-services.net/ns/sysmlv2#definition_DirectedUsage">
    <rdfs:isDefinedBy rdf:resource="http://open-services.net/ns/sysmlv2#"/>
    <rdfs:comment>The usages of this Definition that are directedFeatures.</rdfs:comment>
    <rdfs:label>definition_DirectedUsage</rdfs:label>
  </rdf:Property>
  <rdf:Property rdf:about="http://open-services.net/ns/sysmlv2#usage_NestedAllocation">
    <rdfs:isDefinedBy rdf:resource="http://open-services.net/ns/sysmlv2#"/>
    <rdfs:comment>The AllocationUsages that are nestedUsages of this Usage.</rdfs:comment>
    <rdfs:label>usage_NestedAllocation</rdfs:label>
  </rdf:Property>
  <rdf:Property rdf:about="http://open-services.net/ns/sysmlv2#requirementUsage_SubjectParameter">
    <rdfs:isDefinedBy rdf:resource="http://open-services.net/ns/sysmlv2#"/>
    <rdfs:comment>The parameter of this RequirementUsage that represents its subject.</rdfs:comment>
    <rdfs:label>requirementUsage_SubjectParameter</rdfs:label>
  </rdf:Property>
  <rdf:Property rdf:about="http://open-services.net/ns/sysmlv2#subclassification_Superclassifier">
    <rdfs:isDefinedBy rdf:resource="http://open-services.net/ns/sysmlv2#"/>
    <rdfs:comment>The more general Classifier in this Subclassification.</rdfs:comment>
    <rdfs:label>subclassification_Superclassifier</rdfs:label>
  </rdf:Property>
  <rdf:Property rdf:about="http://open-services.net/ns/sysmlv2#import_IsRecursive">
    <rdfs:isDefinedBy rdf:resource="http://open-services.net/ns/sysmlv2#"/>
    <rdfs:comment>Whether to recursively import Memberships from visible, owned sub-Namespaces.</rdfs:comment>
    <rdfs:label>import_IsRecursive</rdfs:label>
  </rdf:Property>
  <rdf:Property rdf:about="http://open-services.net/ns/sysmlv2#occurrenceUsage_IndividualDefinition">
    <rdfs:isDefinedBy rdf:resource="http://open-services.net/ns/sysmlv2#"/>
    <rdfs:comment>The at most one occurrenceDefinition that has isIndividual = true.</rdfs:comment>
    <rdfs:label>occurrenceUsage_IndividualDefinition</rdfs:label>
  </rdf:Property>
  <oslc_sysmlv2:TransitionFeatureKind rdf:about="http://open-services.net/ns/sysmlv2#transitionFeatureKind_Effect">
    <rdfs:isDefinedBy rdf:resource="http://open-services.net/ns/sysmlv2#"/>
    <rdfs:comment>Indicates that the transitionFeature of a TransitionFeatureMembership is an effectAction.</rdfs:comment>
    <rdfs:label>transitionFeatureKind_Effect</rdfs:label>
  </oslc_sysmlv2:TransitionFeatureKind>
  <oslc_sysmlv2:RequirementConstraintKind rdf:about="http://open-services.net/ns/sysmlv2#requirementConstraintKind_Requirement">
    <rdfs:isDefinedBy rdf:resource="http://open-services.net/ns/sysmlv2#"/>
    <rdfs:comment>Indicates that a member ConstraintUsage of a RequirementDefinition or RequirementUsagerepresents an requirement.</rdfs:comment>
    <rdfs:label>requirementConstraintKind_Requirement</rdfs:label>
  </oslc_sysmlv2:RequirementConstraintKind>
  <oslc_sysmlv2:PortionKind rdf:about="http://open-services.net/ns/sysmlv2#portionKind_Snapshot">
    <rdfs:isDefinedBy rdf:resource="http://open-services.net/ns/sysmlv2#"/>
    <rdfs:comment>A snapshot of an Occurrence (a time slice with zero duration).</rdfs:comment>
    <rdfs:label>portionKind_Snapshot</rdfs:label>
  </oslc_sysmlv2:PortionKind>
  <oslc_sysmlv2:VisibilityKind rdf:about="http://open-services.net/ns/sysmlv2#visibilityKind_Private">
    <rdfs:isDefinedBy rdf:resource="http://open-services.net/ns/sysmlv2#"/>
    <rdfs:comment>Indicates a Membership is not visible outside its owning Namespace.</rdfs:comment>
    <rdfs:label>visibilityKind_Private</rdfs:label>
  </oslc_sysmlv2:VisibilityKind>
  <oslc_sysmlv2:VisibilityKind rdf:about="http://open-services.net/ns/sysmlv2#visibilityKind_Public">
    <rdfs:isDefinedBy rdf:resource="http://open-services.net/ns/sysmlv2#"/>
    <rdfs:comment>Indicates that a Membership is publicly visible outside its owning Namespace.</rdfs:comment>
    <rdfs:label>visibilityKind_Public</rdfs:label>
  </oslc_sysmlv2:VisibilityKind>
  <oslc_sysmlv2:TriggerKind rdf:about="http://open-services.net/ns/sysmlv2#triggerKind_After">
    <rdfs:isDefinedBy rdf:resource="http://open-services.net/ns/sysmlv2#"/>
    <rdfs:comment>Indicates a relative time trigger, corresponding to the TriggerAfter Function from the Triggers model in the Kernel Semantic Library.</rdfs:comment>
    <rdfs:label>triggerKind_After</rdfs:label>
  </oslc_sysmlv2:TriggerKind>
  <oslc_sysmlv2:TriggerKind rdf:about="http://open-services.net/ns/sysmlv2#triggerKind_When">
    <rdfs:isDefinedBy rdf:resource="http://open-services.net/ns/sysmlv2#"/>
    <rdfs:comment>Indicates a change trigger, corresponding to the TriggerWhen Function from the Triggers model in the Kernel Semantic Library.</rdfs:comment>
    <rdfs:label>triggerKind_When</rdfs:label>
  </oslc_sysmlv2:TriggerKind>
  <oslc_sysmlv2:TransitionFeatureKind rdf:about="http://open-services.net/ns/sysmlv2#transitionFeatureKind_Trigger">
    <rdfs:isDefinedBy rdf:resource="http://open-services.net/ns/sysmlv2#"/>
    <rdfs:comment>Indicates that the transitionFeature of a TransitionFeatureMembership is a triggerAction.</rdfs:comment>
    <rdfs:label>transitionFeatureKind_Trigger</rdfs:label>
  </oslc_sysmlv2:TransitionFeatureKind>
  <oslc_sysmlv2:TransitionFeatureKind rdf:about="http://open-services.net/ns/sysmlv2#transitionFeatureKind_Guard">
    <rdfs:isDefinedBy rdf:resource="http://open-services.net/ns/sysmlv2#"/>
    <rdfs:comment>Indicates that the transitionFeature of a TransitionFeatureMembership is a guardExpression.</rdfs:comment>
    <rdfs:label>transitionFeatureKind_Guard</rdfs:label>
  </oslc_sysmlv2:TransitionFeatureKind>
  <oslc_sysmlv2:TriggerKind rdf:about="http://open-services.net/ns/sysmlv2#triggerKind_At">
    <rdfs:isDefinedBy rdf:resource="http://open-services.net/ns/sysmlv2#"/>
    <rdfs:comment>Indicates an absolute time trigger, corresponding to the TriggerAt Function from the Triggers model in the Kernel Semantic Library.</rdfs:comment>
    <rdfs:label>triggerKind_At</rdfs:label>
  </oslc_sysmlv2:TriggerKind>
  <oslc_sysmlv2:StateSubactionKind rdf:about="http://open-services.net/ns/sysmlv2#stateSubactionKind_Exit">
    <rdfs:isDefinedBy rdf:resource="http://open-services.net/ns/sysmlv2#"/>
    <rdfs:comment>Indicates that the action of a StateSubactionMembership is an exitAction.</rdfs:comment>
    <rdfs:label>stateSubactionKind_Exit</rdfs:label>
  </oslc_sysmlv2:StateSubactionKind>
  <oslc_sysmlv2:StateSubactionKind rdf:about="http://open-services.net/ns/sysmlv2#stateSubactionKind_Do">
    <rdfs:isDefinedBy rdf:resource="http://open-services.net/ns/sysmlv2#"/>
    <rdfs:comment>Indicates that the action of a StateSubactionMembership is a doAction.</rdfs:comment>
    <rdfs:label>stateSubactionKind_Do</rdfs:label>
  </oslc_sysmlv2:StateSubactionKind>
  <oslc_sysmlv2:RequirementConstraintKind rdf:about="http://open-services.net/ns/sysmlv2#requirementConstraintKind_Assumption">
    <rdfs:isDefinedBy rdf:resource="http://open-services.net/ns/sysmlv2#"/>
    <rdfs:comment>Indicates that a member ConstraintUsage of a RequirementDefinition or RequirementUsage represents an assumption.</rdfs:comment>
    <rdfs:label>requirementConstraintKind_Assumption</rdfs:label>
  </oslc_sysmlv2:RequirementConstraintKind>
  <oslc_sysmlv2:PortionKind rdf:about="http://open-services.net/ns/sysmlv2#portionKind_Timeslice">
    <rdfs:isDefinedBy rdf:resource="http://open-services.net/ns/sysmlv2#"/>
    <rdfs:comment>A time slice of an Occurrence (a portion over time).</rdfs:comment>
    <rdfs:label>portionKind_Timeslice</rdfs:label>
  </oslc_sysmlv2:PortionKind>
  <oslc_sysmlv2:FeatureDirectionKind rdf:about="http://open-services.net/ns/sysmlv2#featureDirectionKind_Out">
    <rdfs:isDefinedBy rdf:resource="http://open-services.net/ns/sysmlv2#"/>
    <rdfs:comment>Values of the Feature on each instance of its domain are determined internally to that instance and used externally.</rdfs:comment>
    <rdfs:label>featureDirectionKind_Out</rdfs:label>
  </oslc_sysmlv2:FeatureDirectionKind>
  <oslc_sysmlv2:FeatureDirectionKind rdf:about="http://open-services.net/ns/sysmlv2#featureDirectionKind_In">
    <rdfs:isDefinedBy rdf:resource="http://open-services.net/ns/sysmlv2#"/>
    <rdfs:comment>Values of the Feature on each instance of its domain are determined externally to that instance and used internally.</rdfs:comment>
    <rdfs:label>featureDirectionKind_In</rdfs:label>
  </oslc_sysmlv2:FeatureDirectionKind>
  <oslc_sysmlv2:StateSubactionKind rdf:about="http://open-services.net/ns/sysmlv2#stateSubactionKind_Entry">
    <rdfs:isDefinedBy rdf:resource="http://open-services.net/ns/sysmlv2#"/>
    <rdfs:comment>Indicates that the action of a StateSubactionMembership is an entryAction.</rdfs:comment>
    <rdfs:label>stateSubactionKind_Entry</rdfs:label>
  </oslc_sysmlv2:StateSubactionKind>
  <oslc_sysmlv2:FeatureDirectionKind rdf:about="http://open-services.net/ns/sysmlv2#featureDirectionKind_Inout">
    <rdfs:isDefinedBy rdf:resource="http://open-services.net/ns/sysmlv2#"/>
    <rdfs:comment>Values of the Feature on each instance are determined either as in or out directions, or both.</rdfs:comment>
    <rdfs:label>featureDirectionKind_Inout</rdfs:label>
  </oslc_sysmlv2:FeatureDirectionKind>
  <oslc_sysmlv2:VisibilityKind rdf:about="http://open-services.net/ns/sysmlv2#visibilityKind_Protected">
    <rdfs:isDefinedBy rdf:resource="http://open-services.net/ns/sysmlv2#"/>
    <rdfs:comment>An intermediate level of visibility between public and private. By default, it is equivalent to private for the purposes of normal access to and import of Elements from a Namespace. However, other Relationships may be specified to include Memberships with protected visibility in the list of memberships for a Namespace (e.g., Specialization).</rdfs:comment>
    <rdfs:label>visibilityKind_Protected</rdfs:label>
  </oslc_sysmlv2:VisibilityKind>
</rdf:RDF>
