{
    "@graph": [
        {
            "@id": "oslc_config:ChangeSetSelections",
            "rdfs:comment": "A resource listing the version resources selected by a change set configuration.",
            "rdfs:subClassOf": {
                "@id": "oslc_config:Selections"
            },
            "rdfs:label": "ChangeSetSelections",
            "rdfs:isDefinedBy": {
                "@id": "http://open-services.net/ns/config#"
            },
            "@type": "rdfs:Class"
        },
        {
            "@id": "oslc_config:Selections",
            "rdfs:comment": "A resource listing the version resources selected by a configuration.",
            "rdfs:label": "Selections",
            "rdfs:isDefinedBy": {
                "@id": "http://open-services.net/ns/config#"
            },
            "@type": "rdfs:Class"
        },
        {
            "@id": "http://open-services.net/ns/config#",
            "dcterms:dateCopyrighted": "2012-2023",
            "dcterms:title": "OSLC Configuration Management vocabulary",
            "dcterms:issued": {
                "@value": "2023-07-23",
                "@type": "http://www.w3.org/2001/XMLSchema#date"
            },
            "dcterms:isPartOf": {
                "@id": "https://docs.oasis-open-projects.org/oslc-op/config/v1.0/os/oslc-config-mgt.html"
            },
            "dcterms:hasVersion": "PS",
            "vann:preferredNamespacePrefix": "oslc_config",
            "rdfs:label": "OSLC Configuration Management vocabulary",
            "dcterms:publisher": {
                "@id": "https://open-services.net/about/"
            },
            "dcterms:source": {
                "@id": "https://docs.oasis-open-projects.org/oslc-op/config/v1.0/os/config-vocab.ttl"
            },
            "dcterms:description": "The OSLC Configuration Management vocabulary defines terms for versioned resources and configurations of those versioned resources.",
            "dcterms:license": {
                "@id": "http://www.apache.org/licenses/LICENSE-2.0"
            },
            "@type": "owl:Ontology"
        },
        {
            "@id": "oslc_config:Activity",
            "rdfs:comment": "An activity is a read-only resource representing a long-running operation, such as recursive baseline or stream creation.",
            "rdfs:label": "Activity",
            "rdfs:isDefinedBy": {
                "@id": "http://open-services.net/ns/config#"
            },
            "@type": "rdfs:Class"
        },
        {
            "@id": "oslc_config:Configuration",
            "rdfs:comment": "A configuration identifies a set of versions of resources in a component. Configurations commonly identify exactly one version of each resource in a component. Configurations can also assemble other configurations into a shared context across multiple components.",
            "rdfs:label": "Configuration",
            "rdfs:isDefinedBy": {
                "@id": "http://open-services.net/ns/config#"
            },
            "@type": "rdfs:Class"
        },
        {
            "@id": "oslc_config:RemoveAll",
            "rdfs:comment": "For a change set, an indicator that all selections in the overriden configuration are to be ignored; all selections are defined by the change set.",
            "rdfs:label": "RemovalAll",
            "rdfs:isDefinedBy": {
                "@id": "http://open-services.net/ns/config#"
            },
            "@type": "rdfs:Class"
        },
        {
            "@id": "oslc_config:ChangeSet",
            "rdfs:comment": "A change set configuration represents a set of changes (including additions and removals) to some other configuration.",
            "rdfs:subClassOf": {
                "@id": "oslc_config:Configuration"
            },
            "rdfs:label": "ChangeSet",
            "rdfs:isDefinedBy": {
                "@id": "http://open-services.net/ns/config#"
            },
            "@type": "rdfs:Class"
        },
        {
            "@id": "oslc_config:configuration",
            "rdfs:comment": "A reference to a Configuration resource.",
            "rdfs:label": "configuration",
            "rdfs:isDefinedBy": {
                "@id": "http://open-services.net/ns/config#"
            },
            "@type": "rdf:Property"
        },
        {
            "@id": "oslc_config:baselineOfStream",
            "rdfs:comment": "The stream from which a baseline was made.",
            "rdfs:range": {
                "@id": "oslc_config:Stream"
            },
            "rdfs:label": "baselineOfStream",
            "rdfs:isDefinedBy": {
                "@id": "http://open-services.net/ns/config#"
            },
            "@type": "rdf:Property"
        },
        {
            "@id": "oslc_config:Stream",
            "rdfs:comment": "A mutable configuration. Contributions to this configuration can be streams or baselines.",
            "rdfs:subClassOf": {
                "@id": "oslc_config:Configuration"
            },
            "rdfs:label": "Stream",
            "rdfs:isDefinedBy": {
                "@id": "http://open-services.net/ns/config#"
            },
            "@type": "rdfs:Class"
        },
        {
            "@id": "oslc_config:committer",
            "rdfs:comment": "The entity that committed or checked in this resource.",
            "rdfs:label": "committer",
            "rdfs:isDefinedBy": {
                "@id": "http://open-services.net/ns/config#"
            },
            "@type": "rdf:Property"
        },
        {
            "@id": "oslc_config:previousBaseline",
            "rdfs:comment": "For a stream or a baseline, a link to the most recent baseline of the same stream.",
            "rdfs:range": {
                "@id": "oslc_config:Baseline"
            },
            "rdfs:label": "previousBaseline",
            "rdfs:isDefinedBy": {
                "@id": "http://open-services.net/ns/config#"
            },
            "@type": "rdf:Property"
        },
        {
            "@id": "oslc_config:Baseline",
            "rdfs:comment": "An immutable configuration with immutable selections of immutable resources, with immutable contributions that are themselves baselines.",
            "rdfs:subClassOf": {
                "@id": "oslc_config:Configuration"
            },
            "rdfs:label": "Baseline",
            "rdfs:isDefinedBy": {
                "@id": "http://open-services.net/ns/config#"
            },
            "@type": "rdfs:Class"
        },
        {
            "@id": "oslc_config:progressMessage",
            "rdfs:comment": "Text describing the progress of an operation.",
            "rdfs:label": "progressMessage",
            "rdfs:isDefinedBy": {
                "@id": "http://open-services.net/ns/config#"
            },
            "@type": "rdf:Property"
        },
        {
            "@id": "oslc_config:configurations",
            "rdfs:comment": "A Linked Data Platform Container for configurations of a component.",
            "rdfs:label": "configurations",
            "rdfs:isDefinedBy": {
                "@id": "http://open-services.net/ns/config#"
            },
            "@type": "rdf:Property"
        },
        {
            "@id": "oslc_config:component",
            "rdfs:comment": "A reference to a Component resource.",
            "rdfs:label": "component",
            "rdfs:isDefinedBy": {
                "@id": "http://open-services.net/ns/config#"
            },
            "@type": "rdf:Property"
        },
        {
            "@id": "oslc_config:contribution",
            "rdfs:comment": "A reference to a Contribution resource.",
            "rdfs:range": {
                "@id": "oslc_config:Contribution"
            },
            "rdfs:label": "contribution",
            "rdfs:isDefinedBy": {
                "@id": "http://open-services.net/ns/config#"
            },
            "@type": "rdf:Property"
        },
        {
            "@id": "oslc_config:Contribution",
            "rdfs:comment": "A contribution represents the contribution of one configuration to another.",
            "rdfs:label": "Contribution",
            "rdfs:isDefinedBy": {
                "@id": "http://open-services.net/ns/config#"
            },
            "@type": "rdfs:Class"
        },
        {
            "@id": "oslc_config:ConfigurationSettings",
            "rdfs:comment": "Information about settings and preferences for a Configuration Management service.",
            "rdfs:label": "ConfigurationSettings",
            "rdfs:isDefinedBy": {
                "@id": "http://open-services.net/ns/config#"
            },
            "@type": "rdfs:Class"
        },
        {
            "@id": "oslc_config:selections",
            "rdfs:comment": "A reference to a Selections resource.",
            "rdfs:range": {
                "@id": "oslc_config:Selections"
            },
            "rdfs:label": "selections",
            "rdfs:isDefinedBy": {
                "@id": "http://open-services.net/ns/config#"
            },
            "@type": "rdf:Property"
        },
        {
            "@id": "oslc_config:selects",
            "rdfs:comment": "A reference to a selected version resource.",
            "rdfs:label": "selects",
            "rdfs:isDefinedBy": {
                "@id": "http://open-services.net/ns/config#"
            },
            "@type": "rdf:Property"
        },
        {
            "@id": "oslc_config:versionId",
            "rdfs:comment": "A human-readable version identifier.",
            "rdfs:label": "versionId",
            "rdfs:isDefinedBy": {
                "@id": "http://open-services.net/ns/config#"
            },
            "@type": "rdf:Property"
        },
        {
            "@id": "oslc_config:VersionResource",
            "rdfs:comment": "This type is used as a marker for any version resource.",
            "rdfs:label": "VersionResource",
            "rdfs:isDefinedBy": {
                "@id": "http://open-services.net/ns/config#"
            },
            "@type": "rdfs:Class"
        },
        {
            "@id": "oslc_config:accepts",
            "rdfs:comment": "A type of configuration acceptable as a contribution to the subject configuration.",
            "rdfs:range": {
                "@id": "oslc_config:Configuration"
            },
            "rdfs:label": "accepts",
            "rdfs:isDefinedBy": {
                "@id": "http://open-services.net/ns/config#"
            },
            "@type": "rdf:Property"
        },
        {
            "@id": "oslc_config:Removals",
            "rdfs:comment": "For a change set, the selections to be removed from an overridden configuration.",
            "rdfs:label": "Removals",
            "rdfs:isDefinedBy": {
                "@id": "http://open-services.net/ns/config#"
            },
            "@type": "rdfs:Class"
        },
        {
            "@id": "oslc_config:contributionOrder",
            "rdfs:comment": "The ordering value for a contribution.",
            "rdfs:label": "contributionOrder",
            "rdfs:isDefinedBy": {
                "@id": "http://open-services.net/ns/config#"
            },
            "@type": "rdf:Property"
        },
        {
            "@id": "oslc_config:acceptedBy",
            "rdfs:comment": "A type of configuration accepted as a contribution by the subject configuration.",
            "rdfs:range": {
                "@id": "oslc_config:Configuration"
            },
            "rdfs:label": "acceptedBy",
            "rdfs:isDefinedBy": {
                "@id": "http://open-services.net/ns/config#"
            },
            "@type": "rdf:Property"
        },
        {
            "@id": "oslc_config:UnboundSelections",
            "rdfs:comment": "An indicator that a set of selections are as-yet unbound concept resources as opposed to bound version resources.",
            "rdfs:label": "UnboundSelections",
            "rdfs:isDefinedBy": {
                "@id": "http://open-services.net/ns/config#"
            },
            "@type": "rdfs:Class"
        },
        {
            "@id": "oslc_config:PersonalConfiguration",
            "rdfs:comment": "A configuration intended for use by a single agent, rather than shared.",
            "rdfs:subClassOf": {
                "@id": "oslc_config:Configuration"
            },
            "rdfs:label": "PersonalConfiguration",
            "rdfs:isDefinedBy": {
                "@id": "http://open-services.net/ns/config#"
            },
            "@type": "rdfs:Class"
        },
        {
            "@id": "oslc_config:Component",
            "rdfs:comment": "A unit of organization consisting of a set of versioned resources. Components are the units of configurability, and form reusable assets or building blocks.",
            "rdfs:label": "Component",
            "rdfs:isDefinedBy": {
                "@id": "http://open-services.net/ns/config#"
            },
            "@type": "rdfs:Class"
        },
        {
            "@id": "oslc_config:baselines",
            "rdfs:comment": "A Linked Data Platform Container for baselines of a stream.",
            "rdfs:label": "baselines",
            "rdfs:isDefinedBy": {
                "@id": "http://open-services.net/ns/config#"
            },
            "@type": "rdf:Property"
        },
        {
            "@id": "oslc_config:committed",
            "rdfs:comment": "Date and time a resource was committed, or checked in.",
            "rdfs:label": "committed",
            "rdfs:isDefinedBy": {
                "@id": "http://open-services.net/ns/config#"
            },
            "@type": "rdf:Property"
        },
        {
            "@id": "oslc_config:branch",
            "rdfs:comment": "Identifies a resource as one for a specific branch or variant of the component.",
            "rdfs:label": "branch",
            "rdfs:isDefinedBy": {
                "@id": "http://open-services.net/ns/config#"
            },
            "@type": "rdf:Property"
        },
        {
            "@id": "oslc_config:configurationSettings",
            "rdfs:comment": "A reference to information about settings and preferences for a Configuration Management service.",
            "rdfs:label": "configurationSettings",
            "rdfs:isDefinedBy": {
                "@id": "http://open-services.net/ns/config#"
            },
            "@type": "rdf:Property"
        },
        {
            "@id": "oslc_config:mutable",
            "rdfs:comment": "A boolean property indicating whether or not a resource is modifiable; replaced by use of Baseline and Stream types.",
            "vs:term_status": "archaic",
            "rdfs:label": "mutable",
            "rdfs:isDefinedBy": {
                "@id": "http://open-services.net/ns/config#"
            },
            "@type": "rdf:Property"
        },
        {
            "@id": "oslc_config:release",
            "rdfs:comment": "A reference to a resource representing a release.",
            "rdfs:label": "release",
            "rdfs:isDefinedBy": {
                "@id": "http://open-services.net/ns/config#"
            },
            "@type": "rdf:Property"
        },
        {
            "@id": "oslc_config:globalConfigurationService",
            "rdfs:comment": "An oslc:usage value marking a global configuration service.",
            "rdfs:label": "globalConfigurationService",
            "rdfs:isDefinedBy": {
                "@id": "http://open-services.net/ns/config#"
            },
            "@type": "rdfs:Resource"
        },
        {
            "@id": "oslc_config:overrides",
            "rdfs:comment": "A reference to a configuration modified by a change set configuration.",
            "rdfs:label": "overrides",
            "rdfs:isDefinedBy": {
                "@id": "http://open-services.net/ns/config#"
            },
            "@type": "rdf:Property"
        },
        {
            "@id": "oslc_config:streams",
            "rdfs:comment": "A Linked Data Platform Container for streams created from a baseline.",
            "rdfs:label": "streams",
            "rdfs:isDefinedBy": {
                "@id": "http://open-services.net/ns/config#"
            },
            "@type": "rdf:Property"
        },
        {
            "@id": "oslc_config:derivedFrom",
            "rdfs:comment": "A resource from which this resource was derived; the use of prov:wasDerivedFrom is preferred.",
            "vs:term_status": "archaic",
            "rdfs:label": "derivedFrom",
            "rdfs:isDefinedBy": {
                "@id": "http://open-services.net/ns/config#"
            },
            "@type": "rdf:Property"
        }
    ],
    "@context": {
        "owl": "http://www.w3.org/2002/07/owl#",
        "rdf": "http://www.w3.org/1999/02/22-rdf-syntax-ns#",
        "dcterms": "http://purl.org/dc/terms/",
        "rdfs": "http://www.w3.org/2000/01/rdf-schema#",
        "oslc_config": "http://open-services.net/ns/config#",
        "vann": "http://purl.org/vocab/vann/",
        "vs": "http://www.w3.org/2003/06/sw-vocab-status/ns#"
    }
}
